@prefix cim:     <https://cim.ucaiug.io/ns#> .
@prefix cims:    <http://iec.ch/TC57/1999/rdf-schema-extensions-19990926#> .
@prefix co:      <https://ap.cim4.eu/Contingency#> .
@prefix dcat:    <http://www.w3.org/ns/dcat#> .
@prefix dcterms: <http://purl.org/dc/terms/#> .
@prefix nc:      <https://cim4.eu/ns/nc#> .
@prefix owl:     <http://www.w3.org/2002/07/owl#> .
@prefix profcim: <https://cim.ucaiug.io/ns/prof-cim#> .
@prefix rdf:     <http://www.w3.org/1999/02/22-rdf-syntax-ns#> .
@prefix rdfs:    <http://www.w3.org/2000/01/rdf-schema#> .

cim:Boolean  rdf:type           rdfs:Class ;
        rdfs:comment            "A type with the value space \"true\" and \"false\"." ;
        rdfs:label              "Boolean"@en ;
        cims:belongsToCategory  co:Package_ContingencyProfile ;
        cims:stereotype         "Primitive" .

cim:Contingency  rdf:type       rdfs:Class ;
        rdfs:comment            "An event threatening system reliability, consisting of one or more contingency elements." ;
        rdfs:label              "Contingency"@en ;
        rdfs:subClassOf         cim:IdentifiedObject ;
        cims:belongsToCategory  co:Package_ContingencyProfile .

cim:Contingency.ContingencyElement
        rdf:type              rdf:Property ;
        rdfs:comment          "A contingency can have any number of contingency elements." ;
        rdfs:domain           cim:Contingency ;
        rdfs:label            "ContingencyElement"@en ;
        rdfs:range            cim:ContingencyElement ;
        cims:AssociationUsed  "No" ;
        cims:inverseRoleName  cim:ContingencyElement.Contingency ;
        cims:multiplicity     cims:M:1..n ;
        cims:stereotype       <http://iec.ch/TC57/NonStandard/UML#ofAggregate> .

cim:Contingency.SimulationEvents
        rdf:type              rdf:Property ;
        rdfs:comment          "Simulation event for a contingency." ;
        rdfs:domain           cim:Contingency ;
        rdfs:label            "SimulationEvents"@en ;
        rdfs:range            cim:SimulationEvents ;
        cims:AssociationUsed  "Yes" ;
        cims:inverseRoleName  cim:SimulationEvents.Contingency ;
        cims:multiplicity     cims:M:0..1 ;
        cims:stereotype       "NC" .

cim:ContingencyElement
        rdf:type                rdfs:Class ;
        rdfs:comment            "An element of a system event to be studied by contingency analysis, representing a change in status of a single piece of equipment. " ;
        rdfs:label              "ContingencyElement"@en ;
        rdfs:subClassOf         cim:IdentifiedObject ;
        cims:belongsToCategory  co:Package_ContingencyProfile .

cim:ContingencyElement.Contingency
        rdf:type              rdf:Property ;
        rdfs:comment          "A contingency element belongs to one contingency." ;
        rdfs:domain           cim:ContingencyElement ;
        rdfs:label            "Contingency"@en ;
        rdfs:range            cim:Contingency ;
        cims:AssociationUsed  "Yes" ;
        cims:inverseRoleName  cim:Contingency.ContingencyElement ;
        cims:multiplicity     cims:M:1 .

cim:ContingencyEquipment
        rdf:type                rdfs:Class ;
        rdfs:comment            "Equipment whose in service status is to change, such as a power transformer or AC line segment." ;
        rdfs:label              "ContingencyEquipment"@en ;
        rdfs:subClassOf         cim:ContingencyElement ;
        cims:belongsToCategory  co:Package_ContingencyProfile ;
        cims:stereotype         <http://iec.ch/TC57/NonStandard/UML#concrete> .

cim:ContingencyEquipment.Equipment
        rdf:type              rdf:Property ;
        rdfs:comment          "The single piece of equipment to which to apply the contingency." ;
        rdfs:domain           cim:ContingencyEquipment ;
        rdfs:label            "Equipment"@en ;
        rdfs:range            cim:Equipment ;
        cims:AssociationUsed  "Yes" ;
        cims:inverseRoleName  cim:Equipment.ContingencyEquipment ;
        cims:multiplicity     cims:M:1 .

cim:ContingencyEquipment.contingentStatus
        rdf:type           rdf:Property ;
        rdfs:comment       "The status for the associated equipment when in the contingency state.   This status is independent of the case to which the contingency is originally applied, but defines the equipment status when the contingency is applied." ;
        rdfs:domain        cim:ContingencyEquipment ;
        rdfs:label         "contingentStatus"@en ;
        rdfs:range         cim:ContingencyEquipmentStatusKind ;
        cims:multiplicity  cims:M:1..1 ;
        cims:stereotype    <http://iec.ch/TC57/NonStandard/UML#attribute> .

cim:ContingencyEquipmentStatusKind
        rdf:type                rdfs:Class ;
        rdfs:comment            "Indicates the state which the contingency equipment is to be in when the contingency is applied." ;
        rdfs:label              "ContingencyEquipmentStatusKind"@en ;
        cims:belongsToCategory  co:Package_ContingencyProfile ;
        cims:stereotype         <http://iec.ch/TC57/NonStandard/UML#enumeration> .

cim:ContingencyEquipmentStatusKind.inService
        rdf:type         cim:ContingencyEquipmentStatusKind ;
        rdfs:comment     "The equipment is to be put into service." ;
        rdfs:label       "inService"@en ;
        cims:stereotype  "enum" .

cim:ContingencyEquipmentStatusKind.outOfService
        rdf:type         cim:ContingencyEquipmentStatusKind ;
        rdfs:comment     "The equipment is to be taken out of service." ;
        rdfs:label       "outOfService"@en ;
        cims:stereotype  "enum" .

cim:Date  rdf:type              rdfs:Class ;
        rdfs:comment            "Date as \"yyyy-mm-dd\", which conforms with ISO 8601. UTC time zone is specified as \"yyyy-mm-ddZ\". A local timezone relative UTC is specified as \"yyyy-mm-dd(+/-)hh:mm\"." ;
        rdfs:label              "Date"@en ;
        cims:belongsToCategory  co:Package_DocContingencyProfile ;
        cims:stereotype         "Primitive" .

cim:DateTime  rdf:type          rdfs:Class ;
        rdfs:comment            "Date and time as \"yyyy-mm-ddThh:mm:ss.sss\", which conforms with ISO 8601. UTC time zone is specified as \"yyyy-mm-ddThh:mm:ss.sssZ\". A local timezone relative UTC is specified as \"yyyy-mm-ddThh:mm:ss.sss-hh:mm\". The second component (shown here as \"ss.sss\") could have any number of digits in its fractional part to allow any kind of precision beyond seconds." ;
        rdfs:label              "DateTime"@en ;
        cims:belongsToCategory  co:Package_DocContingencyProfile ;
        cims:stereotype         "Primitive" .

cim:Equipment  rdf:type         rdfs:Class ;
        rdfs:comment            "The parts of a power system that are physical devices, electronic or mechanical." ;
        rdfs:label              "Equipment"@en ;
        cims:belongsToCategory  co:Package_ContingencyProfile .

cim:Equipment.ContingencyEquipment
        rdf:type              rdf:Property ;
        rdfs:comment          "The contingency equipments in which this equipment participates." ;
        rdfs:domain           cim:Equipment ;
        rdfs:label            "ContingencyEquipment"@en ;
        rdfs:range            cim:ContingencyEquipment ;
        cims:AssociationUsed  "No" ;
        cims:inverseRoleName  cim:ContingencyEquipment.Equipment ;
        cims:multiplicity     cims:M:0..n .

cim:Float  rdf:type             rdfs:Class ;
        rdfs:comment            "A floating point number. The range is unspecified and not limited." ;
        rdfs:label              "Float"@en ;
        cims:belongsToCategory  co:Package_ContingencyProfile ;
        cims:stereotype         "Primitive" .

cim:IdentifiedObject  rdf:type  rdfs:Class ;
        rdfs:comment            "This is a root class to provide common identification for all classes needing identification and naming attributes." ;
        rdfs:label              "IdentifiedObject"@en ;
        cims:belongsToCategory  co:Package_ContingencyProfile .

cim:IdentifiedObject.description
        rdf:type           rdf:Property ;
        rdfs:comment       "The description is a free human readable text describing or naming the object. It may be non unique and may not correlate to a naming hierarchy." ;
        rdfs:domain        cim:IdentifiedObject ;
        rdfs:label         "description"@en ;
        cims:dataType      cim:String ;
        cims:multiplicity  cims:M:0..1 ;
        cims:stereotype    <http://iec.ch/TC57/NonStandard/UML#attribute> .

cim:IdentifiedObject.mRID
        rdf:type           rdf:Property ;
        rdfs:comment       "Master resource identifier issued by a model authority. The mRID is unique within an exchange context. Global uniqueness is easily achieved by using a UUID, as specified in RFC 4122, for the mRID. The use of UUID is strongly recommended.\nFor CIMXML data files in RDF syntax conforming to IEC 61970-552, the mRID is mapped to rdf:ID or rdf:about attributes that identify CIM object elements." ;
        rdfs:domain        cim:IdentifiedObject ;
        rdfs:label         "mRID"@en ;
        cims:dataType      cim:String ;
        cims:multiplicity  cims:M:1..1 ;
        cims:stereotype    <http://iec.ch/TC57/NonStandard/UML#attribute> .

cim:IdentifiedObject.name
        rdf:type           rdf:Property ;
        rdfs:comment       "The name is any free human readable and possibly non unique text naming the object." ;
        rdfs:domain        cim:IdentifiedObject ;
        rdfs:label         "name"@en ;
        cims:dataType      cim:String ;
        cims:multiplicity  cims:M:0..1 ;
        cims:stereotype    <http://iec.ch/TC57/NonStandard/UML#attribute> .

cim:PerCent  rdf:type           rdfs:Class ;
        rdfs:comment            "Percentage on a defined base.   For example, specify as 100 to indicate at the defined base." ;
        rdfs:label              "PerCent"@en ;
        cims:belongsToCategory  co:Package_ContingencyProfile ;
        cims:stereotype         "CIMDatatype" .

cim:PerCent.multiplier
        rdf:type           rdf:Property ;
        rdfs:domain        cim:PerCent ;
        rdfs:label         "multiplier"@en ;
        rdfs:range         cim:UnitMultiplier ;
        cims:isFixed       "none" ;
        cims:multiplicity  cims:M:0..1 ;
        cims:stereotype    <http://iec.ch/TC57/NonStandard/UML#attribute> .

cim:PerCent.unit  rdf:type  rdf:Property ;
        rdfs:domain        cim:PerCent ;
        rdfs:label         "unit"@en ;
        rdfs:range         cim:UnitSymbol ;
        cims:isFixed       "none" ;
        cims:multiplicity  cims:M:0..1 ;
        cims:stereotype    <http://iec.ch/TC57/NonStandard/UML#attribute> .

cim:PerCent.value  rdf:type  rdf:Property ;
        rdfs:comment       "Normally 0 to 100 on a defined base." ;
        rdfs:domain        cim:PerCent ;
        rdfs:label         "value"@en ;
        cims:dataType      cim:Float ;
        cims:multiplicity  cims:M:0..1 ;
        cims:stereotype    <http://iec.ch/TC57/NonStandard/UML#attribute> .

cim:SimulationEvents  rdf:type  rdfs:Class ;
        rdfs:comment            "A configuration or a set of events executed during a simulation." ;
        rdfs:label              "SimulationEvents"@en ;
        cims:belongsToCategory  co:Package_ContingencyProfile .

cim:SimulationEvents.Contingency
        rdf:type              rdf:Property ;
        rdfs:comment          "Contingency which has simulation events." ;
        rdfs:domain           cim:SimulationEvents ;
        rdfs:label            "Contingency"@en ;
        rdfs:range            cim:Contingency ;
        cims:AssociationUsed  "No" ;
        cims:inverseRoleName  cim:Contingency.SimulationEvents ;
        cims:multiplicity     cims:M:0..1 ;
        cims:stereotype       "NC" .

cim:String  rdf:type            rdfs:Class ;
        rdfs:comment            "A string consisting of a sequence of characters. The character encoding is UTF-8. The string length is unspecified and unlimited." ;
        rdfs:label              "String"@en ;
        cims:belongsToCategory  co:Package_ContingencyProfile ;
        cims:stereotype         "Primitive" .

cim:UnitMultiplier  rdf:type    rdfs:Class ;
        rdfs:comment            "The unit multipliers defined for the CIM.  When applied to unit symbols, the unit symbol is treated as a derived unit. Regardless of the contents of the unit symbol text, the unit symbol shall be treated as if it were a single-character unit symbol. Unit symbols should not contain multipliers, and it should be left to the multiplier to define the multiple for an entire data type. \n\nFor example, if a unit symbol is \"m2Pers\" and the multiplier is \"k\", then the value is k(m**2/s), and the multiplier applies to the entire final value, not to any individual part of the value. This can be conceptualized by substituting a derived unit symbol for the unit type. If one imagines that the symbol \"Þ\" represents the derived unit \"m2Pers\", then applying the multiplier \"k\" can be conceptualized simply as \"kÞ\".\n\nFor example, the SI unit for mass is \"kg\" and not \"g\".  If the unit symbol is defined as \"kg\", then the multiplier is applied to \"kg\" as a whole and does not replace the \"k\" in front of the \"g\". In this case, the multiplier of \"m\" would be used with the unit symbol of \"kg\" to represent one gram.  As a text string, this violates the instructions in IEC 80000-1. However, because the unit symbol in CIM is treated as a derived unit instead of as an SI unit, it makes more sense to conceptualize the \"kg\" as if it were replaced by one of the proposed replacements for the SI mass symbol. If one imagines that the \"kg\" were replaced by a symbol \"Þ\", then it is easier to conceptualize the multiplier \"m\" as creating the proper unit \"mÞ\", and not the forbidden unit \"mkg\"." ;
        rdfs:label              "UnitMultiplier"@en ;
        cims:belongsToCategory  co:Package_ContingencyProfile ;
        cims:stereotype         <http://iec.ch/TC57/NonStandard/UML#enumeration> .

cim:UnitMultiplier.none
        rdf:type         cim:UnitMultiplier ;
        rdfs:comment     "No multiplier or equivalently multiply by 1." ;
        rdfs:label       "none"@en ;
        cims:stereotype  "enum" .

cim:UnitSymbol  rdf:type        rdfs:Class ;
        rdfs:comment            "The derived units defined for usage in the CIM. In some cases, the derived unit is equal to an SI unit. Whenever possible, the standard derived symbol is used instead of the formula for the derived unit. For example, the unit symbol Farad is defined as \"F\" instead of \"CPerV\". In cases where a standard symbol does not exist for a derived unit, the formula for the unit is used as the unit symbol. For example, density does not have a standard symbol and so it is represented as \"kgPerm3\". With the exception of the \"kg\", which is an SI unit, the unit symbols do not contain multipliers and therefore represent the base derived unit to which a multiplier can be applied as a whole. \nEvery unit symbol is treated as an unparseable text as if it were a single-letter symbol. The meaning of each unit symbol is defined by the accompanying descriptive text and not by the text contents of the unit symbol.\nTo allow the widest possible range of serializations without requiring special character handling, several substitutions are made which deviate from the format described in IEC 80000-1. The division symbol \"/\" is replaced by the letters \"Per\". Exponents are written in plain text after the unit as \"m3\" instead of being formatted as \"m\" with a superscript of 3  or introducing a symbol as in \"m^3\". The degree symbol \"°\" is replaced with the letters \"deg\". Any clarification of the meaning for a substitution is included in the description for the unit symbol.\nNon-SI units are included in list of unit symbols to allow sources of data to be correctly labelled with their non-SI units (for example, a GPS sensor that is reporting numbers that represent feet instead of meters). This allows software to use the unit symbol information correctly convert and scale the raw data of those sources into SI-based units. \nThe integer values are used for harmonization with IEC 61850." ;
        rdfs:label              "UnitSymbol"@en ;
        cims:belongsToCategory  co:Package_ContingencyProfile ;
        cims:stereotype         <http://iec.ch/TC57/NonStandard/UML#enumeration> .

cim:UnitSymbol.none  rdf:type  cim:UnitSymbol ;
        rdfs:comment     "Dimension less quantity, e.g. count, per unit, etc." ;
        rdfs:label       "none"@en ;
        cims:stereotype  "enum" .

co:Ontology  rdf:type         owl:Ontology ;
        dcterms:conformsTo    "file://CIM100_CGMES31v01_501-20v02_NC23v62_MM10v01.eap" , "urn:iso:std:iec:61970-401:draft:ed-1" , "urn:iso:std:iec:61970-301:ed-7:amd1" , "urn:iso:std:iec:61970-501:draft:ed-2" , "urn:iso:std:iec:61970-600-2:ed-1" , "file://iec61970cim17v40_iec61968cim13v13a_iec62325cim03v17a.eap" ;
        dcterms:creator       "ENTSO-E CIM WG NC project"@en ;
        dcterms:description   "This vocabulary is describing the contingency profile."@en ;
        dcterms:identifier    "urn:uuid:8947de1c-6e53-4f1f-82c3-99ef118db9eb" ;
        dcterms:language      "en-GB" ;
        dcterms:license       "https://www.apache.org/licenses/LICENSE-2.0"@en ;
        dcterms:modified      "2024-03-20"^^<http://www.w3.org/2001/XMLSchema#date> ;
        dcterms:publisher     "ENTSO-E"@en ;
        dcterms:rightsHolder  "ENTSO-E"@en ;
        dcterms:title         "Contingency Vocabulary"@en ;
        owl:priorVersion      <http://entsoe.eu/ns/CIM/Contingency-EU/2.2> ;
        owl:versionIRI        <https://ap.cim4.eu/Contingency/2.3> ;
        owl:versionInfo       "2.3.0"@en ;
        dcat:keyword          "CO" ;
        dcat:theme            "vocabulary"@en .

co:Package_ContingencyProfile
        rdf:type      cims:ClassCategory ;
        rdfs:comment  "This package contains contingency profile." ;
        rdfs:label    "ContingencyProfile"@en .

co:Package_DocContingencyProfile
        rdf:type      cims:ClassCategory ;
        rdfs:comment  "This package contains datatypes used only in the RDFS header." ;
        rdfs:label    "DocContingencyProfile"@en .

nc:Contingency.EquipmentOperator
        rdf:type              rdf:Property ;
        rdfs:comment          "System operator that is operating the equipment that is being run a contingency on." ;
        rdfs:domain           cim:Contingency ;
        rdfs:label            "EquipmentOperator"@en ;
        rdfs:range            nc:SystemOperator ;
        cims:AssociationUsed  "Yes" ;
        cims:inverseRoleName  nc:SystemOperator.Contingency ;
        cims:multiplicity     cims:M:0..1 ;
        cims:stereotype       "NC" .

nc:Contingency.normalMustStudy
        rdf:type           rdf:Property ;
        rdfs:comment       "Specifies the requirement of study the contingency under normal operating conditions. True means the contingency must be study in a normal scenario. False means that the contingency does not need to be included in the scenario. This is the default value if mustStudy is missing." ;
        rdfs:domain        cim:Contingency ;
        rdfs:label         "normalMustStudy"@en ;
        cims:dataType      cim:Boolean ;
        cims:multiplicity  cims:M:1..1 ;
        cims:stereotype    "NC" ;
        cims:stereotype    <http://iec.ch/TC57/NonStandard/UML#attribute> .

nc:Contingency.normalProbability
        rdf:type           rdf:Property ;
        rdfs:comment       "Normal probability of the occurrence of the contingency based on normal operational condition. The value is used as the default if the probability is missing.\nThe allowed value range is [0,100]." ;
        rdfs:domain        cim:Contingency ;
        rdfs:label         "normalProbability"@en ;
        cims:dataType      cim:PerCent ;
        cims:multiplicity  cims:M:0..1 ;
        cims:stereotype    "NC" ;
        cims:stereotype    <http://iec.ch/TC57/NonStandard/UML#attribute> .

nc:ContingencyConditionKind
        rdf:type                rdfs:Class ;
        rdfs:comment            "Kinds of occurrence criteria of application." ;
        rdfs:label              "ContingencyConditionKind"@en ;
        cims:belongsToCategory  co:Package_ContingencyProfile ;
        cims:stereotype         "NC" ;
        cims:stereotype         <http://iec.ch/TC57/NonStandard/UML#enumeration> .

nc:ContingencyConditionKind.design
        rdf:type         nc:ContingencyConditionKind ;
        rdfs:comment     "Permanent occurrence factor which is design condition." ;
        rdfs:label       "design"@en ;
        cims:stereotype  "enum" .

nc:ContingencyConditionKind.environmental
        rdf:type         nc:ContingencyConditionKind ;
        rdfs:comment     "Temporary occurrence factor which is weather or environmental condition (e.g. storm)." ;
        rdfs:label       "environmental"@en ;
        cims:stereotype  "enum" .

nc:ContingencyConditionKind.geographicalLocation
        rdf:type         nc:ContingencyConditionKind ;
        rdfs:comment     "Permanent occurrence factor which is specific geographical location." ;
        rdfs:label       "geographicalLocation"@en ;
        cims:stereotype  "enum" .

nc:ContingencyConditionKind.malfunction
        rdf:type         nc:ContingencyConditionKind ;
        rdfs:comment     "Temporary occurrence factor which is life time or generic malfunction affecting the risk of failure condition." ;
        rdfs:label       "malfunction"@en ;
        cims:stereotype  "enum" .

nc:ContingencyConditionKind.operational
        rdf:type         nc:ContingencyConditionKind ;
        rdfs:comment     "Temporary occurrence factor which is operational condition." ;
        rdfs:label       "operational"@en ;
        cims:stereotype  "enum" .

nc:ExceptionalContingency
        rdf:type                rdfs:Class ;
        rdfs:comment            "Exceptional contingency means the simultaneous occurrence of multiple contingencies with a common cause." ;
        rdfs:label              "ExceptionalContingency"@en ;
        rdfs:subClassOf         cim:Contingency ;
        cims:belongsToCategory  co:Package_ContingencyProfile ;
        cims:stereotype         "NC" ;
        cims:stereotype         <http://iec.ch/TC57/NonStandard/UML#concrete> .

nc:ExceptionalContingency.kind
        rdf:type           rdf:Property ;
        rdfs:comment       "Defines the kind of relevance and criteria of application of the exceptional contingency." ;
        rdfs:domain        nc:ExceptionalContingency ;
        rdfs:label         "kind"@en ;
        rdfs:range         nc:ContingencyConditionKind ;
        cims:multiplicity  cims:M:1..1 ;
        cims:stereotype    "NC" ;
        cims:stereotype    <http://iec.ch/TC57/NonStandard/UML#attribute> .

nc:OrdinaryContingency
        rdf:type                rdfs:Class ;
        rdfs:comment            "Ordinary contingency means the occurrence of a contingency of a single branch or injection." ;
        rdfs:label              "OrdinaryContingency"@en ;
        rdfs:subClassOf         cim:Contingency ;
        cims:belongsToCategory  co:Package_ContingencyProfile ;
        cims:stereotype         "NC" ;
        cims:stereotype         <http://iec.ch/TC57/NonStandard/UML#concrete> .

nc:OutOfRangeContingency
        rdf:type                rdfs:Class ;
        rdfs:comment            "Out of range means the simultaneous occurrence of multiple contingencies without a common cause, or a loss of power generating modules with a total loss of generation capacity exceeding the reference incident." ;
        rdfs:label              "OutOfRangeContingency"@en ;
        rdfs:subClassOf         cim:Contingency ;
        cims:belongsToCategory  co:Package_ContingencyProfile ;
        cims:stereotype         "NC" ;
        cims:stereotype         <http://iec.ch/TC57/NonStandard/UML#concrete> .

nc:SystemOperator  rdf:type     rdfs:Class ;
        rdfs:comment            "System operator." ;
        rdfs:label              "SystemOperator"@en ;
        cims:belongsToCategory  co:Package_ContingencyProfile ;
        cims:stereotype         "NC" .

nc:SystemOperator.Contingency
        rdf:type              rdf:Property ;
        rdfs:comment          "Contingency for the equipment that is operated by the system operator." ;
        rdfs:domain           nc:SystemOperator ;
        rdfs:label            "Contingency"@en ;
        rdfs:range            cim:Contingency ;
        cims:AssociationUsed  "No" ;
        cims:inverseRoleName  nc:Contingency.EquipmentOperator ;
        cims:multiplicity     cims:M:0..n ;
        cims:stereotype       "NC" .

profcim:IRI  rdf:type           rdfs:Class ;
        rdfs:comment            "An IRI (Internationalized Resource Identifier) within an RDF graph is a Unicode string that conforms to the syntax defined in RFC 3987.\nThe primitive is serialized as rdf:resource in RDFXML.\nIRIs in the RDF abstract syntax must be absolute, and may contain a fragment identifier.\nIRI equality: Two IRIs are equal if and only if they are equivalent under Simple String Comparison according to section 5.1 of [RFC3987]. Further normalization must not be performed when comparing IRIs for equality.\nIRIs are a generalization of URIs [RFC3986] that permits a wider range of Unicode characters. Every absolute URI and URL is an IRI, but not every IRI is an URI. When IRIs are used in operations that are only defined for URIs, they must first be converted according to the mapping defined in section 3.1 of [RFC3987]. A notable example is retrieval over the HTTP protocol. The mapping involves UTF-8 encoding of non-ASCII characters, %-encoding of octets not allowed in URIs, and Punycode-encoding of domain names." ;
        rdfs:label              "IRI"@en ;
        cims:belongsToCategory  co:Package_DocContingencyProfile ;
        cims:stereotype         "profcim" , "Primitive" .
profcim:StringFixedLanguage
        rdf:type                rdfs:Class ;
        rdfs:comment            "A string consisting of a sequence of characters. The character encoding is UTF-8. The string length is unspecified and unlimited.\nThe primitive is serialized as literal without language support." ;
        rdfs:label              "StringFixedLanguage"@en ;
        cims:belongsToCategory  co:Package_DocContingencyProfile ;
        cims:stereotype         "profcim" , "Primitive" .

profcim:StringIRI  rdf:type     rdfs:Class ;
        rdfs:comment            "An IRI (Internationalized Resource Identifier) within an RDF graph is a Unicode string that conforms to the syntax defined in RFC 3987.\nThe primitive is serialized as literal without language support.\nIRIs in the RDF abstract syntax must be absolute, and may contain a fragment identifier.\nIRI equality: Two IRIs are equal if and only if they are equivalent under Simple String Comparison according to section 5.1 of [RFC3987]. Further normalization must not be performed when comparing IRIs for equality.\nIRIs are a generalization of URIs [RFC3986] that permits a wider range of Unicode characters. Every absolute URI and URL is an IRI, but not every IRI is an URI. When IRIs are used in operations that are only defined for URIs, they must first be converted according to the mapping defined in section 3.1 of [RFC3987]. A notable example is retrieval over the HTTP protocol. The mapping involves UTF-8 encoding of non-ASCII characters, %-encoding of octets not allowed in URIs, and Punycode-encoding of domain names." ;
        rdfs:label              "StringIRI"@en ;
        cims:belongsToCategory  co:Package_DocContingencyProfile ;
        cims:stereotype         "profcim" , "Primitive" .

profcim:URL  rdf:type           rdfs:Class ;
        rdfs:comment            "A Uniform Resource Locator (URL), colloquially termed a web address, is a reference to a web resource that specifies its location on a computer network and a mechanism for retrieving it. A URL is a specific type of Uniform Resource Identifier (URI), although many people use the two terms interchangeably.URLs occur most commonly to reference web pages (http), but are also used for file transfer (ftp), email (mailto), database access (JDBC), and many other applications." ;
        rdfs:label              "URL"@en ;
        cims:belongsToCategory  co:Package_DocContingencyProfile ;
        cims:stereotype         "profcim" , "Primitive" .

