@prefix cim:     <https://cim.ucaiug.io/ns#> .
@prefix cims:    <http://iec.ch/TC57/1999/rdf-schema-extensions-19990926#> .
@prefix dcat:    <http://www.w3.org/ns/dcat#> .
@prefix dcterms: <http://purl.org/dc/terms/#> .
@prefix gd:      <https://ap.cim4.eu/GridDisturbance#> .
@prefix nc:      <https://cim4.eu/ns/nc#> .
@prefix owl:     <http://www.w3.org/2002/07/owl#> .
@prefix profcim: <https://cim.ucaiug.io/ns/prof-cim#> .
@prefix rdf:     <http://www.w3.org/1999/02/22-rdf-syntax-ns#> .
@prefix rdfs:    <http://www.w3.org/2000/01/rdf-schema#> .

cim:ActivePower  rdf:type       rdfs:Class ;
        rdfs:comment            "Product of RMS value of the voltage and the RMS value of the in-phase component of the current." ;
        rdfs:label              "ActivePower"@en ;
        cims:belongsToCategory  gd:Package_GridDisturbanceProfile ;
        cims:stereotype         "CIMDatatype" .

cim:ActivePower.multiplier
        rdf:type           rdf:Property ;
        rdfs:domain        cim:ActivePower ;
        rdfs:label         "multiplier"@en ;
        rdfs:range         cim:UnitMultiplier ;
        cims:isFixed       "M" ;
        cims:multiplicity  cims:M:0..1 ;
        cims:stereotype    <http://iec.ch/TC57/NonStandard/UML#attribute> .

cim:ActivePower.unit  rdf:type  rdf:Property ;
        rdfs:domain        cim:ActivePower ;
        rdfs:label         "unit"@en ;
        rdfs:range         cim:UnitSymbol ;
        cims:isFixed       "W" ;
        cims:multiplicity  cims:M:0..1 ;
        cims:stereotype    <http://iec.ch/TC57/NonStandard/UML#attribute> .

cim:ActivePower.value
        rdf:type           rdf:Property ;
        rdfs:domain        cim:ActivePower ;
        rdfs:label         "value"@en ;
        cims:dataType      cim:Float ;
        cims:multiplicity  cims:M:0..1 ;
        cims:stereotype    <http://iec.ch/TC57/NonStandard/UML#attribute> .

cim:BaseVoltage  rdf:type       rdfs:Class ;
        rdfs:comment            "Defines a system base voltage which is referenced. " ;
        rdfs:label              "BaseVoltage"@en ;
        rdfs:subClassOf         cim:IdentifiedObject ;
        cims:belongsToCategory  gd:Package_GridDisturbanceProfile .

cim:BaseVoltage.Fault
        rdf:type              rdf:Property ;
        rdfs:comment          "The fault which belongs to the base voltage." ;
        rdfs:domain           cim:BaseVoltage ;
        rdfs:label            "Fault"@en ;
        rdfs:range            cim:Fault ;
        cims:AssociationUsed  "No" ;
        cims:inverseRoleName  cim:Fault.BaseVoltage ;
        cims:multiplicity     cims:M:0..n ;
        cims:stereotype       "NC" .

cim:Boolean  rdf:type           rdfs:Class ;
        rdfs:comment            "A type with the value space \"true\" and \"false\"." ;
        rdfs:label              "Boolean"@en ;
        cims:belongsToCategory  gd:Package_GridDisturbanceProfile ;
        cims:stereotype         "Primitive" .

cim:CoordinateSystem  rdf:type  rdfs:Class ;
        rdfs:comment            "Coordinate reference system." ;
        rdfs:label              "CoordinateSystem"@en ;
        rdfs:subClassOf         cim:IdentifiedObject ;
        cims:belongsToCategory  gd:Package_GridDisturbanceProfile ;
        cims:stereotype         <http://iec.ch/TC57/NonStandard/UML#concrete> .

cim:CoordinateSystem.Locations
        rdf:type              rdf:Property ;
        rdfs:comment          "All locations described with position points in this coordinate system." ;
        rdfs:domain           cim:CoordinateSystem ;
        rdfs:label            "Locations"@en ;
        rdfs:range            cim:Location ;
        cims:AssociationUsed  "No" ;
        cims:inverseRoleName  cim:Location.CoordinateSystem ;
        cims:multiplicity     cims:M:0..n .

cim:CoordinateSystem.crsUrn
        rdf:type           rdf:Property ;
        rdfs:comment       "A Uniform Resource Name (URN) for the coordinate reference system (crs) used to define 'Location.PositionPoints'.\nAn example would be the European Petroleum Survey Group (EPSG) code for a coordinate reference system, defined in URN under the Open Geospatial Consortium (OGC) namespace as: urn:ogc:def:crs:EPSG::XXXX, where XXXX is an EPSG code (a full list of codes can be found at the EPSG Registry web site http://www.epsg-registry.org/). To define the coordinate system as being WGS84 (latitude, longitude) using an EPSG OGC, this attribute would be urn:ogc:def:crs:EPSG::4236.\nA profile should limit this code to a set of allowed URNs agreed to by all sending and receiving parties." ;
        rdfs:domain        cim:CoordinateSystem ;
        rdfs:label         "crsUrn"@en ;
        cims:dataType      cim:String ;
        cims:multiplicity  cims:M:1..1 ;
        cims:stereotype    <http://iec.ch/TC57/NonStandard/UML#attribute> .

cim:Date  rdf:type              rdfs:Class ;
        rdfs:comment            "Date as \"yyyy-mm-dd\", which conforms with ISO 8601. UTC time zone is specified as \"yyyy-mm-ddZ\". A local timezone relative UTC is specified as \"yyyy-mm-dd(+/-)hh:mm\"." ;
        rdfs:label              "Date"@en ;
        cims:belongsToCategory  gd:Package_DocGridDisturbanceProfile ;
        cims:stereotype         "Primitive" .

cim:DateTime  rdf:type          rdfs:Class ;
        rdfs:comment            "Date and time as \"yyyy-mm-ddThh:mm:ss.sss\", which conforms with ISO 8601. UTC time zone is specified as \"yyyy-mm-ddThh:mm:ss.sssZ\". A local timezone relative UTC is specified as \"yyyy-mm-ddThh:mm:ss.sss-hh:mm\". The second component (shown here as \"ss.sss\") could have any number of digits in its fractional part to allow any kind of precision beyond seconds." ;
        rdfs:label              "DateTime"@en ;
        cims:belongsToCategory  gd:Package_GridDisturbanceProfile ;
        cims:stereotype         "Primitive" .

cim:Document  rdf:type          rdfs:Class ;
        rdfs:comment            "Parent class for different groupings of information collected and managed as a part of a business process. It will frequently contain references to other objects, such as assets, people and power system resources." ;
        rdfs:label              "Document"@en ;
        rdfs:subClassOf         cim:IdentifiedObject ;
        cims:belongsToCategory  gd:Package_GridDisturbanceProfile .

cim:Duration  rdf:type          rdfs:Class ;
        rdfs:comment            "Duration as \"PnYnMnDTnHnMnS\" which conforms to ISO 8601, where nY expresses a number of years, nM a number of months, nD a number of days. The letter T separates the date expression from the time expression and, after it, nH identifies a number of hours, nM a number of minutes and nS a number of seconds. The number of seconds could be expressed as a decimal number, but all other numbers are integers." ;
        rdfs:label              "Duration"@en ;
        cims:belongsToCategory  gd:Package_GridDisturbanceProfile ;
        cims:stereotype         "Primitive" .

cim:Equipment  rdf:type         rdfs:Class ;
        rdfs:comment            "The parts of a power system that are physical devices, electronic or mechanical." ;
        rdfs:label              "Equipment"@en ;
        cims:belongsToCategory  gd:Package_GridDisturbanceProfile ;
        cims:stereotype         "Description" .

cim:Equipment.Faults  rdf:type  rdf:Property ;
        rdfs:comment          "All faults on this equipment." ;
        rdfs:domain           cim:Equipment ;
        rdfs:label            "Faults"@en ;
        rdfs:range            cim:Fault ;
        cims:AssociationUsed  "No" ;
        cims:inverseRoleName  cim:Fault.FaultyEquipment ;
        cims:multiplicity     cims:M:0..1 .

cim:Equipment.Outages
        rdf:type              rdf:Property ;
        rdfs:comment          "All outages in which this equipment is involved." ;
        rdfs:domain           cim:Equipment ;
        rdfs:label            "Outages"@en ;
        rdfs:range            cim:Outage ;
        cims:AssociationUsed  "No" ;
        cims:inverseRoleName  cim:Outage.Equipments ;
        cims:multiplicity     cims:M:0..1 .

cim:Equipment.UnplannedOutage
        rdf:type              rdf:Property ;
        rdfs:comment          "The outage this tripped breaker is involved with." ;
        rdfs:domain           cim:Equipment ;
        rdfs:label            "UnplannedOutage"@en ;
        rdfs:range            cim:UnplannedOutage ;
        cims:AssociationUsed  "Yes" ;
        cims:inverseRoleName  cim:UnplannedOutage.TrippedEquipment ;
        cims:multiplicity     cims:M:0..1 ;
        cims:stereotype       "NC" .

cim:Fault  rdf:type             rdfs:Class ;
        rdfs:comment            "Abnormal condition causing current flow through conducting equipment, such as caused by equipment failure or short circuits from objects not typically modelled (for example, a tree falling on a line)." ;
        rdfs:label              "Fault"@en ;
        rdfs:subClassOf         cim:IdentifiedObject ;
        cims:belongsToCategory  gd:Package_GridDisturbanceProfile ;
        cims:stereotype         <http://iec.ch/TC57/NonStandard/UML#concrete> .

cim:Fault.BaseVoltage
        rdf:type              rdf:Property ;
        rdfs:comment          "The base voltage of this fault." ;
        rdfs:domain           cim:Fault ;
        rdfs:label            "BaseVoltage"@en ;
        rdfs:range            cim:BaseVoltage ;
        cims:AssociationUsed  "Yes" ;
        cims:inverseRoleName  cim:BaseVoltage.Fault ;
        cims:multiplicity     cims:M:0..1 ;
        cims:stereotype       "NC" .

cim:Fault.FaultyEquipment
        rdf:type              rdf:Property ;
        rdfs:comment          "Equipment carrying this fault." ;
        rdfs:domain           cim:Fault ;
        rdfs:label            "FaultyEquipment"@en ;
        rdfs:range            cim:Equipment ;
        cims:AssociationUsed  "Yes" ;
        cims:inverseRoleName  cim:Equipment.Faults ;
        cims:multiplicity     cims:M:1 .

cim:Fault.Location  rdf:type  rdf:Property ;
        rdfs:comment          "Location of this fault." ;
        rdfs:domain           cim:Fault ;
        rdfs:label            "Location"@en ;
        rdfs:range            cim:Location ;
        cims:AssociationUsed  "Yes" ;
        cims:inverseRoleName  cim:Location.Fault ;
        cims:multiplicity     cims:M:1 .

cim:Fault.kind  rdf:type   rdf:Property ;
        rdfs:comment       "The kind of phase fault." ;
        rdfs:domain        cim:Fault ;
        rdfs:label         "kind"@en ;
        rdfs:range         cim:PhaseConnectedFaultKind ;
        cims:multiplicity  cims:M:0..1 ;
        cims:stereotype    <http://iec.ch/TC57/NonStandard/UML#attribute> .

cim:Fault.occurredDateTime
        rdf:type           rdf:Property ;
        rdfs:comment       "The date and time at which the fault occurred." ;
        rdfs:domain        cim:Fault ;
        rdfs:label         "occurredDateTime"@en ;
        cims:dataType      cim:DateTime ;
        cims:multiplicity  cims:M:1..1 ;
        cims:stereotype    <http://iec.ch/TC57/NonStandard/UML#attribute> .

cim:Fault.phases  rdf:type  rdf:Property ;
        rdfs:comment       "The phases participating in the fault. The fault connections into these phases are further specified by the type of fault." ;
        rdfs:domain        cim:Fault ;
        rdfs:label         "phases"@en ;
        rdfs:range         cim:PhaseCode ;
        cims:multiplicity  cims:M:0..1 ;
        cims:stereotype    <http://iec.ch/TC57/NonStandard/UML#attribute> .

cim:FaultCauseType  rdf:type    rdfs:Class ;
        rdfs:comment            "Type of cause of the fault." ;
        rdfs:label              "FaultCauseType"@en ;
        rdfs:subClassOf         cim:IdentifiedObject ;
        cims:belongsToCategory  gd:Package_GridDisturbanceProfile ;
        cims:stereotype         <http://iec.ch/TC57/NonStandard/UML#concrete> .

cim:Float  rdf:type             rdfs:Class ;
        rdfs:comment            "A floating point number. The range is unspecified and not limited." ;
        rdfs:label              "Float"@en ;
        cims:belongsToCategory  gd:Package_GridDisturbanceProfile ;
        cims:stereotype         "Primitive" .

cim:IdentifiedObject  rdf:type  rdfs:Class ;
        rdfs:comment            "This is a root class to provide common identification for all classes needing identification and naming attributes." ;
        rdfs:label              "IdentifiedObject"@en ;
        cims:belongsToCategory  gd:Package_GridDisturbanceProfile .

cim:IdentifiedObject.description
        rdf:type           rdf:Property ;
        rdfs:comment       "The description is a free human readable text describing or naming the object. It may be non unique and may not correlate to a naming hierarchy." ;
        rdfs:domain        cim:IdentifiedObject ;
        rdfs:label         "description"@en ;
        cims:dataType      cim:String ;
        cims:multiplicity  cims:M:0..1 ;
        cims:stereotype    <http://iec.ch/TC57/NonStandard/UML#attribute> .

cim:IdentifiedObject.mRID
        rdf:type           rdf:Property ;
        rdfs:comment       "Master resource identifier issued by a model authority. The mRID is unique within an exchange context. Global uniqueness is easily achieved by using a UUID, as specified in RFC 4122, for the mRID. The use of UUID is strongly recommended.\nFor CIMXML data files in RDF syntax conforming to IEC 61970-552, the mRID is mapped to rdf:ID or rdf:about attributes that identify CIM object elements." ;
        rdfs:domain        cim:IdentifiedObject ;
        rdfs:label         "mRID"@en ;
        cims:dataType      cim:String ;
        cims:multiplicity  cims:M:1..1 ;
        cims:stereotype    <http://iec.ch/TC57/NonStandard/UML#attribute> .

cim:IdentifiedObject.name
        rdf:type           rdf:Property ;
        rdfs:comment       "The name is any free human readable and possibly non unique text naming the object." ;
        rdfs:domain        cim:IdentifiedObject ;
        rdfs:label         "name"@en ;
        cims:dataType      cim:String ;
        cims:multiplicity  cims:M:0..1 ;
        cims:stereotype    <http://iec.ch/TC57/NonStandard/UML#attribute> .

cim:Integer  rdf:type           rdfs:Class ;
        rdfs:comment            "An integer number. The range is unspecified and not limited." ;
        rdfs:label              "Integer"@en ;
        cims:belongsToCategory  gd:Package_GridDisturbanceProfile ;
        cims:stereotype         "Primitive" .

cim:Location  rdf:type          rdfs:Class ;
        rdfs:comment            "The place, scene, or point of something where someone or something has been, is, and/or will be at a given moment in time. It can be defined with one or more position points (coordinates) in a given coordinate system." ;
        rdfs:label              "Location"@en ;
        rdfs:subClassOf         cim:IdentifiedObject ;
        cims:belongsToCategory  gd:Package_GridDisturbanceProfile ;
        cims:stereotype         <http://iec.ch/TC57/NonStandard/UML#concrete> .

cim:Location.CoordinateSystem
        rdf:type              rdf:Property ;
        rdfs:comment          "Coordinate system used to describe position points of this location." ;
        rdfs:domain           cim:Location ;
        rdfs:label            "CoordinateSystem"@en ;
        rdfs:range            cim:CoordinateSystem ;
        cims:AssociationUsed  "Yes" ;
        cims:inverseRoleName  cim:CoordinateSystem.Locations ;
        cims:multiplicity     cims:M:1 .

cim:Location.Fault  rdf:type  rdf:Property ;
        rdfs:comment          "All faults at this location." ;
        rdfs:domain           cim:Location ;
        rdfs:label            "Fault"@en ;
        rdfs:range            cim:Fault ;
        cims:AssociationUsed  "No" ;
        cims:inverseRoleName  cim:Fault.Location ;
        cims:multiplicity     cims:M:0..n .

cim:Location.PositionPoints
        rdf:type              rdf:Property ;
        rdfs:comment          "Sequence of position points describing this location, expressed in coordinate system 'Location.CoordinateSystem'." ;
        rdfs:domain           cim:Location ;
        rdfs:label            "PositionPoints"@en ;
        rdfs:range            cim:PositionPoint ;
        cims:AssociationUsed  "No" ;
        cims:inverseRoleName  cim:PositionPoint.Location ;
        cims:multiplicity     cims:M:1..n .

cim:Outage  rdf:type            rdfs:Class ;
        rdfs:comment            "Document describing details of an active or planned outage in a part of the electrical network.\nA non-planned outage may be created upon:\n- a breaker trip,\n- a fault indicator status change,\n- a meter event indicating customer outage,\n- a reception of one or more customer trouble calls, or\n- an operator command, reflecting information obtained from the field crew.\nOutage restoration may be performed using a switching plan which complements the outage information with detailed switching activities, including the relationship to the crew and work.\nA planned outage may be created upon:\n- a request for service, maintenance or construction work in the field, or\n- an operator-defined outage for what-if/contingency network analysis." ;
        rdfs:label              "Outage"@en ;
        rdfs:subClassOf         cim:Document ;
        cims:belongsToCategory  gd:Package_GridDisturbanceProfile .

cim:Outage.Equipments
        rdf:type              rdf:Property ;
        rdfs:comment          "All equipments associated with this outage." ;
        rdfs:domain           cim:Outage ;
        rdfs:label            "Equipments"@en ;
        rdfs:range            cim:Equipment ;
        cims:AssociationUsed  "Yes" ;
        cims:inverseRoleName  cim:Equipment.Outages ;
        cims:multiplicity     cims:M:1 .

cim:PhaseCode  rdf:type         rdfs:Class ;
        rdfs:comment            "An unordered enumeration of phase identifiers.  Allows designation of phases for both transmission and distribution equipment, circuits and loads.   The enumeration, by itself, does not describe how the phases are connected together or connected to ground.  Ground is not explicitly denoted as a phase.\nResidential and small commercial loads are often served from single-phase, or split-phase, secondary circuits. For the example of s12N, phases 1 and 2 refer to hot wires that are 180 degrees out of phase, while N refers to the neutral wire. Through single-phase transformer connections, these secondary circuits may be served from one or two of the primary phases A, B, and C. For three-phase loads, use the A, B, C phase codes instead of s12N.\nThe integer values are from IEC 61968-9 to support revenue metering applications." ;
        rdfs:label              "PhaseCode"@en ;
        cims:belongsToCategory  gd:Package_GridDisturbanceProfile ;
        cims:stereotype         <http://iec.ch/TC57/NonStandard/UML#enumeration> .

cim:PhaseCode.A  rdf:type  cim:PhaseCode ;
        rdfs:comment     "Phase A." ;
        rdfs:label       "A"@en ;
        cims:stereotype  "enum" .

cim:PhaseCode.AB  rdf:type  cim:PhaseCode ;
        rdfs:comment     "Phases A and B." ;
        rdfs:label       "AB"@en ;
        cims:stereotype  "enum" .

cim:PhaseCode.ABC  rdf:type  cim:PhaseCode ;
        rdfs:comment     "Phases A, B, and C." ;
        rdfs:label       "ABC"@en ;
        cims:stereotype  "enum" .

cim:PhaseCode.ABCN  rdf:type  cim:PhaseCode ;
        rdfs:comment     "Phases A, B, C, and N." ;
        rdfs:label       "ABCN"@en ;
        cims:stereotype  "enum" .

cim:PhaseCode.ABN  rdf:type  cim:PhaseCode ;
        rdfs:comment     "Phases A, B, and neutral." ;
        rdfs:label       "ABN"@en ;
        cims:stereotype  "enum" .

cim:PhaseCode.AC  rdf:type  cim:PhaseCode ;
        rdfs:comment     "Phases A and C." ;
        rdfs:label       "AC"@en ;
        cims:stereotype  "enum" .

cim:PhaseCode.ACN  rdf:type  cim:PhaseCode ;
        rdfs:comment     "Phases A, C and neutral." ;
        rdfs:label       "ACN"@en ;
        cims:stereotype  "enum" .

cim:PhaseCode.AN  rdf:type  cim:PhaseCode ;
        rdfs:comment     "Phases A and neutral." ;
        rdfs:label       "AN"@en ;
        cims:stereotype  "enum" .

cim:PhaseCode.B  rdf:type  cim:PhaseCode ;
        rdfs:comment     "Phase B." ;
        rdfs:label       "B"@en ;
        cims:stereotype  "enum" .

cim:PhaseCode.BC  rdf:type  cim:PhaseCode ;
        rdfs:comment     "Phases B and C." ;
        rdfs:label       "BC"@en ;
        cims:stereotype  "enum" .

cim:PhaseCode.BCN  rdf:type  cim:PhaseCode ;
        rdfs:comment     "Phases B, C, and neutral." ;
        rdfs:label       "BCN"@en ;
        cims:stereotype  "enum" .

cim:PhaseCode.BN  rdf:type  cim:PhaseCode ;
        rdfs:comment     "Phases B and neutral." ;
        rdfs:label       "BN"@en ;
        cims:stereotype  "enum" .

cim:PhaseCode.C  rdf:type  cim:PhaseCode ;
        rdfs:comment     "Phase C." ;
        rdfs:label       "C"@en ;
        cims:stereotype  "enum" .

cim:PhaseCode.CN  rdf:type  cim:PhaseCode ;
        rdfs:comment     "Phases C and neutral." ;
        rdfs:label       "CN"@en ;
        cims:stereotype  "enum" .

cim:PhaseCode.N  rdf:type  cim:PhaseCode ;
        rdfs:comment     "Neutral phase." ;
        rdfs:label       "N"@en ;
        cims:stereotype  "enum" .

cim:PhaseCode.X  rdf:type  cim:PhaseCode ;
        rdfs:comment     "Unknown non-neutral phase." ;
        rdfs:label       "X"@en ;
        cims:stereotype  "enum" .

cim:PhaseCode.XN  rdf:type  cim:PhaseCode ;
        rdfs:comment     "Unknown non-neutral phase plus neutral." ;
        rdfs:label       "XN"@en ;
        cims:stereotype  "enum" .

cim:PhaseCode.XY  rdf:type  cim:PhaseCode ;
        rdfs:comment     "Two unknown non-neutral phases." ;
        rdfs:label       "XY"@en ;
        cims:stereotype  "enum" .

cim:PhaseCode.XYN  rdf:type  cim:PhaseCode ;
        rdfs:comment     "Two unknown non-neutral phases plus neutral." ;
        rdfs:label       "XYN"@en ;
        cims:stereotype  "enum" .

cim:PhaseCode.none  rdf:type  cim:PhaseCode ;
        rdfs:comment     "No phases specified." ;
        rdfs:label       "none"@en ;
        cims:stereotype  "enum" .

cim:PhaseCode.s1  rdf:type  cim:PhaseCode ;
        rdfs:comment     "Secondary phase 1." ;
        rdfs:label       "s1"@en ;
        cims:stereotype  "enum" .

cim:PhaseCode.s12  rdf:type  cim:PhaseCode ;
        rdfs:comment     "Secondary phase 1 and 2." ;
        rdfs:label       "s12"@en ;
        cims:stereotype  "enum" .

cim:PhaseCode.s12N  rdf:type  cim:PhaseCode ;
        rdfs:comment     "Secondary phases 1, 2, and neutral." ;
        rdfs:label       "s12N"@en ;
        cims:stereotype  "enum" .

cim:PhaseCode.s1N  rdf:type  cim:PhaseCode ;
        rdfs:comment     "Secondary phase 1 and neutral." ;
        rdfs:label       "s1N"@en ;
        cims:stereotype  "enum" .

cim:PhaseCode.s2  rdf:type  cim:PhaseCode ;
        rdfs:comment     "Secondary phase 2." ;
        rdfs:label       "s2"@en ;
        cims:stereotype  "enum" .

cim:PhaseCode.s2N  rdf:type  cim:PhaseCode ;
        rdfs:comment     "Secondary phase 2 and neutral." ;
        rdfs:label       "s2N"@en ;
        cims:stereotype  "enum" .

cim:PhaseConnectedFaultKind
        rdf:type                rdfs:Class ;
        rdfs:comment            "The type of fault connection among phases." ;
        rdfs:label              "PhaseConnectedFaultKind"@en ;
        cims:belongsToCategory  gd:Package_GridDisturbanceProfile ;
        cims:stereotype         <http://iec.ch/TC57/NonStandard/UML#enumeration> .

cim:PhaseConnectedFaultKind.lineOpen
        rdf:type         cim:PhaseConnectedFaultKind ;
        rdfs:comment     "The fault is when the conductor path is broken between two terminals. Additional coexisting faults may be required if the broken conductor also causes connections to grounds or other lines or phases." ;
        rdfs:label       "lineOpen"@en ;
        cims:stereotype  "enum" .

cim:PhaseConnectedFaultKind.lineToGround
        rdf:type         cim:PhaseConnectedFaultKind ;
        rdfs:comment     "The fault connects the indicated phases to ground. The line to line fault impedance is not used and assumed infinite. The full ground impedance is connected between each phase specified in the fault and ground, but not between the phases." ;
        rdfs:label       "lineToGround"@en ;
        cims:stereotype  "enum" .

cim:PhaseConnectedFaultKind.lineToLine
        rdf:type         cim:PhaseConnectedFaultKind ;
        rdfs:comment     "The fault connects the specified phases together without a connection to ground. The ground impedance of this fault is ignored. The line to line impedance is connected between each of the phases specified in the fault. For example three times for a three phase fault, one time for a two phase fault.  A single phase fault should not be specified." ;
        rdfs:label       "lineToLine"@en ;
        cims:stereotype  "enum" .

cim:PhaseConnectedFaultKind.lineToLineToGround
        rdf:type         cim:PhaseConnectedFaultKind ;
        rdfs:comment     "The fault connects the indicated phases to ground and to each other. The line to line impedance is connected between each of the phases specified in the fault in a full mesh. For example three times for a three phase fault, one time for a two phase fault. A single phase fault should not be specified. The full ground impedance is connected between each phase specified in the fault and ground." ;
        rdfs:label       "lineToLineToGround"@en ;
        cims:stereotype  "enum" .

cim:PositionPoint  rdf:type     rdfs:Class ;
        rdfs:comment            "Set of spatial coordinates that determine a point, defined in the coordinate system specified in 'Location.CoordinateSystem'. Use a single position point instance to describe a point-oriented location. Use a sequence of position points to describe a line-oriented object (physical location of non-point oriented objects like cables or lines), or area of an object (like a substation or a geographical zone - in this case, have first and last position point with the same values)." ;
        rdfs:label              "PositionPoint"@en ;
        cims:belongsToCategory  gd:Package_GridDisturbanceProfile ;
        cims:stereotype         <http://iec.ch/TC57/NonStandard/UML#concrete> .
cim:PositionPoint.Location
        rdf:type              rdf:Property ;
        rdfs:comment          "Location described by this position point." ;
        rdfs:domain           cim:PositionPoint ;
        rdfs:label            "Location"@en ;
        rdfs:range            cim:Location ;
        cims:AssociationUsed  "Yes" ;
        cims:inverseRoleName  cim:Location.PositionPoints ;
        cims:multiplicity     cims:M:1 .

cim:PositionPoint.xPosition
        rdf:type           rdf:Property ;
        rdfs:comment       "X axis position." ;
        rdfs:domain        cim:PositionPoint ;
        rdfs:label         "xPosition"@en ;
        cims:dataType      cim:String ;
        cims:multiplicity  cims:M:1..1 ;
        cims:stereotype    <http://iec.ch/TC57/NonStandard/UML#attribute> .

cim:PositionPoint.yPosition
        rdf:type           rdf:Property ;
        rdfs:comment       "Y axis position." ;
        rdfs:domain        cim:PositionPoint ;
        rdfs:label         "yPosition"@en ;
        cims:dataType      cim:String ;
        cims:multiplicity  cims:M:1..1 ;
        cims:stereotype    <http://iec.ch/TC57/NonStandard/UML#attribute> .

cim:PositionPoint.zPosition
        rdf:type           rdf:Property ;
        rdfs:comment       "(if applicable) Z axis position." ;
        rdfs:domain        cim:PositionPoint ;
        rdfs:label         "zPosition"@en ;
        cims:dataType      cim:String ;
        cims:multiplicity  cims:M:0..1 ;
        cims:stereotype    <http://iec.ch/TC57/NonStandard/UML#attribute> .

cim:RealEnergy  rdf:type        rdfs:Class ;
        rdfs:comment            "Real electrical energy." ;
        rdfs:label              "RealEnergy"@en ;
        cims:belongsToCategory  gd:Package_GridDisturbanceProfile ;
        cims:stereotype         "CIMDatatype" .

cim:RealEnergy.multiplier
        rdf:type           rdf:Property ;
        rdfs:domain        cim:RealEnergy ;
        rdfs:label         "multiplier"@en ;
        rdfs:range         cim:UnitMultiplier ;
        cims:multiplicity  cims:M:0..1 ;
        cims:stereotype    <http://iec.ch/TC57/NonStandard/UML#attribute> .

cim:RealEnergy.unit  rdf:type  rdf:Property ;
        rdfs:domain        cim:RealEnergy ;
        rdfs:label         "unit"@en ;
        rdfs:range         cim:UnitSymbol ;
        cims:isFixed       "Wh" ;
        cims:multiplicity  cims:M:0..1 ;
        cims:stereotype    <http://iec.ch/TC57/NonStandard/UML#attribute> .

cim:RealEnergy.value  rdf:type  rdf:Property ;
        rdfs:domain        cim:RealEnergy ;
        rdfs:label         "value"@en ;
        cims:dataType      cim:Float ;
        cims:multiplicity  cims:M:0..1 ;
        cims:stereotype    <http://iec.ch/TC57/NonStandard/UML#attribute> .

cim:String  rdf:type            rdfs:Class ;
        rdfs:comment            "A string consisting of a sequence of characters. The character encoding is UTF-8. The string length is unspecified and unlimited." ;
        rdfs:label              "String"@en ;
        cims:belongsToCategory  gd:Package_GridDisturbanceProfile ;
        cims:stereotype         "Primitive" .

cim:UnitMultiplier  rdf:type    rdfs:Class ;
        rdfs:comment            "The unit multipliers defined for the CIM.  When applied to unit symbols, the unit symbol is treated as a derived unit. Regardless of the contents of the unit symbol text, the unit symbol shall be treated as if it were a single-character unit symbol. Unit symbols should not contain multipliers, and it should be left to the multiplier to define the multiple for an entire data type. \n\nFor example, if a unit symbol is \"m2Pers\" and the multiplier is \"k\", then the value is k(m**2/s), and the multiplier applies to the entire final value, not to any individual part of the value. This can be conceptualized by substituting a derived unit symbol for the unit type. If one imagines that the symbol \"Þ\" represents the derived unit \"m2Pers\", then applying the multiplier \"k\" can be conceptualized simply as \"kÞ\".\n\nFor example, the SI unit for mass is \"kg\" and not \"g\".  If the unit symbol is defined as \"kg\", then the multiplier is applied to \"kg\" as a whole and does not replace the \"k\" in front of the \"g\". In this case, the multiplier of \"m\" would be used with the unit symbol of \"kg\" to represent one gram.  As a text string, this violates the instructions in IEC 80000-1. However, because the unit symbol in CIM is treated as a derived unit instead of as an SI unit, it makes more sense to conceptualize the \"kg\" as if it were replaced by one of the proposed replacements for the SI mass symbol. If one imagines that the \"kg\" were replaced by a symbol \"Þ\", then it is easier to conceptualize the multiplier \"m\" as creating the proper unit \"mÞ\", and not the forbidden unit \"mkg\"." ;
        rdfs:label              "UnitMultiplier"@en ;
        cims:belongsToCategory  gd:Package_GridDisturbanceProfile ;
        cims:stereotype         <http://iec.ch/TC57/NonStandard/UML#enumeration> .

cim:UnitMultiplier.M  rdf:type  cim:UnitMultiplier ;
        rdfs:comment     "Mega 10**6." ;
        rdfs:label       "M"@en ;
        cims:stereotype  "enum" .

cim:UnitMultiplier.k  rdf:type  cim:UnitMultiplier ;
        rdfs:comment     "Kilo 10**3." ;
        rdfs:label       "k"@en ;
        cims:stereotype  "enum" .

cim:UnitSymbol  rdf:type        rdfs:Class ;
        rdfs:comment            "The derived units defined for usage in the CIM. In some cases, the derived unit is equal to an SI unit. Whenever possible, the standard derived symbol is used instead of the formula for the derived unit. For example, the unit symbol Farad is defined as \"F\" instead of \"CPerV\". In cases where a standard symbol does not exist for a derived unit, the formula for the unit is used as the unit symbol. For example, density does not have a standard symbol and so it is represented as \"kgPerm3\". With the exception of the \"kg\", which is an SI unit, the unit symbols do not contain multipliers and therefore represent the base derived unit to which a multiplier can be applied as a whole. \nEvery unit symbol is treated as an unparseable text as if it were a single-letter symbol. The meaning of each unit symbol is defined by the accompanying descriptive text and not by the text contents of the unit symbol.\nTo allow the widest possible range of serializations without requiring special character handling, several substitutions are made which deviate from the format described in IEC 80000-1. The division symbol \"/\" is replaced by the letters \"Per\". Exponents are written in plain text after the unit as \"m3\" instead of being formatted as \"m\" with a superscript of 3  or introducing a symbol as in \"m^3\". The degree symbol \"°\" is replaced with the letters \"deg\". Any clarification of the meaning for a substitution is included in the description for the unit symbol.\nNon-SI units are included in list of unit symbols to allow sources of data to be correctly labelled with their non-SI units (for example, a GPS sensor that is reporting numbers that represent feet instead of meters). This allows software to use the unit symbol information correctly convert and scale the raw data of those sources into SI-based units. \nThe integer values are used for harmonization with IEC 61850." ;
        rdfs:label              "UnitSymbol"@en ;
        cims:belongsToCategory  gd:Package_GridDisturbanceProfile ;
        cims:stereotype         <http://iec.ch/TC57/NonStandard/UML#enumeration> .

cim:UnitSymbol.W  rdf:type  cim:UnitSymbol ;
        rdfs:comment     "Real power in watts (J/s). Electrical power may have real and reactive components. The real portion of electrical power (I&#178;R or VIcos(phi)), is expressed in Watts. See also apparent power and reactive power." ;
        rdfs:label       "W"@en ;
        cims:stereotype  "enum" .

cim:UnitSymbol.Wh  rdf:type  cim:UnitSymbol ;
        rdfs:comment     "Real energy in watt hours." ;
        rdfs:label       "Wh"@en ;
        cims:stereotype  "enum" .

cim:UnplannedOutage  rdf:type   rdfs:Class ;
        rdfs:comment            "Document describing the consequence of an unplanned outage in a part of the electrical network. For the purposes of this model, an unplanned outage refers to a state where energy is not delivered; such as, customers out of service, a street light is not served, etc.\nA unplanned outage may be created upon:\n- impacts the SAIDI calculation\n- a breaker trip,\n- a fault indicator status change,\n- a meter event indicating customer outage,\n- a reception of one or more customer trouble calls, or\n- an operator command, reflecting information obtained from the field crew.\nOutage restoration may be performed using a switching plan which complements the outage information with detailed switching activities, including the relationship to the crew and work." ;
        rdfs:label              "UnplannedOutage"@en ;
        rdfs:subClassOf         cim:Outage ;
        cims:belongsToCategory  gd:Package_GridDisturbanceProfile ;
        cims:stereotype         <http://iec.ch/TC57/NonStandard/UML#concrete> .

cim:UnplannedOutage.TrippedEquipment
        rdf:type              rdf:Property ;
        rdfs:comment          "The equipment that tripped during the outage." ;
        rdfs:domain           cim:UnplannedOutage ;
        rdfs:label            "TrippedEquipment"@en ;
        rdfs:range            cim:Equipment ;
        cims:AssociationUsed  "No" ;
        cims:inverseRoleName  cim:Equipment.UnplannedOutage ;
        cims:multiplicity     cims:M:1..n ;
        cims:stereotype       "NC" .

cim:UnplannedOutage.reportedStartTime
        rdf:type           rdf:Property ;
        rdfs:comment       "The earliest start time of the Outage - as reported by some system or individual" ;
        rdfs:domain        cim:UnplannedOutage ;
        rdfs:label         "reportedStartTime"@en ;
        cims:dataType      cim:DateTime ;
        cims:multiplicity  cims:M:0..1 ;
        cims:stereotype    <http://iec.ch/TC57/NonStandard/UML#attribute> .

gd:Ontology  rdf:type         owl:Ontology ;
        dcterms:conformsTo    "urn:iso:std:iec:61970-501:draft:ed-2" , "urn:iso:std:iec:61970-301:ed-7:amd1" , "file://CIM100_CGMES31v01_501-20v02_NC23v62_MM10v01.eap" , "file://iec61970cim17v40_iec61968cim13v13a_iec62325cim03v17a.eap" , "urn:iso:std:iec:61970-600-2:ed-1" , "urn:iso:std:iec:61970-401:draft:ed-1" ;
        dcterms:creator       "ENTSO-E CIM WG PRA project "@en ;
        dcterms:description   "This vocabulary is describing the grid disturbance profile."@en ;
        dcterms:identifier    "urn:uuid:81c488d7-a09f-49ef-a3cd-3bb19a1d6f16" ;
        dcterms:language      "en-GB" ;
        dcterms:license       "https://www.apache.org/licenses/LICENSE-2.0"@en ;
        dcterms:modified      "2024-04-08"^^<http://www.w3.org/2001/XMLSchema#date> ;
        dcterms:publisher     "ENTSO-E"@en ;
        dcterms:rightsHolder  "ENTSO-E"@en ;
        dcterms:title         "Grid Disturbance vocabulary"@en ;
        owl:versionIRI        <https://ap.cim4.eu/GridDisturbance/1.1> ;
        owl:versionInfo       "1.1.0"@en ;
        dcat:keyword          "GD" ;
        dcat:theme            "vocabulary"@en .

gd:Package_DocGridDisturbanceProfile
        rdf:type      cims:ClassCategory ;
        rdfs:comment  "This package contains datatypes used only in the RDFS header." ;
        rdfs:label    "DocGridDisturbanceProfile"@en .

gd:Package_GridDisturbanceProfile
        rdf:type      cims:ClassCategory ;
        rdfs:comment  "This package contains the grid disturbance profile." ;
        rdfs:label    "GridDisturbanceProfile"@en .

nc:AutoReclosingKind  rdf:type  rdfs:Class ;
        rdfs:comment            "The type of autoreclosing that occurred with the trip.\n\nIf high-speed automatic reclosing is successful at one end of a line, but the line needs to be reclosed manually at the other end, choose manual reclosing.\n\nIn this document, high-speed automatic reclosing refers to automatic reclosing after less than 2 seconds." ;
        rdfs:label              "AutoReclosingKind"@en ;
        cims:belongsToCategory  gd:Package_GridDisturbanceProfile ;
        cims:stereotype         "NC" ;
        cims:stereotype         <http://iec.ch/TC57/NonStandard/UML#enumeration> .

nc:AutoReclosingKind.automaticallyAfter2SecondsOrMore
        rdf:type         nc:AutoReclosingKind ;
        rdfs:comment     "If the automatic reclosing was successful in 2 seconds or more.\n\nAlso known as \"successful high-speed reclosing\"." ;
        rdfs:label       "automaticallyAfter2SecondsOrMore"@en ;
        cims:stereotype  "enum" .

nc:AutoReclosingKind.automaticallyAfterLessThan2Seconds
        rdf:type         nc:AutoReclosingKind ;
        rdfs:comment     "If the automatic reclosing was successful in 2 seconds or less.\n\nAlso known as \"successful high-speed reclosing\"." ;
        rdfs:label       "automaticallyAfterLessThan2Seconds"@en ;
        cims:stereotype  "enum" .

nc:AutoReclosingKind.manuallyAfterInspection
        rdf:type         nc:AutoReclosingKind ;
        rdfs:comment     "If the reclosing was done manually after inspection of the component." ;
        rdfs:label       "manuallyAfterInspection"@en ;
        cims:stereotype  "enum" .

nc:AutoReclosingKind.manuallyAfterRepair
        rdf:type         nc:AutoReclosingKind ;
        rdfs:comment     "If the reclosing was done manually after repair." ;
        rdfs:label       "manuallyAfterRepair"@en ;
        cims:stereotype  "enum" .

nc:AutoReclosingKind.manuallyAfterRestructuringOfOperations
        rdf:type         nc:AutoReclosingKind ;
        rdfs:comment     "If the reclosing was done manually after restructuring of operations." ;
        rdfs:label       "manuallyAfterRestructuringOfOperations"@en ;
        cims:stereotype  "enum" .

nc:AutoReclosingKind.manuallyWithoutEitherInspectionRepairOrRestructuringOfOperations
        rdf:type         nc:AutoReclosingKind ;
        rdfs:comment     "If the reclosing was done manually without any inspections, repairs or restructurings of operations." ;
        rdfs:label       "manuallyWithoutEitherInspectionRepairOrRestructuringOfOperations"@en ;
        cims:stereotype  "enum" .

nc:AutoReclosingKind.other
        rdf:type         nc:AutoReclosingKind ;
        rdfs:comment     "If the type of auto-reclosing is not unknown but does not fit the other categories, report it as other." ;
        rdfs:label       "other"@en ;
        cims:stereotype  "enum" .

nc:AutoReclosingKind.unknown
        rdf:type         nc:AutoReclosingKind ;
        rdfs:comment     "If the type of auto-reclosing is unknown." ;
        rdfs:label       "unknown"@en ;
        cims:stereotype  "enum" .

nc:CertaintyLevelKind
        rdf:type                rdfs:Class ;
        rdfs:comment            "High certainty level is used when the cause of a fault is 100 % certain or when the cause is the most probable cause and potentially determined by an expert. " ;
        rdfs:label              "CertaintyLevelKind"@en ;
        cims:belongsToCategory  gd:Package_GridDisturbanceProfile ;
        cims:stereotype         "NC" ;
        cims:stereotype         <http://iec.ch/TC57/NonStandard/UML#enumeration> .

nc:CertaintyLevelKind.high
        rdf:type         nc:CertaintyLevelKind ;
        rdfs:comment     "The certainty level is high." ;
        rdfs:label       "high"@en ;
        cims:stereotype  "enum" .

nc:CertaintyLevelKind.low
        rdf:type         nc:CertaintyLevelKind ;
        rdfs:comment     "The certainty level is low." ;
        rdfs:label       "low"@en ;
        cims:stereotype  "enum" .

nc:CertaintyLevelKind.medium
        rdf:type         nc:CertaintyLevelKind ;
        rdfs:comment     "The certainty level is medium." ;
        rdfs:label       "medium"@en ;
        cims:stereotype  "enum" .

nc:CertaintyLevelKind.none
        rdf:type         nc:CertaintyLevelKind ;
        rdfs:comment     "The certainty level is none." ;
        rdfs:label       "none"@en ;
        cims:stereotype  "enum" .

nc:Equipment.Interruption
        rdf:type              rdf:Property ;
        rdfs:comment          "The interruption that belongs to the interrupted delivery equipment." ;
        rdfs:domain           cim:Equipment ;
        rdfs:label            "Interruption"@en ;
        rdfs:range            nc:Interruption ;
        cims:AssociationUsed  "No" ;
        cims:inverseRoleName  nc:Interruption.InterruptedDeliveryEquipment ;
        cims:multiplicity     cims:M:0..1 ;
        cims:stereotype       "NC" .

nc:Fault.FaultCause  rdf:type  rdf:Property ;
        rdfs:comment          "The fault and cause combination to be simulated for this fault." ;
        rdfs:domain           cim:Fault ;
        rdfs:label            "FaultCause"@en ;
        rdfs:range            nc:FaultCause ;
        cims:AssociationUsed  "No" ;
        cims:inverseRoleName  nc:FaultCause.Fault ;
        cims:multiplicity     cims:M:1..n ;
        cims:stereotype       "NC" ;
        cims:stereotype       <http://iec.ch/TC57/NonStandard/UML#ofAggregate> .

nc:Fault.FaultOutage  rdf:type  rdf:Property ;
        rdfs:comment          "The combination of a fault and an outage to be simulated for this fault." ;
        rdfs:domain           cim:Fault ;
        rdfs:label            "FaultOutage"@en ;
        rdfs:range            nc:FaultOutage ;
        cims:AssociationUsed  "No" ;
        cims:inverseRoleName  nc:FaultOutage.Fault ;
        cims:multiplicity     cims:M:0..n ;
        cims:stereotype       "NC" .

nc:Fault.GridDisturbance
        rdf:type              rdf:Property ;
        rdfs:comment          "A grid disturbance to contain all faults." ;
        rdfs:domain           cim:Fault ;
        rdfs:label            "GridDisturbance"@en ;
        rdfs:range            nc:GridDisturbance ;
        cims:AssociationUsed  "Yes" ;
        cims:inverseRoleName  nc:GridDisturbance.Fault ;
        cims:multiplicity     cims:M:0..1 ;
        cims:stereotype       "NC" .

nc:Fault.SystemOperator
        rdf:type              rdf:Property ;
        rdfs:comment          "The system operator in whose control area this fault occurred." ;
        rdfs:domain           cim:Fault ;
        rdfs:label            "SystemOperator"@en ;
        rdfs:range            nc:SystemOperator ;
        cims:AssociationUsed  "Yes" ;
        cims:inverseRoleName  nc:SystemOperator.Fault ;
        cims:multiplicity     cims:M:0..1 ;
        cims:stereotype       "NC" .

nc:Fault.category  rdf:type  rdf:Property ;
        rdfs:comment       "The fault category." ;
        rdfs:domain        cim:Fault ;
        rdfs:label         "category"@en ;
        rdfs:range         nc:FaultCategoryKind ;
        cims:multiplicity  cims:M:1..1 ;
        cims:stereotype    "NC" ;
        cims:stereotype    <http://iec.ch/TC57/NonStandard/UML#attribute> .

nc:Fault.duration  rdf:type  rdf:Property ;
        rdfs:comment       "The duration of the fault." ;
        rdfs:domain        cim:Fault ;
        rdfs:label         "duration"@en ;
        cims:dataType      cim:Duration ;
        cims:multiplicity  cims:M:1..1 ;
        cims:stereotype    "NC" ;
        cims:stereotype    <http://iec.ch/TC57/NonStandard/UML#attribute> .

nc:Fault.faultKind  rdf:type  rdf:Property ;
        rdfs:comment       "One fault can consist of several fault types. If a fault consists of several fault types, the most significant fault type is used.\n\nIn case of developing faults, that is in faults changing from one type to another, the final type is given." ;
        rdfs:domain        cim:Fault ;
        rdfs:label         "faultKind"@en ;
        rdfs:range         nc:FaultKind ;
        cims:multiplicity  cims:M:1..1 ;
        cims:stereotype    "NC" ;
        cims:stereotype    <http://iec.ch/TC57/NonStandard/UML#attribute> .

nc:Fault.isDirectlyEarthed
        rdf:type           rdf:Property ;
        rdfs:comment       "Whether the power system is directly earthed (true) or compensated (false). \nUsually optional for faults on units with reactive compensation with voltages lower than 100 kV." ;
        rdfs:domain        cim:Fault ;
        rdfs:label         "isDirectlyEarthed"@en ;
        cims:dataType      cim:Boolean ;
        cims:multiplicity  cims:M:1..1 ;
        cims:stereotype    "NC" ;
        cims:stereotype    <http://iec.ch/TC57/NonStandard/UML#attribute> .

nc:Fault.isIntermittent
        rdf:type           rdf:Property ;
        rdfs:comment       "The kind of occurrence of the fault. It is either intermittent (true) or non-intermittent (false).\nAn intermittent fault is a recurring fault in the same unit and in the same place and for the same reason which repeats itself before it becomes necessary to carry out any repairs or eliminate the cause [8].\nA non-intermittent fault occurs only once.\n\nNote 1: a fault which repeats itself after an inspection, which did not result in the fault being pinpointed or repaired, is not considered an intermittent fault. A fault like this is considered as the beginning of a grid disturbance every time the fault occurs.\nNote 2: one example of an intermittent fault is galloping lines.\nNote 3: when deciding whether a fault is intermittent or not, one should consider more of the cause, location and consequence of the fault and not on the time between the faults. An intermittent fault is counted as one fault. However, all individual caused outages are connected to this fault.\nNote 4: there is no standard for the required timespan between intermittent faults. Some system operators use 2 hours." ;
        rdfs:domain        cim:Fault ;
        rdfs:label         "isIntermittent"@en ;
        cims:dataType      cim:Boolean ;
        cims:multiplicity  cims:M:1..1 ;
        cims:stereotype    "NC" ;
        cims:stereotype    <http://iec.ch/TC57/NonStandard/UML#attribute> .

nc:Fault.isPermanent  rdf:type  rdf:Property ;
        rdfs:comment       "Whether the fault is a permanent (true) or a temporary (false) fault.\nA permanent fault is a fault that will remain unless it is removed by some intervention.\nNote 1 to entry: The “intervention” may be modification or maintenance.\nNote 2: a permanent fault requires repair or adjustment before the unit is ready for operation. For example, the resetting of computers is considered as repair work and a switch in the wrong position is considered as a permanent fault. Signal acknowledgement is not considered as repair work. \nNote 3: the duration of the disconnection is irrelevant when determining if a fault is permanent or not.\n\nA temporary fault is a fault where the unit or component is undamaged and is restored to service by switching operations without repair but possibly with on-site inspection.  \nNote 1: a temporary fault does not require measures other than the reconnection of circuit breakers, replacement of fuses or signal acknowledgement.\nNote 2: the duration of the disconnection is irrelevant when determining if a fault is temporary or not. If, for example, a fault results in long-term disconnection and (on-site) inspection cannot pinpoint its source, the fault is considered to be temporary as no repairs are carried out." ;
        rdfs:domain        cim:Fault ;
        rdfs:label         "isPermanent"@en ;
        cims:dataType      cim:Boolean ;
        cims:multiplicity  cims:M:1..1 ;
        cims:stereotype    "NC" ;
        cims:stereotype    <http://iec.ch/TC57/NonStandard/UML#attribute> .

nc:Fault.repairTime  rdf:type  rdf:Property ;
        rdfs:comment       "Time from when repair commences, including necessary troubleshooting, until the unit’s function(s) has (have) been resumed and the unit is ready for operation.\n\nNote 1: repair time is registered only for permanent faults and does not include administrative delays (voluntary waiting time). However, any preparations necessary to carry out repairs, for example the collection or ordering of spare parts, waiting for spare parts or transport, are included in the repair time. \n\nNote 2: the repair time is zero if a fault is left unrepaired deliberately.\n\nNote 3: this definition differs from the IEC 192-07-19 definition by also including the preparation time necessary to carry out the repairs mentioned in note 1." ;
        rdfs:domain        cim:Fault ;
        rdfs:label         "repairTime"@en ;
        cims:dataType      cim:Duration ;
        cims:multiplicity  cims:M:0..1 ;
        cims:stereotype    "NC" ;
        cims:stereotype    <http://iec.ch/TC57/NonStandard/UML#attribute> .

nc:Fault.sequenceNumber
        rdf:type           rdf:Property ;
        rdfs:comment       "A chronological serial number indicating the order of the faults related to the grid disturbance. \n\nPrimary faults have fault ID “1”, and secondary/latent faults have fault ID “2” or more." ;
        rdfs:domain        cim:Fault ;
        rdfs:label         "sequenceNumber"@en ;
        cims:dataType      cim:Integer ;
        cims:multiplicity  cims:M:1..1 ;
        cims:stereotype    "NC" ;
        cims:stereotype    <http://iec.ch/TC57/NonStandard/UML#attribute> .

nc:FaultCategoryKind  rdf:type  rdfs:Class ;
        rdfs:comment            "Available kinds of fault categories." ;
        rdfs:label              "FaultCategoryKind"@en ;
        cims:belongsToCategory  gd:Package_GridDisturbanceProfile ;
        cims:stereotype         "NC" ;
        cims:stereotype         <http://iec.ch/TC57/NonStandard/UML#enumeration> .

nc:FaultCategoryKind.operational
        rdf:type         nc:FaultCategoryKind ;
        rdfs:comment     "A fault due to a temporary human error.\n\nNote 1: incorrect operation is considered a fault in a component, or in other words, the incorrect operation is attributed to the unit which has been operated incorrectly." ;
        rdfs:label       "operational"@en ;
        cims:stereotype  "enum" .

nc:FaultCategoryKind.system
        rdf:type         nc:FaultCategoryKind ;
        rdfs:comment     "A fault due to off-nominal parameters, exceeding of regulated norms and standards, or exceeding protection limits.\n\nNote 1: Typical examples of system fault causes are high/low frequency, power oscillations, overload, overvoltage, undervoltage or high harmonic content in voltage or current. Common causes for system faults are significant changes in load or generation and switching of lines or transformers with following change of load flow." ;
        rdfs:label       "system"@en ;
        cims:stereotype  "enum" .

nc:FaultCategoryKind.technical
        rdf:type         nc:FaultCategoryKind ;
        rdfs:comment     "A fault due to a technical error." ;
        rdfs:label       "technical"@en ;
        cims:stereotype  "enum" .

nc:FaultCause  rdf:type         rdfs:Class ;
        rdfs:comment            "Fault cause." ;
        rdfs:label              "FaultCause"@en ;
        cims:belongsToCategory  gd:Package_GridDisturbanceProfile ;
        cims:stereotype         "NC" ;
        cims:stereotype         <http://iec.ch/TC57/NonStandard/UML#concrete> .

nc:FaultCause.Fault  rdf:type  rdf:Property ;
        rdfs:comment          "The fault defined for this fault and cause combination." ;
        rdfs:domain           nc:FaultCause ;
        rdfs:label            "Fault"@en ;
        rdfs:range            cim:Fault ;
        cims:AssociationUsed  "Yes" ;
        cims:inverseRoleName  nc:Fault.FaultCause ;
        cims:multiplicity     cims:M:1 ;
        cims:stereotype       "NC" .

nc:FaultCause.FaultCauseType
        rdf:type              rdf:Property ;
        rdfs:comment          "The fault and cause combination to be simulated for this cause." ;
        rdfs:domain           nc:FaultCause ;
        rdfs:label            "FaultCauseType"@en ;
        rdfs:range            cim:FaultCauseType ;
        cims:AssociationUsed  "Yes" ;
        cims:inverseRoleName  nc:FaultCauseType.FaultCause ;
        cims:multiplicity     cims:M:1 ;
        cims:stereotype       "NC" .

nc:FaultCause.certaintyLevel
        rdf:type           rdf:Property ;
        rdfs:comment       "The degree of certainty of which the cause of a fault is determined by a user. \nNote 1: the used certainty levels are low, medium and high. High certainty level is used when the cause of a fault is 100 % certain or when the cause is the most probable cause and potentially determined by an expert. Medium certainty level is used when the cause of the fault is very probable but there is not enough evidence to fully support the claim. Low certainty level is used when there is some idea of what the cause could be with the help of, for example, the fault details or expert knowledge. \nNote 2: the fault cause ‘unknown’ is used if no other fault cause can be chosen by any degree of certainty. " ;
        rdfs:domain        nc:FaultCause ;
        rdfs:label         "certaintyLevel"@en ;
        rdfs:range         nc:CertaintyLevelKind ;
        cims:multiplicity  cims:M:1..1 ;
        cims:stereotype    "NC" ;
        cims:stereotype    <http://iec.ch/TC57/NonStandard/UML#attribute> .

nc:FaultCause.mRID  rdf:type  rdf:Property ;
        rdfs:comment       "Master resource identifier issued by a model authority. The mRID is unique within an exchange context. Global uniqueness is easily achieved by using a UUID, as specified in RFC 4122, for the mRID. The use of UUID is strongly recommended.\nFor CIMXML data files in RDF syntax conforming to IEC 61970-552, the mRID is mapped to rdf:ID or rdf:about attributes that identify CIM object elements." ;
        rdfs:domain        nc:FaultCause ;
        rdfs:label         "mRID"@en ;
        cims:dataType      cim:String ;
        cims:multiplicity  cims:M:1..1 ;
        cims:stereotype    "NC" ;
        cims:stereotype    <http://iec.ch/TC57/NonStandard/UML#attribute> .

nc:FaultCauseType.FaultCause
        rdf:type              rdf:Property ;
        rdfs:comment          "The fault cause defined for this fault and cause combination." ;
        rdfs:domain           cim:FaultCauseType ;
        rdfs:label            "FaultCause"@en ;
        rdfs:range            nc:FaultCause ;
        cims:AssociationUsed  "No" ;
        cims:inverseRoleName  nc:FaultCause.FaultCauseType ;
        cims:multiplicity     cims:M:0..n ;
        cims:stereotype       "NC" .

nc:FaultKind  rdf:type          rdfs:Class ;
        rdfs:comment            "One fault can consist of several fault types. If a fault consists of several fault types, the most significant fault type is used.\n\nIn case of developing faults, that is in faults changing from one type to another, the final type is given." ;
        rdfs:label              "FaultKind"@en ;
        cims:belongsToCategory  gd:Package_GridDisturbanceProfile ;
        cims:stereotype         "NC" ;
        cims:stereotype         <http://iec.ch/TC57/NonStandard/UML#enumeration> .

nc:FaultKind.functional
        rdf:type         nc:FaultKind ;
        rdfs:comment     "The components main function failed to occur." ;
        rdfs:label       "functional"@en ;
        cims:stereotype  "enum" .

nc:FaultKind.lineOpen
        rdf:type         nc:FaultKind ;
        rdfs:comment     "The fault is when the conductor path is broken between two terminals. Additional coexisting faults may be required if the broken conductor also causes connections to grounds or other lines or phases." ;
        rdfs:label       "lineOpen"@en ;
        cims:stereotype  "enum" .

nc:FaultKind.lineToGround
        rdf:type         nc:FaultKind ;
        rdfs:comment     "The fault connects the indicated phases to ground. The line to line fault impedance is not used and assumed infinite. The full ground impedance is connected between each phase specified in the fault and ground, but not between the phases." ;
        rdfs:label       "lineToGround"@en ;
        cims:stereotype  "enum" .

nc:FaultKind.lineToLine
        rdf:type         nc:FaultKind ;
        rdfs:comment     "The fault connects the specified phases together without a connection to ground. The ground impedance of this fault is ignored. The line to line impedance is connected between each of the phases specified in the fault. For example three times for a three phase fault, one time for a two phase fault.  A single phase fault should not be specified." ;
        rdfs:label       "lineToLine"@en ;
        cims:stereotype  "enum" .

nc:FaultKind.lineToLineToGround
        rdf:type         nc:FaultKind ;
        rdfs:comment     "The fault connects the indicated phases to ground and to each other. The line to line impedance is connected between each of the phases specified in the fault in a full mesh. For example three times for a three phase fault, one time for a two phase fault. A single phase fault should not be specified. The full ground impedance is connected between each phase specified in the fault and ground." ;
        rdfs:label       "lineToLineToGround"@en ;
        cims:stereotype  "enum" .

nc:FaultKind.other  rdf:type  nc:FaultKind ;
        rdfs:comment     "For example, geomagnetic currents, SSR, capacitor bank imbalances, bad contact, overheating." ;
        rdfs:label       "other"@en ;
        cims:stereotype  "enum" .

nc:FaultKind.undesiredFunction
        rdf:type         nc:FaultKind ;
        rdfs:comment     "If the component's main function occurred correctly but had an undesired result, that is, the fault.\nIs only stated if the component is a circuit breaker, disconnector or control system." ;
        rdfs:label       "undesiredFunction"@en ;
        cims:stereotype  "enum" .

nc:FaultOutage  rdf:type        rdfs:Class ;
        rdfs:comment            "Association class for relating one fault and one outage." ;
        rdfs:label              "FaultOutage"@en ;
        cims:belongsToCategory  gd:Package_GridDisturbanceProfile ;
        cims:stereotype         "NC" ;
        cims:stereotype         <http://iec.ch/TC57/NonStandard/UML#concrete> .

nc:FaultOutage.Fault  rdf:type  rdf:Property ;
        rdfs:comment          "The fault defined for this combination of a fault and an outage. " ;
        rdfs:domain           nc:FaultOutage ;
        rdfs:label            "Fault"@en ;
        rdfs:range            cim:Fault ;
        cims:AssociationUsed  "Yes" ;
        cims:inverseRoleName  nc:Fault.FaultOutage ;
        cims:multiplicity     cims:M:1 ;
        cims:stereotype       "NC" .

nc:FaultOutage.Outage
        rdf:type              rdf:Property ;
        rdfs:comment          "The outage defined for this combination of a fault and an outage." ;
        rdfs:domain           nc:FaultOutage ;
        rdfs:label            "Outage"@en ;
        rdfs:range            cim:Outage ;
        cims:AssociationUsed  "Yes" ;
        cims:inverseRoleName  nc:Outage.FaultOutage ;
        cims:multiplicity     cims:M:1 ;
        cims:stereotype       "NC" .

nc:FaultOutage.isMainFault
        rdf:type           rdf:Property ;
        rdfs:comment       "If true the fault outage is the main fault." ;
        rdfs:domain        nc:FaultOutage ;
        rdfs:label         "isMainFault"@en ;
        cims:dataType      cim:Boolean ;
        cims:multiplicity  cims:M:0..1 ;
        cims:stereotype    "NC" ;
        cims:stereotype    <http://iec.ch/TC57/NonStandard/UML#attribute> .

nc:FaultOutage.mRID  rdf:type  rdf:Property ;
        rdfs:comment       "Master resource identifier issued by a model authority. The mRID is unique within an exchange context. Global uniqueness is easily achieved by using a UUID, as specified in RFC 4122, for the mRID. The use of UUID is strongly recommended.\nFor CIMXML data files in RDF syntax conforming to IEC 61970-552, the mRID is mapped to rdf:ID or rdf:about attributes that identify CIM object elements." ;
        rdfs:domain        nc:FaultOutage ;
        rdfs:label         "mRID"@en ;
        cims:dataType      cim:String ;
        cims:multiplicity  cims:M:1..1 ;
        cims:stereotype    "NC" ;
        cims:stereotype    <http://iec.ch/TC57/NonStandard/UML#attribute> .

nc:GridDisturbance  rdf:type    rdfs:Class ;
        rdfs:comment            "Automatic, unintended, or manual undeferrable switching of breakers as a result of faults in the power grid." ;
        rdfs:label              "GridDisturbance"@en ;
        rdfs:subClassOf         cim:IdentifiedObject ;
        cims:belongsToCategory  gd:Package_GridDisturbanceProfile ;
        cims:stereotype         "NC" ;
        cims:stereotype         <http://iec.ch/TC57/NonStandard/UML#concrete> .

nc:GridDisturbance.Fault
        rdf:type              rdf:Property ;
        rdfs:comment          "Faults that are related to one grid disturbance." ;
        rdfs:domain           nc:GridDisturbance ;
        rdfs:label            "Fault"@en ;
        rdfs:range            cim:Fault ;
        cims:AssociationUsed  "No" ;
        cims:inverseRoleName  nc:Fault.GridDisturbance ;
        cims:multiplicity     cims:M:1..n ;
        cims:stereotype       "NC" .

nc:Interruption  rdf:type       rdfs:Class ;
        rdfs:comment            "Disappearance of the supply voltage at a delivery point." ;
        rdfs:label              "Interruption"@en ;
        rdfs:subClassOf         cim:IdentifiedObject ;
        cims:belongsToCategory  gd:Package_GridDisturbanceProfile ;
        cims:stereotype         "NC" ;
        cims:stereotype         <http://iec.ch/TC57/NonStandard/UML#concrete> .

nc:Interruption.InterruptedDeliveryEquipment
        rdf:type              rdf:Property ;
        rdfs:comment          "The delivery point (equipment) that is affected by the interruption. It is an equipment, power transformer or busbar in the grid where electricity is exchanged." ;
        rdfs:domain           nc:Interruption ;
        rdfs:label            "InterruptedDeliveryEquipment"@en ;
        rdfs:range            cim:Equipment ;
        cims:AssociationUsed  "Yes" ;
        cims:inverseRoleName  nc:Equipment.Interruption ;
        cims:multiplicity     cims:M:1 ;
        cims:stereotype       "NC" .

nc:Interruption.Outage
        rdf:type              rdf:Property ;
        rdfs:comment          "One outage may have multiple interruptions." ;
        rdfs:domain           nc:Interruption ;
        rdfs:label            "Outage"@en ;
        rdfs:range            cim:Outage ;
        cims:AssociationUsed  "Yes" ;
        cims:inverseRoleName  nc:Outage.Interruption ;
        cims:multiplicity     cims:M:0..1 ;
        cims:stereotype       "NC" .

nc:Interruption.duration
        rdf:type           rdf:Property ;
        rdfs:comment       "The duration of the interruption." ;
        rdfs:domain        nc:Interruption ;
        rdfs:label         "duration"@en ;
        cims:dataType      cim:Duration ;
        cims:multiplicity  cims:M:1..1 ;
        cims:stereotype    "NC" ;
        cims:stereotype    <http://iec.ch/TC57/NonStandard/UML#attribute> .

nc:Interruption.energyNotDelivered
        rdf:type           rdf:Property ;
        rdfs:comment       "The estimated energy which would have been delivered through the delivery point if no interruption and no transmission restrictions had occurred." ;
        rdfs:domain        nc:Interruption ;
        rdfs:label         "energyNotDelivered"@en ;
        cims:dataType      cim:RealEnergy ;
        cims:multiplicity  cims:M:0..1 ;
        cims:stereotype    "NC" ;
        cims:stereotype    <http://iec.ch/TC57/NonStandard/UML#attribute> .

nc:Interruption.energyNotSupplied
        rdf:type           rdf:Property ;
        rdfs:comment       "The estimated energy which would have been supplied to end-users if no interruption and no transmission restrictions had occurred." ;
        rdfs:domain        nc:Interruption ;
        rdfs:label         "energyNotSupplied"@en ;
        cims:dataType      cim:RealEnergy ;
        cims:multiplicity  cims:M:0..1 ;
        cims:stereotype    "NC" ;
        cims:stereotype    <http://iec.ch/TC57/NonStandard/UML#attribute> .

nc:Interruption.interruptedPower
        rdf:type           rdf:Property ;
        rdfs:comment       "The estimated power that was delivered through the delivery point when the interruption occurred." ;
        rdfs:domain        nc:Interruption ;
        rdfs:label         "interruptedPower"@en ;
        cims:dataType      cim:ActivePower ;
        cims:multiplicity  cims:M:1..1 ;
        cims:stereotype    "NC" ;
        cims:stereotype    <http://iec.ch/TC57/NonStandard/UML#attribute> .

nc:Interruption.startDateTime
        rdf:type           rdf:Property ;
        rdfs:comment       "The date and time at which the interruption occurred." ;
        rdfs:domain        nc:Interruption ;
        rdfs:label         "startDateTime"@en ;
        cims:dataType      cim:DateTime ;
        cims:multiplicity  cims:M:1..1 ;
        cims:stereotype    "NC" ;
        cims:stereotype    <http://iec.ch/TC57/NonStandard/UML#attribute> .

nc:Outage.FaultOutage
        rdf:type              rdf:Property ;
        rdfs:comment          "The combination of a fault and an outage to be simulated for this outage." ;
        rdfs:domain           cim:Outage ;
        rdfs:label            "FaultOutage"@en ;
        rdfs:range            nc:FaultOutage ;
        cims:AssociationUsed  "No" ;
        cims:inverseRoleName  nc:FaultOutage.Outage ;
        cims:multiplicity     cims:M:0..n ;
        cims:stereotype       "NC" .

nc:Outage.Interruption
        rdf:type              rdf:Property ;
        rdfs:comment          "Multiple interruptions may be connected with an outage." ;
        rdfs:domain           cim:Outage ;
        rdfs:label            "Interruption"@en ;
        rdfs:range            nc:Interruption ;
        cims:AssociationUsed  "No" ;
        cims:inverseRoleName  nc:Interruption.Outage ;
        cims:multiplicity     cims:M:0..n ;
        cims:stereotype       "NC" .

nc:SystemOperator  rdf:type     rdfs:Class ;
        rdfs:comment            "System operator." ;
        rdfs:label              "SystemOperator"@en ;
        cims:belongsToCategory  gd:Package_GridDisturbanceProfile ;
        cims:stereotype         "NC" .

nc:SystemOperator.Fault
        rdf:type              rdf:Property ;
        rdfs:comment          "The faults that have occurred in this System Operator's control area." ;
        rdfs:domain           nc:SystemOperator ;
        rdfs:label            "Fault"@en ;
        rdfs:range            cim:Fault ;
        cims:AssociationUsed  "No" ;
        cims:inverseRoleName  nc:Fault.SystemOperator ;
        cims:multiplicity     cims:M:0..n ;
        cims:stereotype       "NC" .

nc:SystemUnitKind  rdf:type     rdfs:Class ;
        rdfs:comment            "A system unit is defined as:\n\nA group of components which are delimited by one or more circuit breakers.\n\nNote 1: the system unit concept has been defined to simplify the calculation of availability. While a system unit is always delimited by circuit breakers, an individual component may not always be. A system unit may therefore contain more than one component. \n\nNote 2: the circuit breakers are not included in the system unit.\n \nNote 3: a tripped element is synonymous to a tripped system unit.\n\nNote 4: the type of a system unit is determined by its dominant component. The available system unit types are power transformer, overhead line, cable, reactor, busbar, series capacitor, shunt capacitor and SVC.\n\nNote 5: when a system unit is no longer transporting or supplying electrical energy, the system unit is affected by an outage. The system unit is unavailable after the outage has occurred." ;
        rdfs:label              "SystemUnitKind"@en ;
        cims:belongsToCategory  gd:Package_GridDisturbanceProfile ;
        cims:stereotype         "NC" ;
        cims:stereotype         <http://iec.ch/TC57/NonStandard/UML#enumeration> .

nc:SystemUnitKind.busbar
        rdf:type         nc:SystemUnitKind ;
        rdfs:comment     "If the main function of the system unit is busbar." ;
        rdfs:label       "busbar"@en ;
        cims:stereotype  "enum" .

nc:SystemUnitKind.cable
        rdf:type         nc:SystemUnitKind ;
        rdfs:comment     "If the main function of the system unit is cable." ;
        rdfs:label       "cable"@en ;
        cims:stereotype  "enum" .

nc:SystemUnitKind.dcCable
        rdf:type         nc:SystemUnitKind ;
        rdfs:comment     "If the main function of the system unit is DCCable." ;
        rdfs:label       "dcCable"@en ;
        cims:stereotype  "enum" .

nc:SystemUnitKind.dcConverter
        rdf:type         nc:SystemUnitKind ;
        rdfs:comment     "If the main function of the system unit is DCConverter." ;
        rdfs:label       "dcConverter"@en ;
        cims:stereotype  "enum" .

nc:SystemUnitKind.facts
        rdf:type         nc:SystemUnitKind ;
        rdfs:comment     "If the main function of the system unit is FACTS." ;
        rdfs:label       "facts"@en ;
        cims:stereotype  "enum" .

nc:SystemUnitKind.other
        rdf:type         nc:SystemUnitKind ;
        rdfs:comment     "If it is of other kind." ;
        rdfs:label       "other"@en ;
        cims:stereotype  "enum" .

nc:SystemUnitKind.overheadLine
        rdf:type         nc:SystemUnitKind ;
        rdfs:comment     "If the main function of the system unit is overhead line." ;
        rdfs:label       "overheadLine"@en ;
        cims:stereotype  "enum" .

nc:SystemUnitKind.powerTransformer
        rdf:type         nc:SystemUnitKind ;
        rdfs:comment     "If the main function of the system unit is power transformer." ;
        rdfs:label       "powerTransformer"@en ;
        cims:stereotype  "enum" .

nc:SystemUnitKind.reactor
        rdf:type         nc:SystemUnitKind ;
        rdfs:comment     "If the main function of the system unit is reactor." ;
        rdfs:label       "reactor"@en ;
        cims:stereotype  "enum" .

nc:SystemUnitKind.seriesCapacitor
        rdf:type         nc:SystemUnitKind ;
        rdfs:comment     "If the main function of the system unit is series capacitor." ;
        rdfs:label       "seriesCapacitor"@en ;
        cims:stereotype  "enum" .

nc:SystemUnitKind.shuntCapacitor
        rdf:type         nc:SystemUnitKind ;
        rdfs:comment     "If the main function of the system unit is shunt capacitor." ;
        rdfs:label       "shuntCapacitor"@en ;
        cims:stereotype  "enum" .

nc:SystemUnitKind.svc
        rdf:type         nc:SystemUnitKind ;
        rdfs:comment     "If the main function of the system unit is static var compensator (SVC)." ;
        rdfs:label       "svc"@en ;
        cims:stereotype  "enum" .

nc:TripKind  rdf:type           rdfs:Class ;
        rdfs:comment            "Whether the type of the trip due to the outage was automatic, automatic with successful automatic reclosing or manual.\n\nIn case of a fault in the reclosing automatics resulting in lack of reclosing, automatic should be chosen as an alternative." ;
        rdfs:label              "TripKind"@en ;
        cims:belongsToCategory  gd:Package_GridDisturbanceProfile ;
        cims:stereotype         "NC" ;
        cims:stereotype         <http://iec.ch/TC57/NonStandard/UML#enumeration> .

nc:TripKind.automatic
        rdf:type         nc:TripKind ;
        rdfs:comment     "The trip that resulted in the outage was automatic.\n\nIn case of a fault in the reclosing automatics resulting in lack of reclosing, automatic should be chosen as an alternative." ;
        rdfs:label       "automatic"@en ;
        cims:stereotype  "enum" .

nc:TripKind.automaticWithUnsuccessfulAutomaticReclosing
        rdf:type         nc:TripKind ;
        rdfs:comment     "The trip that resulted in an outage was correctly initiated but the automatic reclosing was unsuccessful.\n\nIn case of a fault in the reclosing automatics resulting in lack of reclosing, automatic should be chosen as an alternative." ;
        rdfs:label       "automaticWithUnsuccessfulAutomaticReclosing"@en ;
        cims:stereotype  "enum" .

nc:TripKind.manual  rdf:type  nc:TripKind ;
        rdfs:comment     "The trip that resulted in the outage was manually cleared." ;
        rdfs:label       "manual"@en ;
        cims:stereotype  "enum" .

nc:UnplannedOutage.autoReclosingKind
        rdf:type           rdf:Property ;
        rdfs:comment       "The type of autoreclosing that occurred with the trip.\n\nIf high-speed automatic reclosing is successful at one end of a line, but the line needs to be reclosed manually at the other end, choose manual reclosing.\n\nIn this document, high-speed automatic reclosing refers to automatic reclosing after less than 2 seconds." ;
        rdfs:domain        cim:UnplannedOutage ;
        rdfs:label         "autoReclosingKind"@en ;
        rdfs:range         nc:AutoReclosingKind ;
        cims:multiplicity  cims:M:1..1 ;
        cims:stereotype    "NC" ;
        cims:stereotype    <http://iec.ch/TC57/NonStandard/UML#attribute> .

nc:UnplannedOutage.duration
        rdf:type           rdf:Property ;
        rdfs:comment       "The duration of the unplanned outage." ;
        rdfs:domain        cim:UnplannedOutage ;
        rdfs:label         "duration"@en ;
        cims:dataType      cim:Duration ;
        cims:multiplicity  cims:M:1..1 ;
        cims:stereotype    "NC" ;
        cims:stereotype    <http://iec.ch/TC57/NonStandard/UML#attribute> .

nc:UnplannedOutage.startDateTime
        rdf:type           rdf:Property ;
        rdfs:comment       "The date and time at which the unplanned outage occurred." ;
        rdfs:domain        cim:UnplannedOutage ;
        rdfs:label         "startDateTime"@en ;
        cims:dataType      cim:DateTime ;
        cims:multiplicity  cims:M:0..1 ;
        cims:stereotype    "NC" ;
        cims:stereotype    <http://iec.ch/TC57/NonStandard/UML#attribute> .

nc:UnplannedOutage.systemUnitKind
        rdf:type           rdf:Property ;
        rdfs:comment       "The type of system unit of the component affected by the outage.\n\nA system unit is defined as:\n\nA group of components which are delimited by one or more circuit breakers.\n\nNote 1: the system unit concept has been defined to simplify the calculation of availability. While a system unit is always delimited by circuit breakers, an individual component may not always be. A system unit may therefore contain more than one component. \n\nNote 2: the circuit breakers are not included in the system unit.\n\nNote 3: a tripped element is synonymous to a tripped system unit.\n\nNote 4: the type of a system unit is determined by its dominant component. The available system unit types are power transformer, overhead line, cable, reactor, busbar, series capacitor, shunt capacitor and SVC.\n\nNote 5: when a system unit is no longer transporting or supplying electrical energy, the system unit is affected by an outage. The system unit is unavailable after the outage has occurred." ;
        rdfs:domain        cim:UnplannedOutage ;
        rdfs:label         "systemUnitKind"@en ;
        rdfs:range         nc:SystemUnitKind ;
        cims:multiplicity  cims:M:1..1 ;
        cims:stereotype    "NC" ;
        cims:stereotype    <http://iec.ch/TC57/NonStandard/UML#attribute> .

nc:UnplannedOutage.tripKind
        rdf:type           rdf:Property ;
        rdfs:comment       "Whether the type of the trip due to the outage was automatic, automatic with successful automatic reclosing or manual.\n\nIn case of a fault in the reclosing automatics resulting in lack of reclosing, automatic should be chosen as an alternative." ;
        rdfs:domain        cim:UnplannedOutage ;
        rdfs:label         "tripKind"@en ;
        rdfs:range         nc:TripKind ;
        cims:multiplicity  cims:M:1..1 ;
        cims:stereotype    "NC" ;
        cims:stereotype    <http://iec.ch/TC57/NonStandard/UML#attribute> .

profcim:IRI  rdf:type           rdfs:Class ;
        rdfs:comment            "An IRI (Internationalized Resource Identifier) within an RDF graph is a Unicode string that conforms to the syntax defined in RFC 3987.\nThe primitive is serialized as rdf:resource in RDFXML.\nIRIs in the RDF abstract syntax must be absolute, and may contain a fragment identifier.\nIRI equality: Two IRIs are equal if and only if they are equivalent under Simple String Comparison according to section 5.1 of [RFC3987]. Further normalization must not be performed when comparing IRIs for equality.\nIRIs are a generalization of URIs [RFC3986] that permits a wider range of Unicode characters. Every absolute URI and URL is an IRI, but not every IRI is an URI. When IRIs are used in operations that are only defined for URIs, they must first be converted according to the mapping defined in section 3.1 of [RFC3987]. A notable example is retrieval over the HTTP protocol. The mapping involves UTF-8 encoding of non-ASCII characters, %-encoding of octets not allowed in URIs, and Punycode-encoding of domain names." ;
        rdfs:label              "IRI"@en ;
        cims:belongsToCategory  gd:Package_DocGridDisturbanceProfile ;
        cims:stereotype         "profcim" , "Primitive" .

profcim:StringFixedLanguage
        rdf:type                rdfs:Class ;
        rdfs:comment            "A string consisting of a sequence of characters. The character encoding is UTF-8. The string length is unspecified and unlimited.\nThe primitive is serialized as literal without language support." ;
        rdfs:label              "StringFixedLanguage"@en ;
        cims:belongsToCategory  gd:Package_DocGridDisturbanceProfile ;
        cims:stereotype         "profcim" , "Primitive" .

profcim:StringIRI  rdf:type     rdfs:Class ;
        rdfs:comment            "An IRI (Internationalized Resource Identifier) within an RDF graph is a Unicode string that conforms to the syntax defined in RFC 3987.\nThe primitive is serialized as literal without language support.\nIRIs in the RDF abstract syntax must be absolute, and may contain a fragment identifier.\nIRI equality: Two IRIs are equal if and only if they are equivalent under Simple String Comparison according to section 5.1 of [RFC3987]. Further normalization must not be performed when comparing IRIs for equality.\nIRIs are a generalization of URIs [RFC3986] that permits a wider range of Unicode characters. Every absolute URI and URL is an IRI, but not every IRI is an URI. When IRIs are used in operations that are only defined for URIs, they must first be converted according to the mapping defined in section 3.1 of [RFC3987]. A notable example is retrieval over the HTTP protocol. The mapping involves UTF-8 encoding of non-ASCII characters, %-encoding of octets not allowed in URIs, and Punycode-encoding of domain names." ;
        rdfs:label              "StringIRI"@en ;
        cims:belongsToCategory  gd:Package_DocGridDisturbanceProfile ;
        cims:stereotype         "profcim" , "Primitive" .

profcim:URL  rdf:type           rdfs:Class ;
        rdfs:comment            "A Uniform Resource Locator (URL), colloquially termed a web address, is a reference to a web resource that specifies its location on a computer network and a mechanism for retrieving it. A URL is a specific type of Uniform Resource Identifier (URI), although many people use the two terms interchangeably.URLs occur most commonly to reference web pages (http), but are also used for file transfer (ftp), email (mailto), database access (JDBC), and many other applications." ;
        rdfs:label              "URL"@en ;
        cims:belongsToCategory  gd:Package_DocGridDisturbanceProfile ;
        cims:stereotype         "profcim" , "Primitive" .

