@prefix cim:     <https://cim.ucaiug.io/ns#> .
@prefix cims:    <http://iec.ch/TC57/1999/rdf-schema-extensions-19990926#> .
@prefix dcat:    <http://www.w3.org/ns/dcat#> .
@prefix dcterms: <http://purl.org/dc/terms/#> .
@prefix eu:      <https://cim.ucaiug.io/ns/eu#> .
@prefix nc:      <https://cim4.eu/ns/nc#> .
@prefix or:      <https://ap.cim4.eu/ObjectRegistry#> .
@prefix owl:     <http://www.w3.org/2002/07/owl#> .
@prefix rdf:     <http://www.w3.org/1999/02/22-rdf-syntax-ns#> .
@prefix rdfs:    <http://www.w3.org/2000/01/rdf-schema#> .

<http://iec.ch/TC57/ns/CIM/prof-cim#IRI>
        rdf:type                rdfs:Class ;
        rdfs:comment            "An IRI (Internationalized Resource Identifier) within an RDF graph is a Unicode string that conforms to the syntax defined in RFC 3987.\nThe primitive is serialized as rdf:resource in RDFXML.\nIRIs in the RDF abstract syntax must be absolute, and may contain a fragment identifier.\nIRI equality: Two IRIs are equal if and only if they are equivalent under Simple String Comparison according to section 5.1 of [RFC3987]. Further normalization must not be performed when comparing IRIs for equality.\nIRIs are a generalization of URIs [RFC3986] that permits a wider range of Unicode characters. Every absolute URI and URL is an IRI, but not every IRI is an URI. When IRIs are used in operations that are only defined for URIs, they must first be converted according to the mapping defined in section 3.1 of [RFC3987]. A notable example is retrieval over the HTTP protocol. The mapping involves UTF-8 encoding of non-ASCII characters, %-encoding of octets not allowed in URIs, and Punycode-encoding of domain names." ;
        rdfs:label              "IRI"@en ;
        cims:belongsToCategory  or:Package_DocObjectRegistryProfile ;
        cims:stereotype         "profcim" , "Primitive" .

<http://iec.ch/TC57/ns/CIM/prof-cim#StringFixedLanguage>
        rdf:type                rdfs:Class ;
        rdfs:comment            "A string consisting of a sequence of characters. The character encoding is UTF-8. The string length is unspecified and unlimited.\nThe primitive is serialized as literal without language support." ;
        rdfs:label              "StringFixedLanguage"@en ;
        cims:belongsToCategory  or:Package_DocObjectRegistryProfile ;
        cims:stereotype         "profcim" , "Primitive" .

<http://iec.ch/TC57/ns/CIM/prof-cim#StringIRI>
        rdf:type                rdfs:Class ;
        rdfs:comment            "An IRI (Internationalized Resource Identifier) within an RDF graph is a Unicode string that conforms to the syntax defined in RFC 3987.\nThe primitive is serialized as literal without language support.\nIRIs in the RDF abstract syntax must be absolute, and may contain a fragment identifier.\nIRI equality: Two IRIs are equal if and only if they are equivalent under Simple String Comparison according to section 5.1 of [RFC3987]. Further normalization must not be performed when comparing IRIs for equality.\nIRIs are a generalization of URIs [RFC3986] that permits a wider range of Unicode characters. Every absolute URI and URL is an IRI, but not every IRI is an URI. When IRIs are used in operations that are only defined for URIs, they must first be converted according to the mapping defined in section 3.1 of [RFC3987]. A notable example is retrieval over the HTTP protocol. The mapping involves UTF-8 encoding of non-ASCII characters, %-encoding of octets not allowed in URIs, and Punycode-encoding of domain names." ;
        rdfs:label              "StringIRI"@en ;
        cims:belongsToCategory  or:Package_DocObjectRegistryProfile ;
        cims:stereotype         "profcim" , "Primitive" .

<http://iec.ch/TC57/ns/CIM/prof-cim#URL>
        rdf:type                rdfs:Class ;
        rdfs:comment            "A Uniform Resource Locator (URL), colloquially termed a web address, is a reference to a web resource that specifies its location on a computer network and a mechanism for retrieving it. A URL is a specific type of Uniform Resource Identifier (URI), although many people use the two terms interchangeably.URLs occur most commonly to reference web pages (http), but are also used for file transfer (ftp), email (mailto), database access (JDBC), and many other applications." ;
        rdfs:label              "URL"@en ;
        cims:belongsToCategory  or:Package_DocObjectRegistryProfile ;
        cims:stereotype         "profcim" , "Primitive" .

cim:Date  rdf:type              rdfs:Class ;
        rdfs:comment            "Date as \"yyyy-mm-dd\", which conforms with ISO 8601. UTC time zone is specified as \"yyyy-mm-ddZ\". A local timezone relative UTC is specified as \"yyyy-mm-dd(+/-)hh:mm\"." ;
        rdfs:label              "Date"@en ;
        cims:belongsToCategory  or:Package_DocObjectRegistryProfile ;
        cims:stereotype         "Primitive" .

cim:DateTime  rdf:type          rdfs:Class ;
        rdfs:comment            "Date and time as \"yyyy-mm-ddThh:mm:ss.sss\", which conforms with ISO 8601. UTC time zone is specified as \"yyyy-mm-ddThh:mm:ss.sssZ\". A local timezone relative UTC is specified as \"yyyy-mm-ddThh:mm:ss.sss-hh:mm\". The second component (shown here as \"ss.sss\") could have any number of digits in its fractional part to allow any kind of precision beyond seconds." ;
        rdfs:label              "DateTime"@en ;
        cims:belongsToCategory  or:Package_DocObjectRegistryProfile ;
        cims:stereotype         "Primitive" .

cim:IdentifiedObject  rdf:type  rdfs:Class ;
        rdfs:comment            "This is a root class to provide common identification for all classes needing identification and naming attributes." ;
        rdfs:label              "IdentifiedObject"@en ;
        cims:belongsToCategory  or:Package_ObjectRegistryProfile ;
        cims:stereotype         <http://iec.ch/TC57/NonStandard/UML#concrete> .

cim:IdentifiedObject.aliasName
        rdf:type           rdf:Property ;
        rdfs:comment       "The aliasName is free text human readable name of the object alternative to IdentifiedObject.name. It may be non unique and may not correlate to a naming hierarchy.\nThe attribute aliasName is retained because of backwards compatibility between CIM relases. It is however recommended to replace aliasName with the Name class as aliasName is planned for retirement at a future time." ;
        rdfs:domain        cim:IdentifiedObject ;
        rdfs:label         "aliasName"@en ;
        cims:dataType      cim:String ;
        cims:multiplicity  cims:M:0..1 ;
        cims:stereotype    <http://iec.ch/TC57/NonStandard/UML#attribute> .

cim:IdentifiedObject.description
        rdf:type           rdf:Property ;
        rdfs:comment       "The description is a free human readable text describing or naming the object. It may be non unique and may not correlate to a naming hierarchy." ;
        rdfs:domain        cim:IdentifiedObject ;
        rdfs:label         "description"@en ;
        cims:dataType      cim:String ;
        cims:multiplicity  cims:M:0..1 ;
        cims:stereotype    <http://iec.ch/TC57/NonStandard/UML#attribute> .

cim:IdentifiedObject.mRID
        rdf:type           rdf:Property ;
        rdfs:comment       "Master resource identifier issued by a model authority. The mRID is unique within an exchange context. Global uniqueness is easily achieved by using a UUID, as specified in RFC 4122, for the mRID. The use of UUID is strongly recommended.\nFor CIMXML data files in RDF syntax conforming to IEC 61970-552, the mRID is mapped to rdf:ID or rdf:about attributes that identify CIM object elements." ;
        rdfs:domain        cim:IdentifiedObject ;
        rdfs:label         "mRID"@en ;
        cims:dataType      cim:String ;
        cims:multiplicity  cims:M:1..1 ;
        cims:stereotype    <http://iec.ch/TC57/NonStandard/UML#attribute> .

cim:IdentifiedObject.name
        rdf:type           rdf:Property ;
        rdfs:comment       "The name is any free human readable and possibly non unique text naming the object." ;
        rdfs:domain        cim:IdentifiedObject ;
        rdfs:label         "name"@en ;
        cims:dataType      cim:String ;
        cims:multiplicity  cims:M:0..1 ;
        cims:stereotype    <http://iec.ch/TC57/NonStandard/UML#attribute> .

cim:Name  rdf:type              rdfs:Class ;
        rdfs:comment            "The Name class provides the means to define any number of human readable  names for an object. A name is <b>not</b> to be used for defining inter-object relationships. For inter-object relationships instead use the object identification 'mRID'." ;
        rdfs:label              "Name"@en ;
        cims:belongsToCategory  or:Package_ObjectRegistryProfile ;
        cims:stereotype         <http://iec.ch/TC57/NonStandard/UML#concrete> .

cim:Name.name  rdf:type    rdf:Property ;
        rdfs:comment       "Any free text that used as a name or alternative identifier of the object." ;
        rdfs:domain        cim:Name ;
        rdfs:label         "name"@en ;
        cims:dataType      cim:String ;
        cims:multiplicity  cims:M:1..1 ;
        cims:stereotype    <http://iec.ch/TC57/NonStandard/UML#attribute> .

cim:NameType  rdf:type          rdfs:Class ;
        rdfs:comment            "Type of name. Possible values for attribute 'name' are implementation dependent but standard profiles may specify types. An enterprise may have multiple IT systems each having its own local name for the same object, e.g. a planning system may have different names from an EMS. An object may also have different names within the same IT system, e.g. localName as defined in CIM version 14. The definition from CIM14 is:\nThe localName is a human readable name of the object. It is a free text name local to a node in a naming hierarchy similar to a file directory structure. A power system related naming hierarchy may be: Substation, VoltageLevel, Equipment etc. Children of the same parent in such a hierarchy have names that typically are unique among them." ;
        rdfs:label              "NameType"@en ;
        cims:belongsToCategory  or:Package_ObjectRegistryProfile ;
        cims:stereotype         <http://iec.ch/TC57/NonStandard/UML#concrete> .

cim:NameType.description
        rdf:type           rdf:Property ;
        rdfs:comment       "Description of the name type." ;
        rdfs:domain        cim:NameType ;
        rdfs:label         "description"@en ;
        cims:dataType      cim:String ;
        cims:multiplicity  cims:M:0..1 ;
        cims:stereotype    <http://iec.ch/TC57/NonStandard/UML#attribute> .

cim:NameType.name  rdf:type  rdf:Property ;
        rdfs:comment       "Name of the name type." ;
        rdfs:domain        cim:NameType ;
        rdfs:label         "name"@en ;
        cims:dataType      cim:String ;
        cims:multiplicity  cims:M:1..1 ;
        cims:stereotype    <http://iec.ch/TC57/NonStandard/UML#attribute> .

cim:String  rdf:type            rdfs:Class ;
        rdfs:comment            "A string consisting of a sequence of characters. The character encoding is UTF-8. The string length is unspecified and unlimited." ;
        rdfs:label              "String"@en ;
        cims:belongsToCategory  or:Package_ObjectRegistryProfile ;
        cims:stereotype         "Primitive" .

eu:IdentifiedObject.energyIdentCodeEic
        rdf:type           rdf:Property ;
        rdfs:comment       "The attribute is used for an exchange of the EIC code (Energy identification Code). The length of the string is 16 characters as defined by the EIC code. For details on EIC scheme please refer to ENTSO-E web site." ;
        rdfs:domain        cim:IdentifiedObject ;
        rdfs:label         "energyIdentCodeEic"@en ;
        cims:dataType      cim:String ;
        cims:multiplicity  cims:M:0..1 ;
        cims:stereotype    "deprecated" , "European" ;
        cims:stereotype    <http://iec.ch/TC57/NonStandard/UML#attribute> .

eu:IdentifiedObject.shortName
        rdf:type           rdf:Property ;
        rdfs:comment       "The attribute is used for an exchange of a human readable short name with length of the string 12 characters maximum." ;
        rdfs:domain        cim:IdentifiedObject ;
        rdfs:label         "shortName"@en ;
        cims:dataType      cim:String ;
        cims:multiplicity  cims:M:0..1 ;
        cims:stereotype    "deprecated" , "European" ;
        cims:stereotype    <http://iec.ch/TC57/NonStandard/UML#attribute> .

nc:IdentifiedObject.AlternativeIdentifier
        rdf:type              rdf:Property ;
        rdfs:comment          "All alternative identifiers of this identified object. No two identified objects can have the same alternative identifier." ;
        rdfs:domain           cim:IdentifiedObject ;
        rdfs:label            "AlternativeIdentifier"@en ;
        rdfs:range            cim:Name ;
        cims:AssociationUsed  "No" ;
        cims:inverseRoleName  nc:Name.UniqueIdentifiedObject ;
        cims:multiplicity     cims:M:0..n ;
        cims:stereotype       "NC" .
nc:IdentifiedObject.Name
        rdf:type              rdf:Property ;
        rdfs:comment          "All names of this identified object. Names may be but are not guaranteed to be unique." ;
        rdfs:domain           cim:IdentifiedObject ;
        rdfs:label            "Name"@en ;
        rdfs:range            cim:Name ;
        cims:AssociationUsed  "No" ;
        cims:inverseRoleName  nc:Name.IdentifiedObject ;
        cims:multiplicity     cims:M:0..n ;
        cims:stereotype       "NC" .

nc:IdentifiedObject.ObjectType
        rdf:type              rdf:Property ;
        rdfs:comment          "The object type of the IdentifiedObject." ;
        rdfs:domain           cim:IdentifiedObject ;
        rdfs:label            "ObjectType"@en ;
        rdfs:range            nc:ObjectType ;
        cims:AssociationUsed  "Yes" ;
        cims:inverseRoleName  nc:ObjectType.IdentifiedObject ;
        cims:multiplicity     cims:M:0..1 ;
        cims:stereotype       "NC" .

nc:Name.IdentifiedObject
        rdf:type              rdf:Property ;
        rdfs:comment          "Identified object that this name designates." ;
        rdfs:domain           cim:Name ;
        rdfs:label            "IdentifiedObject"@en ;
        rdfs:range            cim:IdentifiedObject ;
        cims:AssociationUsed  "Yes" ;
        cims:inverseRoleName  nc:IdentifiedObject.Name ;
        cims:multiplicity     cims:M:0..1 ;
        cims:stereotype       "NC" .

nc:Name.NameType  rdf:type    rdf:Property ;
        rdfs:comment          "Type of this name." ;
        rdfs:domain           cim:Name ;
        rdfs:label            "NameType"@en ;
        rdfs:range            cim:NameType ;
        cims:AssociationUsed  "Yes" ;
        cims:inverseRoleName  nc:NameType.Name ;
        cims:multiplicity     cims:M:0..1 ;
        cims:stereotype       "NC" .

nc:Name.NamingAuthority
        rdf:type              rdf:Property ;
        rdfs:comment          "Authority responsible for managing this name." ;
        rdfs:domain           cim:Name ;
        rdfs:label            "NamingAuthority"@en ;
        rdfs:range            nc:NamingAuthority ;
        cims:AssociationUsed  "Yes" ;
        cims:inverseRoleName  nc:NamingAuthority.Name ;
        cims:multiplicity     cims:M:0..1 ;
        cims:stereotype       "NC" .

nc:Name.UniqueIdentifiedObject
        rdf:type              rdf:Property ;
        rdfs:comment          "Identified object that this alternative identifier designates." ;
        rdfs:domain           cim:Name ;
        rdfs:label            "UniqueIdentifiedObject"@en ;
        rdfs:range            cim:IdentifiedObject ;
        cims:AssociationUsed  "Yes" ;
        cims:inverseRoleName  nc:IdentifiedObject.AlternativeIdentifier ;
        cims:multiplicity     cims:M:0..1 ;
        cims:stereotype       "NC" .

nc:Name.language  rdf:type  rdf:Property ;
        rdfs:comment       "Shall be specified as an IETF BCP 47 language tag (e.g. en-US).  Applies to the Name.name attribute. \nIETF language tags combine subtags from other standards such as ISO 639, ISO 15924, ISO 3166-1, and UN M.49. The tag structure has been standardized by the IETF in Best Current Practice (BCP) 47; the subtags are maintained by the IANA Language Subtag Registry." ;
        rdfs:domain        cim:Name ;
        rdfs:label         "language"@en ;
        cims:dataType      cim:String ;
        cims:multiplicity  cims:M:0..1 ;
        cims:stereotype    "NC" ;
        cims:stereotype    <http://iec.ch/TC57/NonStandard/UML#attribute> .

nc:Name.mRID  rdf:type     rdf:Property ;
        rdfs:comment       "Master resource identifier issued by a model authority. The mRID is unique within an exchange context. Global uniqueness is easily achieved by using a UUID, as specified in RFC 4122, for the mRID. The use of UUID is strongly recommended.\nFor CIMXML data files in RDF syntax conforming to IEC 61970-552, the mRID is mapped to rdf:ID or rdf:about attributes that identify CIM object elements." ;
        rdfs:domain        cim:Name ;
        rdfs:label         "mRID"@en ;
        cims:dataType      cim:String ;
        cims:multiplicity  cims:M:0..1 ;
        cims:stereotype    "NC" ;
        cims:stereotype    <http://iec.ch/TC57/NonStandard/UML#attribute> .

nc:NameType.Name  rdf:type    rdf:Property ;
        rdfs:comment          "All names of this type." ;
        rdfs:domain           cim:NameType ;
        rdfs:label            "Name"@en ;
        rdfs:range            cim:Name ;
        cims:AssociationUsed  "No" ;
        cims:inverseRoleName  nc:Name.NameType ;
        cims:multiplicity     cims:M:0..n ;
        cims:stereotype       "NC" .

nc:NameType.NamingAuthority
        rdf:type              rdf:Property ;
        rdfs:comment          "Authority responsible for managing this name type." ;
        rdfs:domain           cim:NameType ;
        rdfs:label            "NamingAuthority"@en ;
        rdfs:range            nc:NamingAuthority ;
        cims:AssociationUsed  "Yes" ;
        cims:inverseRoleName  nc:NamingAuthority.NameType ;
        cims:multiplicity     cims:M:0..1 ;
        cims:stereotype       "NC" .

nc:NameType.mRID  rdf:type  rdf:Property ;
        rdfs:comment       "Master resource identifier issued by a model authority. The mRID is unique within an exchange context. Global uniqueness is easily achieved by using a UUID, as specified in RFC 4122, for the mRID. The use of UUID is strongly recommended.\nFor CIMXML data files in RDF syntax conforming to IEC 61970-552, the mRID is mapped to rdf:ID or rdf:about attributes that identify CIM object elements." ;
        rdfs:domain        cim:NameType ;
        rdfs:label         "mRID"@en ;
        cims:dataType      cim:String ;
        cims:multiplicity  cims:M:1..1 ;
        cims:stereotype    "NC" ;
        cims:stereotype    <http://iec.ch/TC57/NonStandard/UML#attribute> .

nc:NamingAuthority  rdf:type    rdfs:Class ;
        rdfs:comment            "Authority responsible for creation and management of names of a given name type and/or name; typically an organization or an enterprise system." ;
        rdfs:label              "NamingAuthority"@en ;
        cims:belongsToCategory  or:Package_ObjectRegistryProfile ;
        cims:stereotype         "NC" ;
        cims:stereotype         <http://iec.ch/TC57/NonStandard/UML#concrete> .

nc:NamingAuthority.Name
        rdf:type              rdf:Property ;
        rdfs:comment          "All names managed by this authority." ;
        rdfs:domain           nc:NamingAuthority ;
        rdfs:label            "Name"@en ;
        rdfs:range            cim:Name ;
        cims:AssociationUsed  "No" ;
        cims:inverseRoleName  nc:Name.NamingAuthority ;
        cims:multiplicity     cims:M:0..n ;
        cims:stereotype       "NC" .

nc:NamingAuthority.NameType
        rdf:type              rdf:Property ;
        rdfs:comment          "All name types managed by this authority." ;
        rdfs:domain           nc:NamingAuthority ;
        rdfs:label            "NameType"@en ;
        rdfs:range            cim:NameType ;
        cims:AssociationUsed  "No" ;
        cims:inverseRoleName  nc:NameType.NamingAuthority ;
        cims:multiplicity     cims:M:0..n ;
        cims:stereotype       "NC" .

nc:NamingAuthority.description
        rdf:type           rdf:Property ;
        rdfs:comment       "Description of the name authority." ;
        rdfs:domain        nc:NamingAuthority ;
        rdfs:label         "description"@en ;
        cims:dataType      cim:String ;
        cims:multiplicity  cims:M:0..1 ;
        cims:stereotype    "NC" ;
        cims:stereotype    <http://iec.ch/TC57/NonStandard/UML#attribute> .

nc:NamingAuthority.mRID
        rdf:type           rdf:Property ;
        rdfs:comment       "Master resource identifier issued by a model authority. The mRID is unique within an exchange context. Global uniqueness is easily achieved by using a UUID, as specified in RFC 4122, for the mRID. The use of UUID is strongly recommended.\nFor CIMXML data files in RDF syntax conforming to IEC 61970-552, the mRID is mapped to rdf:ID or rdf:about attributes that identify CIM object elements." ;
        rdfs:domain        nc:NamingAuthority ;
        rdfs:label         "mRID"@en ;
        cims:dataType      cim:String ;
        cims:multiplicity  cims:M:1..1 ;
        cims:stereotype    "NC" ;
        cims:stereotype    <http://iec.ch/TC57/NonStandard/UML#attribute> .

nc:NamingAuthority.name
        rdf:type           rdf:Property ;
        rdfs:comment       "Name of the name authority." ;
        rdfs:domain        nc:NamingAuthority ;
        rdfs:label         "name"@en ;
        cims:dataType      cim:String ;
        cims:multiplicity  cims:M:1..1 ;
        cims:stereotype    "NC" ;
        cims:stereotype    <http://iec.ch/TC57/NonStandard/UML#attribute> .

nc:ObjectType  rdf:type         rdfs:Class ;
        rdfs:comment            "Identifies the specialised type of an object when the instance object is serialised using a generalised class. It may be useful when the object type is not otherwise included in the exchange. For example, a Meter may be serialised as an EndDevice in message exchanges and need to have the ObjectType.type be specified as 'Meter' to provide context to the message receiver." ;
        rdfs:label              "ObjectType"@en ;
        cims:belongsToCategory  or:Package_ObjectRegistryProfile ;
        cims:stereotype         "NC" ;
        cims:stereotype         <http://iec.ch/TC57/NonStandard/UML#concrete> .

nc:ObjectType.IdentifiedObject
        rdf:type              rdf:Property ;
        rdfs:comment          "The IdentifiedObject whose type is identified by ObjectType." ;
        rdfs:domain           nc:ObjectType ;
        rdfs:label            "IdentifiedObject"@en ;
        rdfs:range            cim:IdentifiedObject ;
        cims:AssociationUsed  "No" ;
        cims:inverseRoleName  nc:IdentifiedObject.ObjectType ;
        cims:multiplicity     cims:M:0..n ;
        cims:stereotype       "NC" .

nc:ObjectType.type  rdf:type  rdf:Property ;
        rdfs:comment       "The specialised type of an object when the instance object is serialised using a generalised class. For example, a Meter being serialised as an EndDevice in a message exchange should have the type attribute specified as 'Meter'." ;
        rdfs:domain        nc:ObjectType ;
        rdfs:label         "type"@en ;
        cims:dataType      cim:String ;
        cims:multiplicity  cims:M:1..1 ;
        cims:stereotype    "NC" ;
        cims:stereotype    <http://iec.ch/TC57/NonStandard/UML#attribute> .

or:Ontology  rdf:type         owl:Ontology ;
        dcterms:conformsTo    "urn:iso:std:iec:61970-501:draft:ed-2" , "file://CIM100_CGMES31v01_501-20v02_NC23v62_MM10v01.eap" , "urn:iso:std:iec:61970-401:draft:ed-1" , "file://iec61970cim17v40_iec61968cim13v13a_iec62325cim03v17a.eap" , "urn:iso:std:iec:61970-301:ed-7:amd1" , "urn:iso:std:iec:61970-600-2:ed-1" ;
        dcterms:creator       "ENTSO-E CIM WG NC project"@en ;
        dcterms:description   "This vocabulary is describing the object registry profile."@en ;
        dcterms:identifier    "urn:uuid:14166b65-abaa-4611-b466-34975c15c27d" ;
        dcterms:language      "en-GB" ;
        dcterms:license       "https://www.apache.org/licenses/LICENSE-2.0"@en ;
        dcterms:modified      "2024-03-20"^^<http://www.w3.org/2001/XMLSchema#date> ;
        dcterms:publisher     "ENTSO-E"@en ;
        dcterms:rightsHolder  "ENTSO-E"@en ;
        dcterms:title         "Object Registry vocabulary"@en ;
        owl:priorVersion      <http://entsoe.eu/ns/CIM/ObjectRegistry-EU/2.1> ;
        owl:versionIRI        <https://ap.cim4.eu/ObjectRegistry/2.2> ;
        owl:versionInfo       "2.2.0"@en ;
        dcat:keyword          "OR" ;
        dcat:theme            "vocabulary"@en .

or:Package_DocObjectRegistryProfile
        rdf:type      cims:ClassCategory ;
        rdfs:comment  "This package contains datatypes used only in the RDFS header." ;
        rdfs:label    "DocObjectRegistryProfile"@en .

or:Package_ObjectRegistryProfile
        rdf:type      cims:ClassCategory ;
        rdfs:comment  "This package contains the equipment object registry profile." ;
        rdfs:label    "ObjectRegistryProfile"@en .

