@prefix cim:     <https://cim.ucaiug.io/ns#> .
@prefix cims:    <http://iec.ch/TC57/1999/rdf-schema-extensions-19990926#> .
@prefix dcat:    <http://www.w3.org/ns/dcat#> .
@prefix dcterms: <http://purl.org/dc/terms/#> .
@prefix nc:      <https://cim4.eu/ns/nc#> .
@prefix owl:     <http://www.w3.org/2002/07/owl#> .
@prefix profcim: <https://cim.ucaiug.io/ns/prof-cim#> .
@prefix rdf:     <http://www.w3.org/1999/02/22-rdf-syntax-ns#> .
@prefix rdfs:    <http://www.w3.org/2000/01/rdf-schema#> .
@prefix sm:      <https://ap.cim4.eu/SensitivityMatrix#> .

cim:Contingency  rdf:type       rdfs:Class ;
        rdfs:comment            "An event threatening system reliability, consisting of one or more contingency elements." ;
        rdfs:label              "Contingency"@en ;
        cims:belongsToCategory  sm:Package_SensitivityMatrixProfile .

cim:Date  rdf:type              rdfs:Class ;
        rdfs:comment            "Date as \"yyyy-mm-dd\", which conforms with ISO 8601. UTC time zone is specified as \"yyyy-mm-ddZ\". A local timezone relative UTC is specified as \"yyyy-mm-dd(+/-)hh:mm\"." ;
        rdfs:label              "Date"@en ;
        cims:belongsToCategory  sm:Package_DocSensitivityMatrixProfile ;
        cims:stereotype         "Primitive" .

cim:DateTime  rdf:type          rdfs:Class ;
        rdfs:comment            "Date and time as \"yyyy-mm-ddThh:mm:ss.sss\", which conforms with ISO 8601. UTC time zone is specified as \"yyyy-mm-ddThh:mm:ss.sssZ\". A local timezone relative UTC is specified as \"yyyy-mm-ddThh:mm:ss.sss-hh:mm\". The second component (shown here as \"ss.sss\") could have any number of digits in its fractional part to allow any kind of precision beyond seconds." ;
        rdfs:label              "DateTime"@en ;
        cims:belongsToCategory  sm:Package_DocSensitivityMatrixProfile ;
        cims:stereotype         "Primitive" .

cim:Float  rdf:type             rdfs:Class ;
        rdfs:comment            "A floating point number. The range is unspecified and not limited." ;
        rdfs:label              "Float"@en ;
        cims:belongsToCategory  sm:Package_SensitivityMatrixProfile ;
        cims:stereotype         "Primitive" .

cim:IdentifiedObject  rdf:type  rdfs:Class ;
        rdfs:comment            "This is a root class to provide common identification for all classes needing identification and naming attributes." ;
        rdfs:label              "IdentifiedObject"@en ;
        cims:belongsToCategory  sm:Package_SensitivityMatrixProfile .

cim:IdentifiedObject.description
        rdf:type           rdf:Property ;
        rdfs:comment       "The description is a free human readable text describing or naming the object. It may be non unique and may not correlate to a naming hierarchy." ;
        rdfs:domain        cim:IdentifiedObject ;
        rdfs:label         "description"@en ;
        cims:dataType      cim:String ;
        cims:multiplicity  cims:M:0..1 ;
        cims:stereotype    <http://iec.ch/TC57/NonStandard/UML#attribute> .

cim:IdentifiedObject.mRID
        rdf:type           rdf:Property ;
        rdfs:comment       "Master resource identifier issued by a model authority. The mRID is unique within an exchange context. Global uniqueness is easily achieved by using a UUID, as specified in RFC 4122, for the mRID. The use of UUID is strongly recommended.\nFor CIMXML data files in RDF syntax conforming to IEC 61970-552, the mRID is mapped to rdf:ID or rdf:about attributes that identify CIM object elements." ;
        rdfs:domain        cim:IdentifiedObject ;
        rdfs:label         "mRID"@en ;
        cims:dataType      cim:String ;
        cims:multiplicity  cims:M:1..1 ;
        cims:stereotype    <http://iec.ch/TC57/NonStandard/UML#attribute> .

cim:IdentifiedObject.name
        rdf:type           rdf:Property ;
        rdfs:comment       "The name is any free human readable and possibly non unique text naming the object." ;
        rdfs:domain        cim:IdentifiedObject ;
        rdfs:label         "name"@en ;
        cims:dataType      cim:String ;
        cims:multiplicity  cims:M:0..1 ;
        cims:stereotype    <http://iec.ch/TC57/NonStandard/UML#attribute> .

cim:String  rdf:type            rdfs:Class ;
        rdfs:comment            "A string consisting of a sequence of characters. The character encoding is UTF-8. The string length is unspecified and unlimited." ;
        rdfs:label              "String"@en ;
        cims:belongsToCategory  sm:Package_SensitivityMatrixProfile ;
        cims:stereotype         "Primitive" .

nc:AssessedElement  rdf:type    rdfs:Class ;
        rdfs:comment            "Assessed element is a network element for which the electrical state is evaluated in the regional or cross-regional process and which value is expected to fulfil regional rules function of the operational security limits.\nThe measurements and limits are as defined in the steady state hypothesis." ;
        rdfs:label              "AssessedElement"@en ;
        cims:belongsToCategory  sm:Package_SensitivityMatrixProfile ;
        cims:stereotype         "NC" .

nc:AssessedElement.ObservableQuantity
        rdf:type              rdf:Property ;
        rdfs:comment          "The observable quantity for this assessed element with contingency." ;
        rdfs:domain           nc:AssessedElement ;
        rdfs:label            "ObservableQuantity"@en ;
        rdfs:range            nc:ObservableQuantity ;
        cims:AssociationUsed  "No" ;
        cims:inverseRoleName  nc:ObservableQuantity.AssessedElement ;
        cims:multiplicity     cims:M:0..n ;
        cims:stereotype       "NC" .

nc:Contingency.ObservableQuantity
        rdf:type              rdf:Property ;
        rdfs:comment          "The observable quantity for this contingency." ;
        rdfs:domain           cim:Contingency ;
        rdfs:label            "ObservableQuantity"@en ;
        rdfs:range            nc:ObservableQuantity ;
        cims:AssociationUsed  "No" ;
        cims:inverseRoleName  nc:ObservableQuantity.Contingency ;
        cims:multiplicity     cims:M:0..n ;
        cims:stereotype       "NC" .

nc:ControllableQuantity
        rdf:type                rdfs:Class ;
        rdfs:comment            "Controllable quantity is a set point quantity on a grid state alteration or on a remedial action." ;
        rdfs:label              "ControllableQuantity"@en ;
        cims:belongsToCategory  sm:Package_SensitivityMatrixProfile ;
        cims:stereotype         "NC" ;
        cims:stereotype         <http://iec.ch/TC57/NonStandard/UML#concrete> .

nc:ControllableQuantity.GridStateAlteration
        rdf:type              rdf:Property ;
        rdfs:comment          "The grid state alteration for this controllable quantity." ;
        rdfs:domain           nc:ControllableQuantity ;
        rdfs:label            "GridStateAlteration"@en ;
        rdfs:range            nc:GridStateAlteration ;
        cims:AssociationUsed  "Yes" ;
        cims:inverseRoleName  nc:GridStateAlteration.ControllableQuantity ;
        cims:multiplicity     cims:M:0..1 ;
        cims:stereotype       "NC" .

nc:ControllableQuantity.RemedialAction
        rdf:type              rdf:Property ;
        rdfs:comment          "Remedial action which is associated with the controllable quantity." ;
        rdfs:domain           nc:ControllableQuantity ;
        rdfs:label            "RemedialAction"@en ;
        rdfs:range            nc:RemedialAction ;
        cims:AssociationUsed  "Yes" ;
        cims:inverseRoleName  nc:RemedialAction.ControllableQuantity ;
        cims:multiplicity     cims:M:0..1 ;
        cims:stereotype       "NC" .

nc:ControllableQuantity.SensitivityFactor
        rdf:type              rdf:Property ;
        rdfs:comment          "The sensitivity factor associated with a controllable quantity." ;
        rdfs:domain           nc:ControllableQuantity ;
        rdfs:label            "SensitivityFactor"@en ;
        rdfs:range            nc:SensitivityFactor ;
        cims:AssociationUsed  "No" ;
        cims:inverseRoleName  nc:SensitivityFactor.ControllableQuantity ;
        cims:multiplicity     cims:M:1..n ;
        cims:stereotype       "NC" .

nc:ControllableQuantity.value
        rdf:type           rdf:Property ;
        rdfs:comment       "The value of the change applied to the grid state alteration or remedial action. In the case of multiple changes or non-quantifiable changes (e.g. Topology changes) the value needs to represent the suitable value that makes the derivable value given in the observable quantity for the purpose of the calculation of the sensitivity factor.  The value can be integer, float or boolean. In case of boolean 1 equals true and 0 equals false." ;
        rdfs:domain        nc:ControllableQuantity ;
        rdfs:label         "value"@en ;
        cims:dataType      cim:Float ;
        cims:multiplicity  cims:M:0..1 ;
        cims:stereotype    "NC" ;
        cims:stereotype    <http://iec.ch/TC57/NonStandard/UML#attribute> .

nc:GridStateAlteration
        rdf:type                rdfs:Class ;
        rdfs:comment            "Grid state alteration is a change of values describing state (operating point) of one element in the grid model compared to the base case." ;
        rdfs:label              "GridStateAlteration"@en ;
        cims:belongsToCategory  sm:Package_SensitivityMatrixProfile ;
        cims:stereotype         "NC" .

nc:GridStateAlteration.ControllableQuantity
        rdf:type              rdf:Property ;
        rdfs:comment          "The controllable quantity associated with this grid state alteration." ;
        rdfs:domain           nc:GridStateAlteration ;
        rdfs:label            "ControllableQuantity"@en ;
        rdfs:range            nc:ControllableQuantity ;
        cims:AssociationUsed  "No" ;
        cims:inverseRoleName  nc:ControllableQuantity.GridStateAlteration ;
        cims:multiplicity     cims:M:0..n ;
        cims:stereotype       "NC" .

nc:ObservableQuantity
        rdf:type                rdfs:Class ;
        rdfs:comment            "Observable quantity is an electrical quantity on an assessed element or an assessed element with contingency." ;
        rdfs:label              "ObservableQuantity"@en ;
        cims:belongsToCategory  sm:Package_SensitivityMatrixProfile ;
        cims:stereotype         "NC" ;
        cims:stereotype         <http://iec.ch/TC57/NonStandard/UML#concrete> .

nc:ObservableQuantity.AssessedElement
        rdf:type              rdf:Property ;
        rdfs:comment          "The assessed element with contingency associated with this observable quantity." ;
        rdfs:domain           nc:ObservableQuantity ;
        rdfs:label            "AssessedElement"@en ;
        rdfs:range            nc:AssessedElement ;
        cims:AssociationUsed  "Yes" ;
        cims:inverseRoleName  nc:AssessedElement.ObservableQuantity ;
        cims:multiplicity     cims:M:1 ;
        cims:stereotype       "NC" .

nc:ObservableQuantity.Contingency
        rdf:type              rdf:Property ;
        rdfs:comment          "The contingency associated with this observable quantity." ;
        rdfs:domain           nc:ObservableQuantity ;
        rdfs:label            "Contingency"@en ;
        rdfs:range            cim:Contingency ;
        cims:AssociationUsed  "Yes" ;
        cims:inverseRoleName  nc:Contingency.ObservableQuantity ;
        cims:multiplicity     cims:M:0..1 ;
        cims:stereotype       "NC" .

nc:ObservableQuantity.SensitivityFactor
        rdf:type              rdf:Property ;
        rdfs:comment          "The sensitivity factor associated with an observable quantity." ;
        rdfs:domain           nc:ObservableQuantity ;
        rdfs:label            "SensitivityFactor"@en ;
        rdfs:range            nc:SensitivityFactor ;
        cims:AssociationUsed  "No" ;
        cims:inverseRoleName  nc:SensitivityFactor.ObservableQuantity ;
        cims:multiplicity     cims:M:1..n ;
        cims:stereotype       "NC" .

nc:ObservableQuantity.observableQuantityKind
        rdf:type           rdf:Property ;
        rdfs:comment       "Kind of observable quantity." ;
        rdfs:domain        nc:ObservableQuantity ;
        rdfs:label         "observableQuantityKind"@en ;
        rdfs:range         nc:ObservableQuantityKind ;
        cims:multiplicity  cims:M:1..1 ;
        cims:stereotype    "NC" ;
        cims:stereotype    <http://iec.ch/TC57/NonStandard/UML#attribute> .

nc:ObservableQuantityKind
        rdf:type                rdfs:Class ;
        rdfs:comment            "Kind of observable quantity." ;
        rdfs:label              "ObservableQuantityKind"@en ;
        cims:belongsToCategory  sm:Package_SensitivityMatrixProfile ;
        cims:stereotype         "NC" ;
        cims:stereotype         <http://iec.ch/TC57/NonStandard/UML#enumeration> .

nc:ObservableQuantityKind.activePower
        rdf:type         nc:ObservableQuantityKind ;
        rdfs:comment     "The observable quantity is the active power." ;
        rdfs:label       "activePower"@en ;
        cims:stereotype  "enum" .

nc:ObservableQuantityKind.reactivePower
        rdf:type         nc:ObservableQuantityKind ;
        rdfs:comment     "The observable quantity is the reactive power." ;
        rdfs:label       "reactivePower"@en ;
        cims:stereotype  "enum" .

nc:ObservableQuantityKind.voltageAngle
        rdf:type         nc:ObservableQuantityKind ;
        rdfs:comment     "The observable quantity is the angle of terminal voltage." ;
        rdfs:label       "voltageAngle"@en ;
        cims:stereotype  "enum" .

nc:ObservableQuantityKind.voltageMagnitude
        rdf:type         nc:ObservableQuantityKind ;
        rdfs:comment     "The observable quantity is the magnitude of terminal voltage." ;
        rdfs:label       "voltageMagnitude"@en ;
        cims:stereotype  "enum" .

nc:RemedialAction  rdf:type     rdfs:Class ;
        rdfs:comment            "Remedial action describes one or more actions that can be performed on a given power system model situation to eliminate one or more identified breaches of constraints. The remedial action can be costly, and have a cost characteristic, or non costly. " ;
        rdfs:label              "RemedialAction"@en ;
        cims:belongsToCategory  sm:Package_SensitivityMatrixProfile ;
        cims:stereotype         "NC" .

nc:RemedialAction.ControllableQuantity
        rdf:type              rdf:Property ;
        rdfs:comment          "The controllable quantity for a remedial action." ;
        rdfs:domain           nc:RemedialAction ;
        rdfs:label            "ControllableQuantity"@en ;
        rdfs:range            nc:ControllableQuantity ;
        cims:AssociationUsed  "No" ;
        cims:inverseRoleName  nc:ControllableQuantity.RemedialAction ;
        cims:multiplicity     cims:M:0..n ;
        cims:stereotype       "NC" .

nc:SensitivityFactor  rdf:type  rdfs:Class ;
        rdfs:comment            "The sensitivity factor which represents the sensitivity between observable and controllable elements. " ;
        rdfs:label              "SensitivityFactor"@en ;
        cims:belongsToCategory  sm:Package_SensitivityMatrixProfile ;
        cims:stereotype         "NC" ;
        cims:stereotype         <http://iec.ch/TC57/NonStandard/UML#concrete> .

nc:SensitivityFactor.ControllableQuantity
        rdf:type              rdf:Property ;
        rdfs:comment          "The controllable quantity for this sensitivity factor." ;
        rdfs:domain           nc:SensitivityFactor ;
        rdfs:label            "ControllableQuantity"@en ;
        rdfs:range            nc:ControllableQuantity ;
        cims:AssociationUsed  "Yes" ;
        cims:inverseRoleName  nc:ControllableQuantity.SensitivityFactor ;
        cims:multiplicity     cims:M:1 ;
        cims:stereotype       "NC" .

nc:SensitivityFactor.ObservableQuantity
        rdf:type              rdf:Property ;
        rdfs:comment          "The observable quantity for this sensitivity factor." ;
        rdfs:domain           nc:SensitivityFactor ;
        rdfs:label            "ObservableQuantity"@en ;
        rdfs:range            nc:ObservableQuantity ;
        cims:AssociationUsed  "Yes" ;
        cims:inverseRoleName  nc:ObservableQuantity.SensitivityFactor ;
        cims:multiplicity     cims:M:1 ;
        cims:stereotype       "NC" .

nc:SensitivityFactor.SensitivityMatrix
        rdf:type              rdf:Property ;
        rdfs:comment          "The sensitivity matrix which contains this sensitivity factor." ;
        rdfs:domain           nc:SensitivityFactor ;
        rdfs:label            "SensitivityMatrix"@en ;
        rdfs:range            nc:SensitivityMatrix ;
        cims:AssociationUsed  "Yes" ;
        cims:inverseRoleName  nc:SensitivityMatrix.SensitivityFactor ;
        cims:multiplicity     cims:M:1 ;
        cims:stereotype       "NC" .

nc:SensitivityFactor.value
        rdf:type           rdf:Property ;
        rdfs:comment       "The value of the sensitivity factor." ;
        rdfs:domain        nc:SensitivityFactor ;
        rdfs:label         "value"@en ;
        cims:dataType      cim:Float ;
        cims:multiplicity  cims:M:1..1 ;
        cims:stereotype    "NC" ;
        cims:stereotype    <http://iec.ch/TC57/NonStandard/UML#attribute> .

nc:SensitivityMatrix  rdf:type  rdfs:Class ;
        rdfs:comment            "The sensitivity matrix which represents the sensitivity factors between observable and controllable elements. " ;
        rdfs:label              "SensitivityMatrix"@en ;
        rdfs:subClassOf         cim:IdentifiedObject ;
        cims:belongsToCategory  sm:Package_SensitivityMatrixProfile ;
        cims:stereotype         "NC" ;
        cims:stereotype         <http://iec.ch/TC57/NonStandard/UML#concrete> .

nc:SensitivityMatrix.SensitivityFactor
        rdf:type              rdf:Property ;
        rdfs:comment          "The sensitivity factor which belongs to this sensitivity matrix." ;
        rdfs:domain           nc:SensitivityMatrix ;
        rdfs:label            "SensitivityFactor"@en ;
        rdfs:range            nc:SensitivityFactor ;
        cims:AssociationUsed  "No" ;
        cims:inverseRoleName  nc:SensitivityFactor.SensitivityMatrix ;
        cims:multiplicity     cims:M:1..n ;
        cims:stereotype       "NC" .

nc:SensitivityMatrix.kind
        rdf:type           rdf:Property ;
        rdfs:comment       "The kind of sensitivity matrix. " ;
        rdfs:domain        nc:SensitivityMatrix ;
        rdfs:label         "kind"@en ;
        rdfs:range         nc:SensitivityMatrixKind ;
        cims:multiplicity  cims:M:1..1 ;
        cims:stereotype    "NC" ;
        cims:stereotype    <http://iec.ch/TC57/NonStandard/UML#attribute> .

nc:SensitivityMatrixKind
        rdf:type                rdfs:Class ;
        rdfs:comment            "Kinds of sensitivity matrix." ;
        rdfs:label              "SensitivityMatrixKind"@en ;
        cims:belongsToCategory  sm:Package_SensitivityMatrixProfile ;
        cims:stereotype         "NC" ;
        cims:stereotype         <http://iec.ch/TC57/NonStandard/UML#enumeration> .

nc:SensitivityMatrixKind.other
        rdf:type         nc:SensitivityMatrixKind ;
        rdfs:comment     "Other kind of sensitivity matrix." ;
        rdfs:label       "other"@en ;
        cims:stereotype  "enum" .

nc:SensitivityMatrixKind.uniformLoad
        rdf:type         nc:SensitivityMatrixKind ;
        rdfs:comment     "Uniform load matrix." ;
        rdfs:label       "uniformLoad"@en ;
        cims:stereotype  "enum" .

nc:SensitivityMatrixKind.uniformNode
        rdf:type         nc:SensitivityMatrixKind ;
        rdfs:comment     "Uniform node matrix." ;
        rdfs:label       "uniformNode"@en ;
        cims:stereotype  "enum" .

nc:SensitivityMatrixKind.zoneToSlack
        rdf:type         nc:SensitivityMatrixKind ;
        rdfs:comment     "Zone to slack kind of sensitivity matrix." ;
        rdfs:label       "zoneToSlack"@en ;
        cims:stereotype  "enum" .

profcim:IRI  rdf:type           rdfs:Class ;
        rdfs:comment            "An IRI (Internationalized Resource Identifier) within an RDF graph is a Unicode string that conforms to the syntax defined in RFC 3987.\nThe primitive is serialized as rdf:resource in RDFXML.\nIRIs in the RDF abstract syntax must be absolute, and may contain a fragment identifier.\nIRI equality: Two IRIs are equal if and only if they are equivalent under Simple String Comparison according to section 5.1 of [RFC3987]. Further normalization must not be performed when comparing IRIs for equality.\nIRIs are a generalization of URIs [RFC3986] that permits a wider range of Unicode characters. Every absolute URI and URL is an IRI, but not every IRI is an URI. When IRIs are used in operations that are only defined for URIs, they must first be converted according to the mapping defined in section 3.1 of [RFC3987]. A notable example is retrieval over the HTTP protocol. The mapping involves UTF-8 encoding of non-ASCII characters, %-encoding of octets not allowed in URIs, and Punycode-encoding of domain names." ;
        rdfs:label              "IRI"@en ;
        cims:belongsToCategory  sm:Package_DocSensitivityMatrixProfile ;
        cims:stereotype         "profcim" , "Primitive" .
profcim:StringFixedLanguage
        rdf:type                rdfs:Class ;
        rdfs:comment            "A string consisting of a sequence of characters. The character encoding is UTF-8. The string length is unspecified and unlimited.\nThe primitive is serialized as literal without language support." ;
        rdfs:label              "StringFixedLanguage"@en ;
        cims:belongsToCategory  sm:Package_DocSensitivityMatrixProfile ;
        cims:stereotype         "profcim" , "Primitive" .

profcim:StringIRI  rdf:type     rdfs:Class ;
        rdfs:comment            "An IRI (Internationalized Resource Identifier) within an RDF graph is a Unicode string that conforms to the syntax defined in RFC 3987.\nThe primitive is serialized as literal without language support.\nIRIs in the RDF abstract syntax must be absolute, and may contain a fragment identifier.\nIRI equality: Two IRIs are equal if and only if they are equivalent under Simple String Comparison according to section 5.1 of [RFC3987]. Further normalization must not be performed when comparing IRIs for equality.\nIRIs are a generalization of URIs [RFC3986] that permits a wider range of Unicode characters. Every absolute URI and URL is an IRI, but not every IRI is an URI. When IRIs are used in operations that are only defined for URIs, they must first be converted according to the mapping defined in section 3.1 of [RFC3987]. A notable example is retrieval over the HTTP protocol. The mapping involves UTF-8 encoding of non-ASCII characters, %-encoding of octets not allowed in URIs, and Punycode-encoding of domain names." ;
        rdfs:label              "StringIRI"@en ;
        cims:belongsToCategory  sm:Package_DocSensitivityMatrixProfile ;
        cims:stereotype         "profcim" , "Primitive" .

profcim:URL  rdf:type           rdfs:Class ;
        rdfs:comment            "A Uniform Resource Locator (URL), colloquially termed a web address, is a reference to a web resource that specifies its location on a computer network and a mechanism for retrieving it. A URL is a specific type of Uniform Resource Identifier (URI), although many people use the two terms interchangeably.URLs occur most commonly to reference web pages (http), but are also used for file transfer (ftp), email (mailto), database access (JDBC), and many other applications." ;
        rdfs:label              "URL"@en ;
        cims:belongsToCategory  sm:Package_DocSensitivityMatrixProfile ;
        cims:stereotype         "profcim" , "Primitive" .

sm:Ontology  rdf:type         owl:Ontology ;
        dcterms:conformsTo    "file://iec61970cim17v40_iec61968cim13v13a_iec62325cim03v17a.eap" , "urn:iso:std:iec:61970-401:draft:ed-1" , "urn:iso:std:iec:61970-501:draft:ed-2" , "urn:iso:std:iec:61970-301:ed-7:amd1" , "urn:iso:std:iec:61970-600-2:ed-1" , "file://CIM100_CGMES31v01_501-20v02_NC23v62_MM10v01.eap" ;
        dcterms:creator       "ENTSO-E CIM WG NC project"@en ;
        dcterms:description   "This vocabulary is describing the sensitivity matrix."@en ;
        dcterms:identifier    "urn:uuid:d89a8510-528b-49a9-81f1-c51be51caa6f" ;
        dcterms:language      "en-GB" ;
        dcterms:license       "https://www.apache.org/licenses/LICENSE-2.0"@en ;
        dcterms:modified      "2024-03-20"^^<http://www.w3.org/2001/XMLSchema#date> ;
        dcterms:publisher     "ENTSO-E"@en ;
        dcterms:rightsHolder  "ENTSO-E"@en ;
        dcterms:title         "Sensitivity Matrix Vocabulary"@en ;
        owl:priorVersion      <http://entsoe.eu/ns/CIM/SensitivityMatrix-EU/2.2> ;
        owl:versionIRI        <https://ap.cim4.eu/SensitivityMatrix/2.3> ;
        owl:versionInfo       "2.3.0"@en ;
        dcat:keyword          "SM" ;
        dcat:theme            "vocabulary"@en .

sm:Package_DocSensitivityMatrixProfile
        rdf:type      cims:ClassCategory ;
        rdfs:comment  "This package contains datatypes used only in the RDFS header." ;
        rdfs:label    "DocSensitivityMatrixProfile"@en .

sm:Package_SensitivityMatrixProfile
        rdf:type      cims:ClassCategory ;
        rdfs:comment  "This package contains sensitivity matrix profile." ;
        rdfs:label    "SensitivityMatrixProfile"@en .

