@prefix cim:     <https://cim.ucaiug.io/ns#> .
@prefix cims:    <http://iec.ch/TC57/1999/rdf-schema-extensions-19990926#> .
@prefix dcat:    <http://www.w3.org/ns/dcat#> .
@prefix dcterms: <http://purl.org/dc/terms/#> .
@prefix nc:      <https://cim4.eu/ns/nc#> .
@prefix owl:     <http://www.w3.org/2002/07/owl#> .
@prefix profcim: <https://cim.ucaiug.io/ns/prof-cim#> .
@prefix rdf:     <http://www.w3.org/1999/02/22-rdf-syntax-ns#> .
@prefix rdfs:    <http://www.w3.org/2000/01/rdf-schema#> .
@prefix shs:     <https://ap.cim4.eu/SteadyStateHypothesisSchedule#> .

cim:ActivePower  rdf:type       rdfs:Class ;
        rdfs:comment            "Product of RMS value of the voltage and the RMS value of the in-phase component of the current." ;
        rdfs:label              "ActivePower"@en ;
        cims:belongsToCategory  shs:Package_SteadyStateHypothesisScheduleProfile ;
        cims:stereotype         "CIMDatatype" .

cim:ActivePower.multiplier
        rdf:type           rdf:Property ;
        rdfs:domain        cim:ActivePower ;
        rdfs:label         "multiplier"@en ;
        rdfs:range         cim:UnitMultiplier ;
        cims:isFixed       "M" ;
        cims:multiplicity  cims:M:0..1 ;
        cims:stereotype    <http://iec.ch/TC57/NonStandard/UML#attribute> .

cim:ActivePower.unit  rdf:type  rdf:Property ;
        rdfs:domain        cim:ActivePower ;
        rdfs:label         "unit"@en ;
        rdfs:range         cim:UnitSymbol ;
        cims:isFixed       "W" ;
        cims:multiplicity  cims:M:0..1 ;
        cims:stereotype    <http://iec.ch/TC57/NonStandard/UML#attribute> .

cim:ActivePower.value
        rdf:type           rdf:Property ;
        rdfs:domain        cim:ActivePower ;
        rdfs:label         "value"@en ;
        cims:dataType      cim:Float ;
        cims:multiplicity  cims:M:0..1 ;
        cims:stereotype    <http://iec.ch/TC57/NonStandard/UML#attribute> .

cim:ActivePowerLimit  rdf:type  rdfs:Class ;
        rdfs:comment            "Limit on active power flow." ;
        rdfs:label              "ActivePowerLimit"@en ;
        cims:belongsToCategory  shs:Package_SteadyStateHypothesisScheduleProfile .

cim:AngleDegrees  rdf:type      rdfs:Class ;
        rdfs:comment            "Measurement of angle in degrees." ;
        rdfs:label              "AngleDegrees"@en ;
        cims:belongsToCategory  shs:Package_SteadyStateHypothesisScheduleProfile ;
        cims:stereotype         "CIMDatatype" .

cim:AngleDegrees.multiplier
        rdf:type           rdf:Property ;
        rdfs:domain        cim:AngleDegrees ;
        rdfs:label         "multiplier"@en ;
        rdfs:range         cim:UnitMultiplier ;
        cims:isFixed       "none" ;
        cims:multiplicity  cims:M:0..1 ;
        cims:stereotype    <http://iec.ch/TC57/NonStandard/UML#attribute> .

cim:AngleDegrees.unit
        rdf:type           rdf:Property ;
        rdfs:domain        cim:AngleDegrees ;
        rdfs:label         "unit"@en ;
        rdfs:range         cim:UnitSymbol ;
        cims:isFixed       "deg" ;
        cims:multiplicity  cims:M:0..1 ;
        cims:stereotype    <http://iec.ch/TC57/NonStandard/UML#attribute> .

cim:AngleDegrees.value
        rdf:type           rdf:Property ;
        rdfs:domain        cim:AngleDegrees ;
        rdfs:label         "value"@en ;
        cims:dataType      cim:Float ;
        cims:multiplicity  cims:M:0..1 ;
        cims:stereotype    <http://iec.ch/TC57/NonStandard/UML#attribute> .

cim:ApparentPower  rdf:type     rdfs:Class ;
        rdfs:comment            "Product of the RMS value of the voltage and the RMS value of the current." ;
        rdfs:label              "ApparentPower"@en ;
        cims:belongsToCategory  shs:Package_SteadyStateHypothesisScheduleProfile ;
        cims:stereotype         "CIMDatatype" .

cim:ApparentPower.multiplier
        rdf:type           rdf:Property ;
        rdfs:domain        cim:ApparentPower ;
        rdfs:label         "multiplier"@en ;
        rdfs:range         cim:UnitMultiplier ;
        cims:isFixed       "M" ;
        cims:multiplicity  cims:M:0..1 ;
        cims:stereotype    <http://iec.ch/TC57/NonStandard/UML#attribute> .

cim:ApparentPower.unit
        rdf:type           rdf:Property ;
        rdfs:domain        cim:ApparentPower ;
        rdfs:label         "unit"@en ;
        rdfs:range         cim:UnitSymbol ;
        cims:isFixed       "VA" ;
        cims:multiplicity  cims:M:0..1 ;
        cims:stereotype    <http://iec.ch/TC57/NonStandard/UML#attribute> .

cim:ApparentPower.value
        rdf:type           rdf:Property ;
        rdfs:domain        cim:ApparentPower ;
        rdfs:label         "value"@en ;
        cims:dataType      cim:Float ;
        cims:multiplicity  cims:M:0..1 ;
        cims:stereotype    <http://iec.ch/TC57/NonStandard/UML#attribute> .

cim:ApparentPowerLimit
        rdf:type                rdfs:Class ;
        rdfs:comment            "Apparent power limit." ;
        rdfs:label              "ApparentPowerLimit"@en ;
        cims:belongsToCategory  shs:Package_SteadyStateHypothesisScheduleProfile .

cim:AsynchronousMachine
        rdf:type                rdfs:Class ;
        rdfs:comment            "A rotating machine whose shaft rotates asynchronously with the electrical field.  Also known as an induction machine with no external connection to the rotor windings, e.g. squirrel-cage induction machine." ;
        rdfs:label              "AsynchronousMachine"@en ;
        cims:belongsToCategory  shs:Package_SteadyStateHypothesisScheduleProfile .

cim:AsynchronousMachineKind
        rdf:type                rdfs:Class ;
        rdfs:comment            "Kind of Asynchronous Machine." ;
        rdfs:label              "AsynchronousMachineKind"@en ;
        cims:belongsToCategory  shs:Package_SteadyStateHypothesisScheduleProfile ;
        cims:stereotype         <http://iec.ch/TC57/NonStandard/UML#enumeration> .

cim:AsynchronousMachineKind.generator
        rdf:type         cim:AsynchronousMachineKind ;
        rdfs:comment     "The Asynchronous Machine is a generator." ;
        rdfs:label       "generator"@en ;
        cims:stereotype  "enum" .

cim:AsynchronousMachineKind.motor
        rdf:type         cim:AsynchronousMachineKind ;
        rdfs:comment     "The Asynchronous Machine is a motor." ;
        rdfs:label       "motor"@en ;
        cims:stereotype  "enum" .

cim:BatteryStateKind  rdf:type  rdfs:Class ;
        rdfs:comment            "The state of the battery unit." ;
        rdfs:label              "BatteryStateKind"@en ;
        cims:belongsToCategory  shs:Package_SteadyStateHypothesisScheduleProfile ;
        cims:stereotype         <http://iec.ch/TC57/NonStandard/UML#enumeration> .

cim:BatteryStateKind.charging
        rdf:type         cim:BatteryStateKind ;
        rdfs:comment     "Stored energy is increasing." ;
        rdfs:label       "charging"@en ;
        cims:stereotype  "enum" .

cim:BatteryStateKind.discharging
        rdf:type         cim:BatteryStateKind ;
        rdfs:comment     "Stored energy is decreasing." ;
        rdfs:label       "discharging"@en ;
        cims:stereotype  "enum" .

cim:BatteryStateKind.empty
        rdf:type         cim:BatteryStateKind ;
        rdfs:comment     "Unable to discharge, and not charging." ;
        rdfs:label       "empty"@en ;
        cims:stereotype  "enum" .

cim:BatteryStateKind.full
        rdf:type         cim:BatteryStateKind ;
        rdfs:comment     "Unable to charge, and not discharging." ;
        rdfs:label       "full"@en ;
        cims:stereotype  "enum" .

cim:BatteryStateKind.waiting
        rdf:type         cim:BatteryStateKind ;
        rdfs:comment     "Neither charging nor discharging, but able to do so." ;
        rdfs:label       "waiting"@en ;
        cims:stereotype  "enum" .

cim:BatteryUnit  rdf:type       rdfs:Class ;
        rdfs:comment            "An electrochemical energy storage device." ;
        rdfs:label              "BatteryUnit"@en ;
        cims:belongsToCategory  shs:Package_SteadyStateHypothesisScheduleProfile .

cim:Boolean  rdf:type           rdfs:Class ;
        rdfs:comment            "A type with the value space \"true\" and \"false\"." ;
        rdfs:label              "Boolean"@en ;
        cims:belongsToCategory  shs:Package_SteadyStateHypothesisScheduleProfile ;
        cims:stereotype         "Primitive" .

cim:ControlArea  rdf:type       rdfs:Class ;
        rdfs:comment            "A control area is a grouping of generating units and/or loads and a cutset of tie lines (as terminals) which may be used for a variety of purposes including automatic generation control, power flow solution area interchange control specification, and input to load forecasting. All generation and load within the area defined by the terminals on the border are considered in the area interchange control. Note that any number of overlapping control area specifications can be superimposed on the physical model. The following general principles apply to ControlArea:\n1.  The control area orientation for net interchange is positive for an import, negative for an export.\n2.  The control area net interchange is determined by summing flows in Terminals. The Terminals are identified by creating a set of TieFlow objects associated with a ControlArea object. Each TieFlow object identifies one Terminal.\n3.  In a single network model, a tie between two control areas must be modelled in both control area specifications, such that the two representations of the tie flow sum to zero.\n4.  The normal orientation of Terminal flow is positive for flow into the conducting equipment that owns the Terminal. (i.e. flow from a bus into a device is positive.) However, the orientation of each flow in the control area specification must align with the control area convention, i.e. import is positive. If the orientation of the Terminal flow referenced by a TieFlow is positive into the control area, then this is confirmed by setting TieFlow.positiveFlowIn flag TRUE. If not, the orientation must be reversed by setting the TieFlow.positiveFlowIn flag FALSE." ;
        rdfs:label              "ControlArea"@en ;
        cims:belongsToCategory  shs:Package_SteadyStateHypothesisScheduleProfile .

cim:CsConverter  rdf:type       rdfs:Class ;
        rdfs:comment            "DC side of the current source converter (CSC).\nThe firing angle controls the dc voltage at the converter, both for rectifier and inverter. The difference between the dc voltages of the rectifier and inverter determines the dc current. The extinction angle is used to limit the dc voltage at the inverter, if needed, and is not used in active power control. The firing angle, transformer tap position and number of connected filters are the primary means to control a current source dc line. Higher level controls are built on top, e.g. dc voltage, dc current and active power. From a steady state perspective it is sufficient to specify the wanted active power transfer (ACDCConverter.targetPpcc) and the control functions will set the dc voltage, dc current, firing angle, transformer tap position and number of connected filters to meet this. Therefore attributes targetAlpha and targetGamma are not applicable in this case.\nThe reactive power consumed by the converter is a function of the firing angle, transformer tap position and number of connected filter, which can be approximated with half of the active power. The losses is a function of the dc voltage and dc current.\nThe attributes minAlpha and maxAlpha define the range of firing angles for rectifier operation between which no discrete tap changer action takes place. The range is typically 10-18 degrees.\nThe attributes minGamma and maxGamma define the range of extinction angles for inverter operation between which no discrete tap changer action takes place. The range is typically 17-20 degrees." ;
        rdfs:label              "CsConverter"@en ;
        cims:belongsToCategory  shs:Package_SteadyStateHypothesisScheduleProfile .

cim:CsOperatingModeKind
        rdf:type                rdfs:Class ;
        rdfs:comment            "Operating mode for HVDC line operating as Current Source Converter." ;
        rdfs:label              "CsOperatingModeKind"@en ;
        cims:belongsToCategory  shs:Package_SteadyStateHypothesisScheduleProfile ;
        cims:stereotype         <http://iec.ch/TC57/NonStandard/UML#enumeration> .

cim:CsOperatingModeKind.inverter
        rdf:type         cim:CsOperatingModeKind ;
        rdfs:comment     "Operating as inverter, which is the power receiving end." ;
        rdfs:label       "inverter"@en ;
        cims:stereotype  "enum" .

cim:CsOperatingModeKind.rectifier
        rdf:type         cim:CsOperatingModeKind ;
        rdfs:comment     "Operating as rectifier, which is the power sending end." ;
        rdfs:label       "rectifier"@en ;
        cims:stereotype  "enum" .

cim:CsPpccControlKind
        rdf:type                rdfs:Class ;
        rdfs:comment            "Active power control modes for HVDC line operating as Current Source Converter." ;
        rdfs:label              "CsPpccControlKind"@en ;
        cims:belongsToCategory  shs:Package_SteadyStateHypothesisScheduleProfile ;
        cims:stereotype         <http://iec.ch/TC57/NonStandard/UML#enumeration> .

cim:CsPpccControlKind.activePower
        rdf:type         cim:CsPpccControlKind ;
        rdfs:comment     "Control is active power control at AC side, at point of common coupling. Target is provided by ACDCConverter.targetPpcc." ;
        rdfs:label       "activePower"@en ;
        cims:stereotype  "enum" .

cim:CsPpccControlKind.dcCurrent
        rdf:type         cim:CsPpccControlKind ;
        rdfs:comment     "Control is DC current  with target value provided by CsConverter.targetIdc." ;
        rdfs:label       "dcCurrent"@en ;
        cims:stereotype  "enum" .

cim:CsPpccControlKind.dcVoltage
        rdf:type         cim:CsPpccControlKind ;
        rdfs:comment     "Control is DC voltage  with target value provided by ACDCConverter.targetUdc." ;
        rdfs:label       "dcVoltage"@en ;
        cims:stereotype  "enum" .

cim:CurrentFlow  rdf:type       rdfs:Class ;
        rdfs:comment            "Electrical current with sign convention: positive flow is out of the conducting equipment into the connectivity node. Can be both AC and DC." ;
        rdfs:label              "CurrentFlow"@en ;
        cims:belongsToCategory  shs:Package_SteadyStateHypothesisScheduleProfile ;
        cims:stereotype         "CIMDatatype" .

cim:CurrentFlow.multiplier
        rdf:type           rdf:Property ;
        rdfs:domain        cim:CurrentFlow ;
        rdfs:label         "multiplier"@en ;
        rdfs:range         cim:UnitMultiplier ;
        cims:isFixed       "none" ;
        cims:multiplicity  cims:M:0..1 ;
        cims:stereotype    <http://iec.ch/TC57/NonStandard/UML#attribute> .

cim:CurrentFlow.unit  rdf:type  rdf:Property ;
        rdfs:domain        cim:CurrentFlow ;
        rdfs:label         "unit"@en ;
        rdfs:range         cim:UnitSymbol ;
        cims:isFixed       "A" ;
        cims:multiplicity  cims:M:0..1 ;
        cims:stereotype    <http://iec.ch/TC57/NonStandard/UML#attribute> .

cim:CurrentFlow.value
        rdf:type           rdf:Property ;
        rdfs:domain        cim:CurrentFlow ;
        rdfs:label         "value"@en ;
        cims:dataType      cim:Float ;
        cims:multiplicity  cims:M:0..1 ;
        cims:stereotype    <http://iec.ch/TC57/NonStandard/UML#attribute> .

cim:CurrentLimit  rdf:type      rdfs:Class ;
        rdfs:comment            "Operational limit on current. " ;
        rdfs:label              "CurrentLimit"@en ;
        cims:belongsToCategory  shs:Package_SteadyStateHypothesisScheduleProfile .

cim:Date  rdf:type              rdfs:Class ;
        rdfs:comment            "Date as \"yyyy-mm-dd\", which conforms with ISO 8601. UTC time zone is specified as \"yyyy-mm-ddZ\". A local timezone relative UTC is specified as \"yyyy-mm-dd(+/-)hh:mm\"." ;
        rdfs:label              "Date"@en ;
        cims:belongsToCategory  shs:Package_DocSteadyStateHypothesisScheduleProfile ;
        cims:stereotype         "Primitive" .

cim:DateTime  rdf:type          rdfs:Class ;
        rdfs:comment            "Date and time as \"yyyy-mm-ddThh:mm:ss.sss\", which conforms with ISO 8601. UTC time zone is specified as \"yyyy-mm-ddThh:mm:ss.sssZ\". A local timezone relative UTC is specified as \"yyyy-mm-ddThh:mm:ss.sss-hh:mm\". The second component (shown here as \"ss.sss\") could have any number of digits in its fractional part to allow any kind of precision beyond seconds." ;
        rdfs:label              "DateTime"@en ;
        cims:belongsToCategory  shs:Package_SteadyStateHypothesisScheduleProfile ;
        cims:stereotype         "Primitive" .

cim:EnergyConnection  rdf:type  rdfs:Class ;
        rdfs:comment            "A connection of energy generation or consumption on the power system model." ;
        rdfs:label              "EnergyConnection"@en ;
        cims:belongsToCategory  shs:Package_SteadyStateHypothesisScheduleProfile .

cim:Equipment  rdf:type         rdfs:Class ;
        rdfs:comment            "The parts of a power system that are physical devices, electronic or mechanical." ;
        rdfs:label              "Equipment"@en ;
        cims:belongsToCategory  shs:Package_SteadyStateHypothesisScheduleProfile .

cim:EquivalentInjection
        rdf:type                rdfs:Class ;
        rdfs:comment            "This class represents equivalent injections (generation or load).  Voltage regulation is allowed only at the point of connection." ;
        rdfs:label              "EquivalentInjection"@en ;
        cims:belongsToCategory  shs:Package_SteadyStateHypothesisScheduleProfile .

cim:ExternalNetworkInjection
        rdf:type                rdfs:Class ;
        rdfs:comment            "This class represents the external network and it is used for IEC 60909 calculations." ;
        rdfs:label              "ExternalNetworkInjection"@en ;
        cims:belongsToCategory  shs:Package_SteadyStateHypothesisScheduleProfile .

cim:Float  rdf:type             rdfs:Class ;
        rdfs:comment            "A floating point number. The range is unspecified and not limited." ;
        rdfs:label              "Float"@en ;
        cims:belongsToCategory  shs:Package_SteadyStateHypothesisScheduleProfile ;
        cims:stereotype         "Primitive" .

cim:GeneratingUnit  rdf:type    rdfs:Class ;
        rdfs:comment            "A single or set of synchronous machines for converting mechanical power into alternating-current power. For example, individual machines within a set may be defined for scheduling purposes while a single control signal is derived for the set. In this case there would be a GeneratingUnit for each member of the set and an additional GeneratingUnit corresponding to the set." ;
        rdfs:label              "GeneratingUnit"@en ;
        cims:belongsToCategory  shs:Package_SteadyStateHypothesisScheduleProfile .

cim:IdentifiedObject  rdf:type  rdfs:Class ;
        rdfs:comment            "This is a root class to provide common identification for all classes needing identification and naming attributes." ;
        rdfs:label              "IdentifiedObject"@en ;
        cims:belongsToCategory  shs:Package_SteadyStateHypothesisScheduleProfile .

cim:IdentifiedObject.description
        rdf:type           rdf:Property ;
        rdfs:comment       "The description is a free human readable text describing or naming the object. It may be non unique and may not correlate to a naming hierarchy." ;
        rdfs:domain        cim:IdentifiedObject ;
        rdfs:label         "description"@en ;
        cims:dataType      cim:String ;
        cims:multiplicity  cims:M:0..1 ;
        cims:stereotype    <http://iec.ch/TC57/NonStandard/UML#attribute> .

cim:IdentifiedObject.mRID
        rdf:type           rdf:Property ;
        rdfs:comment       "Master resource identifier issued by a model authority. The mRID is unique within an exchange context. Global uniqueness is easily achieved by using a UUID, as specified in RFC 4122, for the mRID. The use of UUID is strongly recommended.\nFor CIMXML data files in RDF syntax conforming to IEC 61970-552, the mRID is mapped to rdf:ID or rdf:about attributes that identify CIM object elements." ;
        rdfs:domain        cim:IdentifiedObject ;
        rdfs:label         "mRID"@en ;
        cims:dataType      cim:String ;
        cims:multiplicity  cims:M:1..1 ;
        cims:stereotype    <http://iec.ch/TC57/NonStandard/UML#attribute> .

cim:IdentifiedObject.name
        rdf:type           rdf:Property ;
        rdfs:comment       "The name is any free human readable and possibly non unique text naming the object." ;
        rdfs:domain        cim:IdentifiedObject ;
        rdfs:label         "name"@en ;
        cims:dataType      cim:String ;
        cims:multiplicity  cims:M:1..1 ;
        cims:stereotype    <http://iec.ch/TC57/NonStandard/UML#attribute> .

cim:Integer  rdf:type           rdfs:Class ;
        rdfs:comment            "An integer number. The range is unspecified and not limited." ;
        rdfs:label              "Integer"@en ;
        cims:belongsToCategory  shs:Package_SteadyStateHypothesisScheduleProfile ;
        cims:stereotype         "Primitive" .

cim:MonthDay  rdf:type          rdfs:Class ;
        rdfs:comment            "MonthDay format as \"--mm-dd\", which conforms with XSD data type gMonthDay." ;
        rdfs:label              "MonthDay"@en ;
        cims:belongsToCategory  shs:Package_SteadyStateHypothesisScheduleProfile ;
        cims:stereotype         "Primitive" .

cim:PU  rdf:type                rdfs:Class ;
        rdfs:comment            "Per Unit - a positive or negative value referred to a defined base. Values typically range from -10 to +10." ;
        rdfs:label              "PU"@en ;
        cims:belongsToCategory  shs:Package_SteadyStateHypothesisScheduleProfile ;
        cims:stereotype         "CIMDatatype" .

cim:PU.multiplier  rdf:type  rdf:Property ;
        rdfs:domain        cim:PU ;
        rdfs:label         "multiplier"@en ;
        rdfs:range         cim:UnitMultiplier ;
        cims:isFixed       "none" ;
        cims:multiplicity  cims:M:0..1 ;
        cims:stereotype    <http://iec.ch/TC57/NonStandard/UML#attribute> .

cim:PU.unit  rdf:type      rdf:Property ;
        rdfs:domain        cim:PU ;
        rdfs:label         "unit"@en ;
        rdfs:range         cim:UnitSymbol ;
        cims:isFixed       "none" ;
        cims:multiplicity  cims:M:0..1 ;
        cims:stereotype    <http://iec.ch/TC57/NonStandard/UML#attribute> .

cim:PU.value  rdf:type     rdf:Property ;
        rdfs:domain        cim:PU ;
        rdfs:label         "value"@en ;
        cims:dataType      cim:Float ;
        cims:multiplicity  cims:M:0..1 ;
        cims:stereotype    <http://iec.ch/TC57/NonStandard/UML#attribute> .

cim:PerCent  rdf:type           rdfs:Class ;
        rdfs:comment            "Percentage on a defined base.   For example, specify as 100 to indicate at the defined base." ;
        rdfs:label              "PerCent"@en ;
        cims:belongsToCategory  shs:Package_SteadyStateHypothesisScheduleProfile ;
        cims:stereotype         "CIMDatatype" .

cim:PerCent.multiplier
        rdf:type           rdf:Property ;
        rdfs:domain        cim:PerCent ;
        rdfs:label         "multiplier"@en ;
        rdfs:range         cim:UnitMultiplier ;
        cims:isFixed       "none" ;
        cims:multiplicity  cims:M:0..1 ;
        cims:stereotype    <http://iec.ch/TC57/NonStandard/UML#attribute> .

cim:PerCent.unit  rdf:type  rdf:Property ;
        rdfs:domain        cim:PerCent ;
        rdfs:label         "unit"@en ;
        rdfs:range         cim:UnitSymbol ;
        cims:isFixed       "none" ;
        cims:multiplicity  cims:M:0..1 ;
        cims:stereotype    <http://iec.ch/TC57/NonStandard/UML#attribute> .

cim:PerCent.value  rdf:type  rdf:Property ;
        rdfs:comment       "Normally 0 to 100 on a defined base." ;
        rdfs:domain        cim:PerCent ;
        rdfs:label         "value"@en ;
        cims:dataType      cim:Float ;
        cims:multiplicity  cims:M:0..1 ;
        cims:stereotype    <http://iec.ch/TC57/NonStandard/UML#attribute> .

cim:ReactivePower  rdf:type     rdfs:Class ;
        rdfs:comment            "Product of RMS value of the voltage and the RMS value of the quadrature component of the current." ;
        rdfs:label              "ReactivePower"@en ;
        cims:belongsToCategory  shs:Package_SteadyStateHypothesisScheduleProfile ;
        cims:stereotype         "CIMDatatype" .

cim:ReactivePower.multiplier
        rdf:type           rdf:Property ;
        rdfs:domain        cim:ReactivePower ;
        rdfs:label         "multiplier"@en ;
        rdfs:range         cim:UnitMultiplier ;
        cims:isFixed       "M" ;
        cims:multiplicity  cims:M:0..1 ;
        cims:stereotype    <http://iec.ch/TC57/NonStandard/UML#attribute> .

cim:ReactivePower.unit
        rdf:type           rdf:Property ;
        rdfs:domain        cim:ReactivePower ;
        rdfs:label         "unit"@en ;
        rdfs:range         cim:UnitSymbol ;
        cims:isFixed       "VAr" ;
        cims:multiplicity  cims:M:0..1 ;
        cims:stereotype    <http://iec.ch/TC57/NonStandard/UML#attribute> .

cim:ReactivePower.value
        rdf:type           rdf:Property ;
        rdfs:domain        cim:ReactivePower ;
        rdfs:label         "value"@en ;
        cims:dataType      cim:Float ;
        cims:multiplicity  cims:M:0..1 ;
        cims:stereotype    <http://iec.ch/TC57/NonStandard/UML#attribute> .

cim:RealEnergy  rdf:type        rdfs:Class ;
        rdfs:comment            "Real electrical energy." ;
        rdfs:label              "RealEnergy"@en ;
        cims:belongsToCategory  shs:Package_SteadyStateHypothesisScheduleProfile ;
        cims:stereotype         "CIMDatatype" .

cim:RealEnergy.multiplier
        rdf:type           rdf:Property ;
        rdfs:domain        cim:RealEnergy ;
        rdfs:label         "multiplier"@en ;
        rdfs:range         cim:UnitMultiplier ;
        cims:isFixed       "M" ;
        cims:multiplicity  cims:M:0..1 ;
        cims:stereotype    <http://iec.ch/TC57/NonStandard/UML#attribute> .

cim:RealEnergy.unit  rdf:type  rdf:Property ;
        rdfs:domain        cim:RealEnergy ;
        rdfs:label         "unit"@en ;
        rdfs:range         cim:UnitSymbol ;
        cims:isFixed       "Wh" ;
        cims:multiplicity  cims:M:0..1 ;
        cims:stereotype    <http://iec.ch/TC57/NonStandard/UML#attribute> .

cim:RealEnergy.value  rdf:type  rdf:Property ;
        rdfs:domain        cim:RealEnergy ;
        rdfs:label         "value"@en ;
        cims:dataType      cim:Float ;
        cims:multiplicity  cims:M:0..1 ;
        cims:stereotype    <http://iec.ch/TC57/NonStandard/UML#attribute> .

cim:RegulatingControl
        rdf:type                rdfs:Class ;
        rdfs:comment            "Specifies a set of equipment that works together to control a power system quantity such as voltage or flow. \nRemote bus voltage control is possible by specifying the controlled terminal located at some place remote from the controlling equipment.\nThe specified terminal shall be associated with the connectivity node of the controlled point.  The most specific subtype of RegulatingControl shall be used in case such equipment participate in the control, e.g. TapChangerControl for tap changers.\nFor flow control, load sign convention is used, i.e. positive sign means flow out from a TopologicalNode (bus) into the conducting equipment.\nThe attribute minAllowedTargetValue and maxAllowedTargetValue are required in the following cases:\n- For a power generating module operated in power factor control mode to specify maximum and minimum power factor values;\n- Whenever it is necessary to have an off center target voltage for the tap changer regulator. For instance, due to long cables to off shore wind farms and the need to have a simpler setup at the off shore transformer platform, the voltage is controlled from the land at the connection point for the off shore wind farm. Since there usually is a voltage rise along the cable, there is typical and overvoltage of up 3-4 kV compared to the on shore station. Thus in normal operation the tap changer on the on shore station is operated with a target set point, which is in the lower parts of the dead band.\nThe attributes minAllowedTargetValue and maxAllowedTargetValue are not related to the attribute targetDeadband and thus they are not treated as an alternative of the targetDeadband. They are needed due to limitations in the local substation controller. The attribute targetDeadband is used to prevent the power flow from move the tap position in circles (hunting) that is to be used regardless of the attributes minAllowedTargetValue and maxAllowedTargetValue." ;
        rdfs:label              "RegulatingControl"@en ;
        cims:belongsToCategory  shs:Package_SteadyStateHypothesisScheduleProfile .

cim:Resistance  rdf:type        rdfs:Class ;
        rdfs:comment            "Resistance (real part of impedance)." ;
        rdfs:label              "Resistance"@en ;
        cims:belongsToCategory  shs:Package_SteadyStateHypothesisScheduleProfile ;
        cims:stereotype         "CIMDatatype" .

cim:Resistance.multiplier
        rdf:type           rdf:Property ;
        rdfs:domain        cim:Resistance ;
        rdfs:label         "multiplier"@en ;
        rdfs:range         cim:UnitMultiplier ;
        cims:isFixed       "none" ;
        cims:multiplicity  cims:M:0..1 ;
        cims:stereotype    <http://iec.ch/TC57/NonStandard/UML#attribute> .

cim:Resistance.unit  rdf:type  rdf:Property ;
        rdfs:domain        cim:Resistance ;
        rdfs:label         "unit"@en ;
        rdfs:range         cim:UnitSymbol ;
        cims:isFixed       "ohm" ;
        cims:multiplicity  cims:M:0..1 ;
        cims:stereotype    <http://iec.ch/TC57/NonStandard/UML#attribute> .

cim:Resistance.value  rdf:type  rdf:Property ;
        rdfs:domain        cim:Resistance ;
        rdfs:label         "value"@en ;
        cims:dataType      cim:Float ;
        cims:multiplicity  cims:M:0..1 ;
        cims:stereotype    <http://iec.ch/TC57/NonStandard/UML#attribute> .

cim:Season  rdf:type            rdfs:Class ;
        rdfs:comment            "A specified time period of the year." ;
        rdfs:label              "Season"@en ;
        rdfs:subClassOf         cim:IdentifiedObject ;
        cims:belongsToCategory  shs:Package_SteadyStateHypothesisScheduleProfile ;
        cims:stereotype         <http://iec.ch/TC57/NonStandard/UML#concrete> .

cim:Season.endDate  rdf:type  rdf:Property ;
        rdfs:comment       "Date season ends." ;
        rdfs:domain        cim:Season ;
        rdfs:label         "endDate"@en ;
        cims:dataType      cim:MonthDay ;
        cims:multiplicity  cims:M:1..1 ;
        cims:stereotype    <http://iec.ch/TC57/NonStandard/UML#attribute> .

cim:Season.startDate  rdf:type  rdf:Property ;
        rdfs:comment       "Date season starts." ;
        rdfs:domain        cim:Season ;
        rdfs:label         "startDate"@en ;
        cims:dataType      cim:MonthDay ;
        cims:multiplicity  cims:M:1..1 ;
        cims:stereotype    <http://iec.ch/TC57/NonStandard/UML#attribute> .

cim:ShuntCompensator  rdf:type  rdfs:Class ;
        rdfs:comment            "A shunt capacitor or reactor or switchable bank of shunt capacitors or reactors. A section of a shunt compensator is an individual capacitor or reactor. A negative value for bPerSection indicates that the compensator is a reactor. ShuntCompensator is a single terminal device.  Ground is implied." ;
        rdfs:label              "ShuntCompensator"@en ;
        cims:belongsToCategory  shs:Package_SteadyStateHypothesisScheduleProfile .

cim:StaticVarCompensator
        rdf:type                rdfs:Class ;
        rdfs:comment            "A facility for providing variable and controllable shunt reactive power. The SVC typically consists of a stepdown transformer, filter, thyristor-controlled reactor, and thyristor-switched capacitor arms.\n\nThe SVC may operate in fixed MVar output mode or in voltage control mode. When in voltage control mode, the output of the SVC will be proportional to the deviation of voltage at the controlled bus from the voltage setpoint.  The SVC characteristic slope defines the proportion.  If the voltage at the controlled bus is equal to the voltage setpoint, the SVC MVar output is zero." ;
        rdfs:label              "StaticVarCompensator"@en ;
        cims:belongsToCategory  shs:Package_SteadyStateHypothesisScheduleProfile .

cim:String  rdf:type            rdfs:Class ;
        rdfs:comment            "A string consisting of a sequence of characters. The character encoding is UTF-8. The string length is unspecified and unlimited." ;
        rdfs:label              "String"@en ;
        cims:belongsToCategory  shs:Package_SteadyStateHypothesisScheduleProfile ;
        cims:stereotype         "Primitive" .

cim:Switch  rdf:type            rdfs:Class ;
        rdfs:comment            "A generic device designed to close, or open, or both, one or more electric circuits.  All switches are two terminal devices including grounding switches. The ACDCTerminal.connected at the two sides of the switch shall not be considered for assessing switch connectivity, i.e. only Switch.open, .normalOpen and .locked are relevant." ;
        rdfs:label              "Switch"@en ;
        cims:belongsToCategory  shs:Package_SteadyStateHypothesisScheduleProfile .

cim:SynchronousMachine
        rdf:type                rdfs:Class ;
        rdfs:comment            "An electromechanical device that operates with shaft rotating synchronously with the network. It is a single machine operating either as a generator or synchronous condenser or pump." ;
        rdfs:label              "SynchronousMachine"@en ;
        cims:belongsToCategory  shs:Package_SteadyStateHypothesisScheduleProfile .

cim:SynchronousMachineOperatingMode
        rdf:type                rdfs:Class ;
        rdfs:comment            "Synchronous machine operating mode." ;
        rdfs:label              "SynchronousMachineOperatingMode"@en ;
        cims:belongsToCategory  shs:Package_SteadyStateHypothesisScheduleProfile ;
        cims:stereotype         <http://iec.ch/TC57/NonStandard/UML#enumeration> .

cim:SynchronousMachineOperatingMode.condenser
        rdf:type         cim:SynchronousMachineOperatingMode ;
        rdfs:comment     "Operating as condenser." ;
        rdfs:label       "condenser"@en ;
        cims:stereotype  "enum" .

cim:SynchronousMachineOperatingMode.generator
        rdf:type         cim:SynchronousMachineOperatingMode ;
        rdfs:comment     "Operating as generator." ;
        rdfs:label       "generator"@en ;
        cims:stereotype  "enum" .

cim:SynchronousMachineOperatingMode.motor
        rdf:type         cim:SynchronousMachineOperatingMode ;
        rdfs:comment     "Operating as motor." ;
        rdfs:label       "motor"@en ;
        cims:stereotype  "enum" .

cim:TapChanger  rdf:type        rdfs:Class ;
        rdfs:comment            "Mechanism for changing transformer winding tap positions." ;
        rdfs:label              "TapChanger"@en ;
        cims:belongsToCategory  shs:Package_SteadyStateHypothesisScheduleProfile .

cim:TapChangerControl
        rdf:type                rdfs:Class ;
        rdfs:comment            "Describes behaviour specific to tap changers, e.g. how the voltage at the end of a line varies with the load level and compensation of the voltage drop by tap adjustment." ;
        rdfs:label              "TapChangerControl"@en ;
        cims:belongsToCategory  shs:Package_SteadyStateHypothesisScheduleProfile .

cim:Time  rdf:type              rdfs:Class ;
        rdfs:comment            "Time as \"hh:mm:ss.sss\", which conforms with ISO 8601. UTC time zone is specified as \"hh:mm:ss.sssZ\". A local timezone relative UTC is specified as \"hh:mm:ss.sss±hh:mm\". The second component (shown here as \"ss.sss\") could have any number of digits in its fractional part to allow any kind of precision beyond seconds." ;
        rdfs:label              "Time"@en ;
        cims:belongsToCategory  shs:Package_SteadyStateHypothesisScheduleProfile ;
        cims:stereotype         "Primitive" .

cim:UnitMultiplier  rdf:type    rdfs:Class ;
        rdfs:comment            "The unit multipliers defined for the CIM.  When applied to unit symbols, the unit symbol is treated as a derived unit. Regardless of the contents of the unit symbol text, the unit symbol shall be treated as if it were a single-character unit symbol. Unit symbols should not contain multipliers, and it should be left to the multiplier to define the multiple for an entire data type. \n\nFor example, if a unit symbol is \"m2Pers\" and the multiplier is \"k\", then the value is k(m**2/s), and the multiplier applies to the entire final value, not to any individual part of the value. This can be conceptualized by substituting a derived unit symbol for the unit type. If one imagines that the symbol \"Þ\" represents the derived unit \"m2Pers\", then applying the multiplier \"k\" can be conceptualized simply as \"kÞ\".\n\nFor example, the SI unit for mass is \"kg\" and not \"g\".  If the unit symbol is defined as \"kg\", then the multiplier is applied to \"kg\" as a whole and does not replace the \"k\" in front of the \"g\". In this case, the multiplier of \"m\" would be used with the unit symbol of \"kg\" to represent one gram.  As a text string, this violates the instructions in IEC 80000-1. However, because the unit symbol in CIM is treated as a derived unit instead of as an SI unit, it makes more sense to conceptualize the \"kg\" as if it were replaced by one of the proposed replacements for the SI mass symbol. If one imagines that the \"kg\" were replaced by a symbol \"Þ\", then it is easier to conceptualize the multiplier \"m\" as creating the proper unit \"mÞ\", and not the forbidden unit \"mkg\"." ;
        rdfs:label              "UnitMultiplier"@en ;
        cims:belongsToCategory  shs:Package_SteadyStateHypothesisScheduleProfile ;
        cims:stereotype         <http://iec.ch/TC57/NonStandard/UML#enumeration> .

cim:UnitMultiplier.M  rdf:type  cim:UnitMultiplier ;
        rdfs:comment     "Mega 10**6." ;
        rdfs:label       "M"@en ;
        cims:stereotype  "enum" .

cim:UnitMultiplier.k  rdf:type  cim:UnitMultiplier ;
        rdfs:comment     "Kilo 10**3." ;
        rdfs:label       "k"@en ;
        cims:stereotype  "enum" .

cim:UnitMultiplier.none
        rdf:type         cim:UnitMultiplier ;
        rdfs:comment     "No multiplier or equivalently multiply by 1." ;
        rdfs:label       "none"@en ;
        cims:stereotype  "enum" .

cim:UnitSymbol  rdf:type        rdfs:Class ;
        rdfs:comment            "The derived units defined for usage in the CIM. In some cases, the derived unit is equal to an SI unit. Whenever possible, the standard derived symbol is used instead of the formula for the derived unit. For example, the unit symbol Farad is defined as \"F\" instead of \"CPerV\". In cases where a standard symbol does not exist for a derived unit, the formula for the unit is used as the unit symbol. For example, density does not have a standard symbol and so it is represented as \"kgPerm3\". With the exception of the \"kg\", which is an SI unit, the unit symbols do not contain multipliers and therefore represent the base derived unit to which a multiplier can be applied as a whole. \nEvery unit symbol is treated as an unparseable text as if it were a single-letter symbol. The meaning of each unit symbol is defined by the accompanying descriptive text and not by the text contents of the unit symbol.\nTo allow the widest possible range of serializations without requiring special character handling, several substitutions are made which deviate from the format described in IEC 80000-1. The division symbol \"/\" is replaced by the letters \"Per\". Exponents are written in plain text after the unit as \"m3\" instead of being formatted as \"m\" with a superscript of 3  or introducing a symbol as in \"m^3\". The degree symbol \"°\" is replaced with the letters \"deg\". Any clarification of the meaning for a substitution is included in the description for the unit symbol.\nNon-SI units are included in list of unit symbols to allow sources of data to be correctly labelled with their non-SI units (for example, a GPS sensor that is reporting numbers that represent feet instead of meters). This allows software to use the unit symbol information correctly convert and scale the raw data of those sources into SI-based units. \nThe integer values are used for harmonization with IEC 61850." ;
        rdfs:label              "UnitSymbol"@en ;
        cims:belongsToCategory  shs:Package_SteadyStateHypothesisScheduleProfile ;
        cims:stereotype         <http://iec.ch/TC57/NonStandard/UML#enumeration> .

cim:UnitSymbol.A  rdf:type  cim:UnitSymbol ;
        rdfs:comment     "Current in amperes." ;
        rdfs:label       "A"@en ;
        cims:stereotype  "enum" .

cim:UnitSymbol.V  rdf:type  cim:UnitSymbol ;
        rdfs:comment     "Electric potential in volts (W/A)." ;
        rdfs:label       "V"@en ;
        cims:stereotype  "enum" .

cim:UnitSymbol.VA  rdf:type  cim:UnitSymbol ;
        rdfs:comment     "Apparent power in volt amperes. See also real power and reactive power." ;
        rdfs:label       "VA"@en ;
        cims:stereotype  "enum" .

cim:UnitSymbol.VAr  rdf:type  cim:UnitSymbol ;
        rdfs:comment     "Reactive power in volt amperes reactive. The “reactive” or “imaginary” component of electrical power (VIsin(phi)). (See also real power and apparent power).\nNote: Different meter designs use different methods to arrive at their results. Some meters may compute reactive power as an arithmetic value, while others compute the value vectorially. The data consumer should determine the method in use and the suitability of the measurement for the intended purpose." ;
        rdfs:label       "VAr"@en ;
        cims:stereotype  "enum" .

cim:UnitSymbol.W  rdf:type  cim:UnitSymbol ;
        rdfs:comment     "Real power in watts (J/s). Electrical power may have real and reactive components. The real portion of electrical power (I&#178;R or VIcos(phi)), is expressed in Watts. See also apparent power and reactive power." ;
        rdfs:label       "W"@en ;
        cims:stereotype  "enum" .

cim:UnitSymbol.Wh  rdf:type  cim:UnitSymbol ;
        rdfs:comment     "Real energy in watt hours." ;
        rdfs:label       "Wh"@en ;
        cims:stereotype  "enum" .

cim:UnitSymbol.deg  rdf:type  cim:UnitSymbol ;
        rdfs:comment     "Plane angle in degrees." ;
        rdfs:label       "deg"@en ;
        cims:stereotype  "enum" .

cim:UnitSymbol.none  rdf:type  cim:UnitSymbol ;
        rdfs:comment     "Dimension less quantity, e.g. count, per unit, etc." ;
        rdfs:label       "none"@en ;
        cims:stereotype  "enum" .

cim:UnitSymbol.ohm  rdf:type  cim:UnitSymbol ;
        rdfs:comment     "Electric resistance in ohms (V/A)." ;
        rdfs:label       "ohm"@en ;
        cims:stereotype  "enum" .

cim:Voltage  rdf:type           rdfs:Class ;
        rdfs:comment            "Electrical voltage, can be both AC and DC." ;
        rdfs:label              "Voltage"@en ;
        cims:belongsToCategory  shs:Package_SteadyStateHypothesisScheduleProfile ;
        cims:stereotype         "CIMDatatype" .

cim:Voltage.multiplier
        rdf:type           rdf:Property ;
        rdfs:domain        cim:Voltage ;
        rdfs:label         "multiplier"@en ;
        rdfs:range         cim:UnitMultiplier ;
        cims:isFixed       "k" ;
        cims:multiplicity  cims:M:0..1 ;
        cims:stereotype    <http://iec.ch/TC57/NonStandard/UML#attribute> .

cim:Voltage.unit  rdf:type  rdf:Property ;
        rdfs:domain        cim:Voltage ;
        rdfs:label         "unit"@en ;
        rdfs:range         cim:UnitSymbol ;
        cims:isFixed       "V" ;
        cims:multiplicity  cims:M:0..1 ;
        cims:stereotype    <http://iec.ch/TC57/NonStandard/UML#attribute> .

cim:Voltage.value  rdf:type  rdf:Property ;
        rdfs:domain        cim:Voltage ;
        rdfs:label         "value"@en ;
        cims:dataType      cim:Float ;
        cims:multiplicity  cims:M:0..1 ;
        cims:stereotype    <http://iec.ch/TC57/NonStandard/UML#attribute> .

cim:VoltageLimit  rdf:type      rdfs:Class ;
        rdfs:comment            "Operational limit applied to voltage.\nThe use of operational VoltageLimit is preferred instead of limits defined at VoltageLevel. The operational VoltageLimits are used, if present." ;
        rdfs:label              "VoltageLimit"@en ;
        cims:belongsToCategory  shs:Package_SteadyStateHypothesisScheduleProfile .

cim:VsConverter  rdf:type       rdfs:Class ;
        rdfs:comment            "DC side of the voltage source converter (VSC)." ;
        rdfs:label              "VsConverter"@en ;
        cims:belongsToCategory  shs:Package_SteadyStateHypothesisScheduleProfile .

cim:VsPpccControlKind
        rdf:type                rdfs:Class ;
        rdfs:comment            "Types applicable to the control of real power and/or DC voltage by voltage source converter." ;
        rdfs:label              "VsPpccControlKind"@en ;
        cims:belongsToCategory  shs:Package_SteadyStateHypothesisScheduleProfile ;
        cims:stereotype         <http://iec.ch/TC57/NonStandard/UML#enumeration> .

cim:VsPpccControlKind.pPcc
        rdf:type         cim:VsPpccControlKind ;
        rdfs:comment     "Control is real power at point of common coupling. The target value is provided by ACDCConverter.targetPpcc." ;
        rdfs:label       "pPcc"@en ;
        cims:stereotype  "enum" .

cim:VsPpccControlKind.pPccAndUdcDroop
        rdf:type         cim:VsPpccControlKind ;
        rdfs:comment     "Control is active power at point of common coupling and local DC voltage, with the droop. Target values are provided by ACDCConverter.targetPpcc, ACDCConverter.targetUdc and VsConverter.droop." ;
        rdfs:label       "pPccAndUdcDroop"@en ;
        cims:stereotype  "enum" .

cim:VsPpccControlKind.pPccAndUdcDroopPilot
        rdf:type         cim:VsPpccControlKind ;
        rdfs:comment     "Control is active power at point of common coupling and the pilot DC voltage, with the droop. The mode is used for Multi Terminal High Voltage DC (MTDC) systems where multiple HVDC Substations are connected to the HVDC transmission lines. The pilot voltage is then used to coordinate the control the DC voltage across the HVDC substations. Targets are provided by ACDCConverter.targetPpcc, ACDCConverter.targetUdc and  VsConverter.droop." ;
        rdfs:label       "pPccAndUdcDroopPilot"@en ;
        cims:stereotype  "enum" .

cim:VsPpccControlKind.pPccAndUdcDroopWithCompensation
        rdf:type         cim:VsPpccControlKind ;
        rdfs:comment     "Control is active power at point of common coupling and compensated DC voltage, with the droop. Compensation factor is the resistance, as an approximation of the DC voltage of a common (real or virtual) node in the DC network. Targets are provided by ACDCConverter.targetPpcc, ACDCConverter.targetUdc, VsConverter.droop and VsConverter.droopCompensation." ;
        rdfs:label       "pPccAndUdcDroopWithCompensation"@en ;
        cims:stereotype  "enum" .

cim:VsPpccControlKind.phasePcc
        rdf:type         cim:VsPpccControlKind ;
        rdfs:comment     "Control is phase at point of common coupling. Target is provided by VsConverter.targetPhasePcc." ;
        rdfs:label       "phasePcc"@en ;
        cims:stereotype  "enum" .

cim:VsPpccControlKind.udc
        rdf:type         cim:VsPpccControlKind ;
        rdfs:comment     "Control is DC voltage  with target value provided by ACDCConverter.targetUdc." ;
        rdfs:label       "udc"@en ;
        cims:stereotype  "enum" .

cim:VsQpccControlKind
        rdf:type                rdfs:Class ;
        rdfs:comment            "Kind of reactive power control at point of common coupling for a voltage source converter." ;
        rdfs:label              "VsQpccControlKind"@en ;
        cims:belongsToCategory  shs:Package_SteadyStateHypothesisScheduleProfile ;
        cims:stereotype         <http://iec.ch/TC57/NonStandard/UML#enumeration> .

cim:VsQpccControlKind.powerFactorPcc
        rdf:type         cim:VsQpccControlKind ;
        rdfs:comment     "Control is power factor at point of common coupling. Target is provided by VsConverter.targetPowerFactorPcc." ;
        rdfs:label       "powerFactorPcc"@en ;
        cims:stereotype  "enum" .

cim:VsQpccControlKind.pulseWidthModulation
        rdf:type         cim:VsQpccControlKind ;
        rdfs:comment     "No explicit control. Pulse-modulation factor is directly set in magnitude (VsConverter.targetPWMfactor) and phase (VsConverter.targetPhasePcc)." ;
        rdfs:label       "pulseWidthModulation"@en ;
        cims:stereotype  "enum" .

cim:VsQpccControlKind.reactivePcc
        rdf:type         cim:VsQpccControlKind ;
        rdfs:comment     "Control is reactive power at point of common coupling. Target is provided by VsConverter.targetQpcc." ;
        rdfs:label       "reactivePcc"@en ;
        cims:stereotype  "enum" .

cim:VsQpccControlKind.voltagePcc
        rdf:type         cim:VsQpccControlKind ;
        rdfs:comment     "Control is voltage at point of common coupling. Target is provided by VsConverter.targetUpcc." ;
        rdfs:label       "voltagePcc"@en ;
        cims:stereotype  "enum" .

nc:ACDCConverterRegularSchedule
        rdf:type                rdfs:Class ;
        rdfs:comment            "Regular schedule for ACDC converter." ;
        rdfs:label              "ACDCConverterRegularSchedule"@en ;
        rdfs:subClassOf         nc:BaseRegularIntervalSchedule ;
        cims:belongsToCategory  shs:Package_SteadyStateHypothesisScheduleProfile ;
        cims:stereotype         "NC" .

nc:ACDCConverterRegularSchedule.p
        rdf:type           rdf:Property ;
        rdfs:comment       "Active power at the point of common coupling. Load sign convention is used, i.e. positive sign means flow out from a node.\nStarting value for a steady state solution in the case a simplified power flow model is used." ;
        rdfs:domain        nc:ACDCConverterRegularSchedule ;
        rdfs:label         "p"@en ;
        cims:dataType      cim:ActivePower ;
        cims:multiplicity  cims:M:1..1 ;
        cims:stereotype    "NC" ;
        cims:stereotype    <http://iec.ch/TC57/NonStandard/UML#attribute> .

nc:ACDCConverterRegularSchedule.q
        rdf:type           rdf:Property ;
        rdfs:comment       "Reactive power at the point of common coupling. Load sign convention is used, i.e. positive sign means flow out from a node.\nStarting value for a steady state solution in the case a simplified power flow model is used." ;
        rdfs:domain        nc:ACDCConverterRegularSchedule ;
        rdfs:label         "q"@en ;
        cims:dataType      cim:ReactivePower ;
        cims:multiplicity  cims:M:1..1 ;
        cims:stereotype    "NC" ;
        cims:stereotype    <http://iec.ch/TC57/NonStandard/UML#attribute> .

nc:ACDCConverterRegularSchedule.targetPpcc
        rdf:type           rdf:Property ;
        rdfs:comment       "Real power injection target in AC grid, at point of common coupling.  Load sign convention is used, i.e. positive sign means flow out from a node." ;
        rdfs:domain        nc:ACDCConverterRegularSchedule ;
        rdfs:label         "targetPpcc"@en ;
        cims:dataType      cim:ActivePower ;
        cims:multiplicity  cims:M:0..1 ;
        cims:stereotype    "NC" ;
        cims:stereotype    <http://iec.ch/TC57/NonStandard/UML#attribute> .

nc:ACDCConverterRegularSchedule.targetUdc
        rdf:type           rdf:Property ;
        rdfs:comment       "Target value for DC voltage magnitude. The attribute shall be a positive value." ;
        rdfs:domain        nc:ACDCConverterRegularSchedule ;
        rdfs:label         "targetUdc"@en ;
        cims:dataType      cim:Voltage ;
        cims:multiplicity  cims:M:0..1 ;
        cims:stereotype    "NC" ;
        cims:stereotype    <http://iec.ch/TC57/NonStandard/UML#attribute> .

nc:ACDCTimePoint  rdf:type      rdfs:Class ;
        rdfs:comment            "ACDC values for a given point in time." ;
        rdfs:label              "ACDCTimePoint"@en ;
        cims:belongsToCategory  shs:Package_SteadyStateHypothesisScheduleProfile ;
        cims:stereotype         "NC" .

nc:ACDCTimePoint.atTime
        rdf:type           rdf:Property ;
        rdfs:comment       "The time the data is valid for." ;
        rdfs:domain        nc:ACDCTimePoint ;
        rdfs:label         "atTime"@en ;
        cims:dataType      cim:DateTime ;
        cims:multiplicity  cims:M:1..1 ;
        cims:stereotype    "NC" ;
        cims:stereotype    <http://iec.ch/TC57/NonStandard/UML#attribute> .

nc:ACDCTimePoint.p  rdf:type  rdf:Property ;
        rdfs:comment       "Active power at the point of common coupling. Load sign convention is used, i.e. positive sign means flow out from a node.\nStarting value for a steady state solution in the case a simplified power flow model is used." ;
        rdfs:domain        nc:ACDCTimePoint ;
        rdfs:label         "p"@en ;
        cims:dataType      cim:ActivePower ;
        cims:multiplicity  cims:M:1..1 ;
        cims:stereotype    "NC" ;
        cims:stereotype    <http://iec.ch/TC57/NonStandard/UML#attribute> .

nc:ACDCTimePoint.q  rdf:type  rdf:Property ;
        rdfs:comment       "Reactive power at the point of common coupling. Load sign convention is used, i.e. positive sign means flow out from a node.\nStarting value for a steady state solution in the case a simplified power flow model is used." ;
        rdfs:domain        nc:ACDCTimePoint ;
        rdfs:label         "q"@en ;
        cims:dataType      cim:ReactivePower ;
        cims:multiplicity  cims:M:1..1 ;
        cims:stereotype    "NC" ;
        cims:stereotype    <http://iec.ch/TC57/NonStandard/UML#attribute> .

nc:ACDCTimePoint.targetPpcc
        rdf:type           rdf:Property ;
        rdfs:comment       "Real power injection target in AC grid, at point of common coupling.  Load sign convention is used, i.e. positive sign means flow out from a node." ;
        rdfs:domain        nc:ACDCTimePoint ;
        rdfs:label         "targetPpcc"@en ;
        cims:dataType      cim:ActivePower ;
        cims:multiplicity  cims:M:0..1 ;
        cims:stereotype    "NC" ;
        cims:stereotype    <http://iec.ch/TC57/NonStandard/UML#attribute> .

nc:ACDCTimePoint.targetUdc
        rdf:type           rdf:Property ;
        rdfs:comment       "Target value for DC voltage magnitude. The attribute shall be a positive value." ;
        rdfs:domain        nc:ACDCTimePoint ;
        rdfs:label         "targetUdc"@en ;
        cims:dataType      cim:Voltage ;
        cims:multiplicity  cims:M:0..1 ;
        cims:stereotype    "NC" ;
        cims:stereotype    <http://iec.ch/TC57/NonStandard/UML#attribute> .

nc:ActivePowerLimit.ActivePowerLimitSchedule
        rdf:type              rdf:Property ;
        rdfs:comment          "Active power limit schedule associated with an active power limit." ;
        rdfs:domain           cim:ActivePowerLimit ;
        rdfs:label            "ActivePowerLimitSchedule"@en ;
        rdfs:range            nc:ActivePowerLimitSchedule ;
        cims:AssociationUsed  "No" ;
        cims:inverseRoleName  nc:ActivePowerLimitSchedule.ActivePowerLimit ;
        cims:multiplicity     cims:M:0..n ;
        cims:stereotype       "NC" .

nc:ActivePowerLimitSchedule
        rdf:type                rdfs:Class ;
        rdfs:comment            "Schedule for active power limit." ;
        rdfs:label              "ActivePowerLimitSchedule"@en ;
        rdfs:subClassOf         nc:BaseIrregularTimeSeries ;
        cims:belongsToCategory  shs:Package_SteadyStateHypothesisScheduleProfile ;
        cims:stereotype         "NC" ;
        cims:stereotype         <http://iec.ch/TC57/NonStandard/UML#concrete> .

nc:ActivePowerLimitSchedule.ActivePowerLimit
        rdf:type              rdf:Property ;
        rdfs:comment          "Active power limit which has active power limit schedules." ;
        rdfs:domain           nc:ActivePowerLimitSchedule ;
        rdfs:label            "ActivePowerLimit"@en ;
        rdfs:range            cim:ActivePowerLimit ;
        cims:AssociationUsed  "Yes" ;
        cims:inverseRoleName  nc:ActivePowerLimit.ActivePowerLimitSchedule ;
        cims:multiplicity     cims:M:0..1 ;
        cims:stereotype       "NC" .

nc:ActivePowerLimitSchedule.ActivePowerLimitTimePoint
        rdf:type              rdf:Property ;
        rdfs:comment          "The time point that relates to this active pwoer limit schedule." ;
        rdfs:domain           nc:ActivePowerLimitSchedule ;
        rdfs:label            "ActivePowerLimitTimePoint"@en ;
        rdfs:range            nc:ActivePowerLimitTimePoint ;
        cims:AssociationUsed  "No" ;
        cims:inverseRoleName  nc:ActivePowerLimitTimePoint.ActivePowerLimitSchedule ;
        cims:multiplicity     cims:M:1..n ;
        cims:stereotype       "NC" ;
        cims:stereotype       <http://iec.ch/TC57/NonStandard/UML#ofAggregate> .

nc:ActivePowerLimitTimePoint
        rdf:type                rdfs:Class ;
        rdfs:comment            "Active power limit for a given point in time." ;
        rdfs:label              "ActivePowerLimitTimePoint"@en ;
        cims:belongsToCategory  shs:Package_SteadyStateHypothesisScheduleProfile ;
        cims:stereotype         "NC" ;
        cims:stereotype         <http://iec.ch/TC57/NonStandard/UML#concrete> .

nc:ActivePowerLimitTimePoint.ActivePowerLimitSchedule
        rdf:type              rdf:Property ;
        rdfs:comment          "The active power limit schedule that has this time point." ;
        rdfs:domain           nc:ActivePowerLimitTimePoint ;
        rdfs:label            "ActivePowerLimitSchedule"@en ;
        rdfs:range            nc:ActivePowerLimitSchedule ;
        cims:AssociationUsed  "Yes" ;
        cims:inverseRoleName  nc:ActivePowerLimitSchedule.ActivePowerLimitTimePoint ;
        cims:multiplicity     cims:M:1 ;
        cims:stereotype       "NC" .

nc:ActivePowerLimitTimePoint.atTime
        rdf:type           rdf:Property ;
        rdfs:comment       "The time the data is valid for." ;
        rdfs:domain        nc:ActivePowerLimitTimePoint ;
        rdfs:label         "atTime"@en ;
        cims:dataType      cim:DateTime ;
        cims:multiplicity  cims:M:1..1 ;
        cims:stereotype    "NC" ;
        cims:stereotype    <http://iec.ch/TC57/NonStandard/UML#attribute> .

nc:ActivePowerLimitTimePoint.value
        rdf:type           rdf:Property ;
        rdfs:comment       "Value of active power limit. The attribute shall be a positive value or zero." ;
        rdfs:domain        nc:ActivePowerLimitTimePoint ;
        rdfs:label         "value"@en ;
        cims:dataType      cim:ActivePower ;
        cims:multiplicity  cims:M:1..1 ;
        cims:stereotype    "NC" ;
        cims:stereotype    <http://iec.ch/TC57/NonStandard/UML#attribute> .

nc:ApparentPowerLimit.ApparentPowerLimitSchedule
        rdf:type              rdf:Property ;
        rdfs:comment          "Apparent power limit schedule associated with an apparent power limit." ;
        rdfs:domain           cim:ApparentPowerLimit ;
        rdfs:label            "ApparentPowerLimitSchedule"@en ;
        rdfs:range            nc:ApparentPowerLimitSchedule ;
        cims:AssociationUsed  "No" ;
        cims:inverseRoleName  nc:ApparentPowerLimitSchedule.ApparentPowerLimit ;
        cims:multiplicity     cims:M:0..n ;
        cims:stereotype       "NC" .

nc:ApparentPowerLimitSchedule
        rdf:type                rdfs:Class ;
        rdfs:comment            "Schedule for apparent power limit." ;
        rdfs:label              "ApparentPowerLimitSchedule"@en ;
        rdfs:subClassOf         nc:BaseIrregularTimeSeries ;
        cims:belongsToCategory  shs:Package_SteadyStateHypothesisScheduleProfile ;
        cims:stereotype         "NC" ;
        cims:stereotype         <http://iec.ch/TC57/NonStandard/UML#concrete> .

nc:ApparentPowerLimitSchedule.ApparentPowerLimit
        rdf:type              rdf:Property ;
        rdfs:comment          "Apparent power limit which has apparent power limit schedules." ;
        rdfs:domain           nc:ApparentPowerLimitSchedule ;
        rdfs:label            "ApparentPowerLimit"@en ;
        rdfs:range            cim:ApparentPowerLimit ;
        cims:AssociationUsed  "Yes" ;
        cims:inverseRoleName  nc:ApparentPowerLimit.ApparentPowerLimitSchedule ;
        cims:multiplicity     cims:M:0..1 ;
        cims:stereotype       "NC" .

nc:ApparentPowerLimitSchedule.ApparentPowerLimitTimePoint
        rdf:type              rdf:Property ;
        rdfs:comment          "The time point that relates to this apparent power limit schedule." ;
        rdfs:domain           nc:ApparentPowerLimitSchedule ;
        rdfs:label            "ApparentPowerLimitTimePoint"@en ;
        rdfs:range            nc:ApparentPowerLimitTimePoint ;
        cims:AssociationUsed  "No" ;
        cims:inverseRoleName  nc:ApparentPowerLimitTimePoint.ApparentPowerLimitSchedule ;
        cims:multiplicity     cims:M:1..n ;
        cims:stereotype       "NC" ;
        cims:stereotype       <http://iec.ch/TC57/NonStandard/UML#ofAggregate> .

nc:ApparentPowerLimitTimePoint
        rdf:type                rdfs:Class ;
        rdfs:comment            "Apparent power limit for a given point in time." ;
        rdfs:label              "ApparentPowerLimitTimePoint"@en ;
        cims:belongsToCategory  shs:Package_SteadyStateHypothesisScheduleProfile ;
        cims:stereotype         "NC" ;
        cims:stereotype         <http://iec.ch/TC57/NonStandard/UML#concrete> .

nc:ApparentPowerLimitTimePoint.ApparentPowerLimitSchedule
        rdf:type              rdf:Property ;
        rdfs:comment          "The apparent power limit schedule that has this time point." ;
        rdfs:domain           nc:ApparentPowerLimitTimePoint ;
        rdfs:label            "ApparentPowerLimitSchedule"@en ;
        rdfs:range            nc:ApparentPowerLimitSchedule ;
        cims:AssociationUsed  "Yes" ;
        cims:inverseRoleName  nc:ApparentPowerLimitSchedule.ApparentPowerLimitTimePoint ;
        cims:multiplicity     cims:M:1 ;
        cims:stereotype       "NC" .

nc:ApparentPowerLimitTimePoint.atTime
        rdf:type           rdf:Property ;
        rdfs:comment       "The time the data is valid for." ;
        rdfs:domain        nc:ApparentPowerLimitTimePoint ;
        rdfs:label         "atTime"@en ;
        cims:dataType      cim:DateTime ;
        cims:multiplicity  cims:M:1..1 ;
        cims:stereotype    "NC" ;
        cims:stereotype    <http://iec.ch/TC57/NonStandard/UML#attribute> .

nc:ApparentPowerLimitTimePoint.value
        rdf:type           rdf:Property ;
        rdfs:comment       "The apparent power limit. The attribute shall be a positive value or zero." ;
        rdfs:domain        nc:ApparentPowerLimitTimePoint ;
        rdfs:label         "value"@en ;
        cims:dataType      cim:ApparentPower ;
        cims:multiplicity  cims:M:1..1 ;
        cims:stereotype    "NC" ;
        cims:stereotype    <http://iec.ch/TC57/NonStandard/UML#attribute> .

nc:AsynchronousMachine.AsynchronousMachineRegularSchedule
        rdf:type              rdf:Property ;
        rdfs:comment          "AsynchronousMachineRegularSchedule which belongs to an asynchronous machine." ;
        rdfs:domain           cim:AsynchronousMachine ;
        rdfs:label            "AsynchronousMachineRegularSchedule"@en ;
        rdfs:range            nc:AsynchronousMachineRegularSchedule ;
        cims:AssociationUsed  "No" ;
        cims:inverseRoleName  nc:AsynchronousMachineRegularSchedule.AsynchronousMachine ;
        cims:multiplicity     cims:M:0..n ;
        cims:stereotype       "NC" .

nc:AsynchronousMachine.AsynchronousMachineSchedule
        rdf:type              rdf:Property ;
        rdfs:comment          "Asynchronous machine schedule associated with an asynchronous machine." ;
        rdfs:domain           cim:AsynchronousMachine ;
        rdfs:label            "AsynchronousMachineSchedule"@en ;
        rdfs:range            nc:AsynchronousMachineSchedule ;
        cims:AssociationUsed  "No" ;
        cims:inverseRoleName  nc:AsynchronousMachineSchedule.AsynchronousMachine ;
        cims:multiplicity     cims:M:0..n ;
        cims:stereotype       "NC" .

nc:AsynchronousMachineRegularSchedule
        rdf:type                rdfs:Class ;
        rdfs:comment            "Regular schedule for asynchronous machine." ;
        rdfs:label              "AsynchronousMachineRegularSchedule"@en ;
        rdfs:subClassOf         nc:BaseRegularIntervalSchedule ;
        cims:belongsToCategory  shs:Package_SteadyStateHypothesisScheduleProfile ;
        cims:stereotype         "NC" ;
        cims:stereotype         <http://iec.ch/TC57/NonStandard/UML#concrete> .

nc:AsynchronousMachineRegularSchedule.AsynchronousMachine
        rdf:type              rdf:Property ;
        rdfs:comment          "AsynchronousMachine which has AsynchronousMachineRegularSchedule." ;
        rdfs:domain           nc:AsynchronousMachineRegularSchedule ;
        rdfs:label            "AsynchronousMachine"@en ;
        rdfs:range            cim:AsynchronousMachine ;
        cims:AssociationUsed  "Yes" ;
        cims:inverseRoleName  nc:AsynchronousMachine.AsynchronousMachineRegularSchedule ;
        cims:multiplicity     cims:M:0..1 ;
        cims:stereotype       "NC" .

nc:AsynchronousMachineRegularSchedule.asynchronousMachineType
        rdf:type           rdf:Property ;
        rdfs:comment       "Indicates the type of Asynchronous Machine (motor or generator)." ;
        rdfs:domain        nc:AsynchronousMachineRegularSchedule ;
        rdfs:label         "asynchronousMachineType"@en ;
        rdfs:range         cim:AsynchronousMachineKind ;
        cims:multiplicity  cims:M:1..1 ;
        cims:stereotype    "NC" ;
        cims:stereotype    <http://iec.ch/TC57/NonStandard/UML#attribute> .

nc:AsynchronousMachineSchedule
        rdf:type                rdfs:Class ;
        rdfs:comment            "Schedule for asynchronous machine." ;
        rdfs:label              "AsynchronousMachineSchedule"@en ;
        rdfs:subClassOf         nc:BaseIrregularTimeSeries ;
        cims:belongsToCategory  shs:Package_SteadyStateHypothesisScheduleProfile ;
        cims:stereotype         "NC" ;
        cims:stereotype         <http://iec.ch/TC57/NonStandard/UML#concrete> .

nc:AsynchronousMachineSchedule.AsynchronousMachine
        rdf:type              rdf:Property ;
        rdfs:comment          "Asynchronous machine which has asynchronous machine schedules." ;
        rdfs:domain           nc:AsynchronousMachineSchedule ;
        rdfs:label            "AsynchronousMachine"@en ;
        rdfs:range            cim:AsynchronousMachine ;
        cims:AssociationUsed  "Yes" ;
        cims:inverseRoleName  nc:AsynchronousMachine.AsynchronousMachineSchedule ;
        cims:multiplicity     cims:M:0..1 ;
        cims:stereotype       "NC" .

nc:AsynchronousMachineSchedule.AsynchronousMachineTimePoint
        rdf:type              rdf:Property ;
        rdfs:comment          "The time point that relates to this asynchronous machine schedule." ;
        rdfs:domain           nc:AsynchronousMachineSchedule ;
        rdfs:label            "AsynchronousMachineTimePoint"@en ;
        rdfs:range            nc:AsynchronousMachineTimePoint ;
        cims:AssociationUsed  "No" ;
        cims:inverseRoleName  nc:AsynchronousMachineTimePoint.AsynchronousMachineSchedule ;
        cims:multiplicity     cims:M:1..n ;
        cims:stereotype       "NC" ;
        cims:stereotype       <http://iec.ch/TC57/NonStandard/UML#ofAggregate> .

nc:AsynchronousMachineTimePoint
        rdf:type                rdfs:Class ;
        rdfs:comment            "Asynchronous machine values for a given point in time." ;
        rdfs:label              "AsynchronousMachineTimePoint"@en ;
        cims:belongsToCategory  shs:Package_SteadyStateHypothesisScheduleProfile ;
        cims:stereotype         "NC" ;
        cims:stereotype         <http://iec.ch/TC57/NonStandard/UML#concrete> .

nc:AsynchronousMachineTimePoint.AsynchronousMachineSchedule
        rdf:type              rdf:Property ;
        rdfs:comment          "The asynchronous machine schedule that has this time point." ;
        rdfs:domain           nc:AsynchronousMachineTimePoint ;
        rdfs:label            "AsynchronousMachineSchedule"@en ;
        rdfs:range            nc:AsynchronousMachineSchedule ;
        cims:AssociationUsed  "Yes" ;
        cims:inverseRoleName  nc:AsynchronousMachineSchedule.AsynchronousMachineTimePoint ;
        cims:multiplicity     cims:M:1 ;
        cims:stereotype       "NC" .

nc:AsynchronousMachineTimePoint.asynchronousMachineType
        rdf:type           rdf:Property ;
        rdfs:comment       "Indicates the type of Asynchronous Machine (motor or generator)." ;
        rdfs:domain        nc:AsynchronousMachineTimePoint ;
        rdfs:label         "asynchronousMachineType"@en ;
        rdfs:range         cim:AsynchronousMachineKind ;
        cims:multiplicity  cims:M:1..1 ;
        cims:stereotype    "NC" ;
        cims:stereotype    <http://iec.ch/TC57/NonStandard/UML#attribute> .

nc:AsynchronousMachineTimePoint.atTime
        rdf:type           rdf:Property ;
        rdfs:comment       "The time the data is valid for." ;
        rdfs:domain        nc:AsynchronousMachineTimePoint ;
        rdfs:label         "atTime"@en ;
        cims:dataType      cim:DateTime ;
        cims:multiplicity  cims:M:1..1 ;
        cims:stereotype    "NC" ;
        cims:stereotype    <http://iec.ch/TC57/NonStandard/UML#attribute> .

nc:BaseIrregularTimeSeries
        rdf:type                rdfs:Class ;
        rdfs:comment            "Time series that has irregular points in time." ;
        rdfs:label              "BaseIrregularTimeSeries"@en ;
        rdfs:subClassOf         nc:BaseTimeSeries ;
        cims:belongsToCategory  shs:Package_SteadyStateHypothesisScheduleProfile ;
        cims:stereotype         "NC" ;
        cims:stereotype         <http://iec.ch/TC57/NonStandard/UML#concrete> .

nc:BaseRegularIntervalSchedule
        rdf:type                rdfs:Class ;
        rdfs:comment            "Time series that has regular points in time." ;
        rdfs:label              "BaseRegularIntervalSchedule"@en ;
        rdfs:subClassOf         nc:BaseTimeSeries ;
        cims:belongsToCategory  shs:Package_SteadyStateHypothesisScheduleProfile ;
        cims:stereotype         "NC" .

nc:BaseRegularIntervalSchedule.HourPattern
        rdf:type              rdf:Property ;
        rdfs:comment          "HourPattern that has base regular interval schedule." ;
        rdfs:domain           nc:BaseRegularIntervalSchedule ;
        rdfs:label            "HourPattern"@en ;
        rdfs:range            nc:HourPattern ;
        cims:AssociationUsed  "Yes" ;
        cims:inverseRoleName  nc:HourPattern.BaseRegularIntervalSchedule ;
        cims:multiplicity     cims:M:0..1 ;
        cims:stereotype       "NC" .

nc:BaseRegularIntervalSchedule.Season
        rdf:type              rdf:Property ;
        rdfs:comment          "Season associated with a base regular interval schedule." ;
        rdfs:domain           nc:BaseRegularIntervalSchedule ;
        rdfs:label            "Season"@en ;
        rdfs:range            cim:Season ;
        cims:AssociationUsed  "Yes" ;
        cims:inverseRoleName  nc:Season.BaseRegularIntervalSchedule ;
        cims:multiplicity     cims:M:0..1 ;
        cims:stereotype       "NC" .

nc:BaseRegularIntervalSchedule.dayOfWeek
        rdf:type           rdf:Property ;
        rdfs:comment       "Day of the week for which the schedule is valid for." ;
        rdfs:domain        nc:BaseRegularIntervalSchedule ;
        rdfs:label         "dayOfWeek"@en ;
        rdfs:range         nc:DayOfWeekKind ;
        cims:multiplicity  cims:M:0..1 ;
        cims:stereotype    "NC" ;
        cims:stereotype    <http://iec.ch/TC57/NonStandard/UML#attribute> .

nc:BaseRegularIntervalSchedule.intervalEndTime
        rdf:type           rdf:Property ;
        rdfs:comment       "Interval end time for which the schedule is valid for." ;
        rdfs:domain        nc:BaseRegularIntervalSchedule ;
        rdfs:label         "intervalEndTime"@en ;
        cims:dataType      cim:DateTime ;
        cims:multiplicity  cims:M:0..1 ;
        cims:stereotype    "NC" ;
        cims:stereotype    <http://iec.ch/TC57/NonStandard/UML#attribute> .

nc:BaseRegularIntervalSchedule.intervalStartTime
        rdf:type           rdf:Property ;
        rdfs:comment       "Interval start time for which the schedule is valid for." ;
        rdfs:domain        nc:BaseRegularIntervalSchedule ;
        rdfs:label         "intervalStartTime"@en ;
        cims:dataType      cim:DateTime ;
        cims:multiplicity  cims:M:0..1 ;
        cims:stereotype    "NC" ;
        cims:stereotype    <http://iec.ch/TC57/NonStandard/UML#attribute> .

nc:BaseTimeSeries  rdf:type     rdfs:Class ;
        rdfs:comment            "Time series of values at points in time." ;
        rdfs:label              "BaseTimeSeries"@en ;
        rdfs:subClassOf         cim:IdentifiedObject ;
        cims:belongsToCategory  shs:Package_SteadyStateHypothesisScheduleProfile ;
        cims:stereotype         "NC" .

nc:BaseTimeSeries.generatedAtTime
        rdf:type           rdf:Property ;
        rdfs:comment       "The time this time series (entity) come to existents and available for use." ;
        rdfs:domain        nc:BaseTimeSeries ;
        rdfs:label         "generatedAtTime"@en ;
        cims:dataType      cim:DateTime ;
        cims:multiplicity  cims:M:0..1 ;
        cims:stereotype    "NC" ;
        cims:stereotype    <http://iec.ch/TC57/NonStandard/UML#attribute> .

nc:BaseTimeSeries.interpolationKind
        rdf:type           rdf:Property ;
        rdfs:comment       "Kind of interpolation done between time point." ;
        rdfs:domain        nc:BaseTimeSeries ;
        rdfs:label         "interpolationKind"@en ;
        rdfs:range         nc:TimeSeriesInterpolationKind ;
        cims:multiplicity  cims:M:1..1 ;
        cims:stereotype    "NC" ;
        cims:stereotype    <http://iec.ch/TC57/NonStandard/UML#attribute> .

nc:BaseTimeSeries.percentile
        rdf:type           rdf:Property ;
        rdfs:comment       "The percentile is a number where a certain percentage of scores/ranking/values of a sample fall below that number. This is a way for expressing uncertainty in the number provided." ;
        rdfs:domain        nc:BaseTimeSeries ;
        rdfs:label         "percentile"@en ;
        cims:dataType      cim:Integer ;
        cims:multiplicity  cims:M:0..1 ;
        cims:stereotype    "NC" ;
        cims:stereotype    <http://iec.ch/TC57/NonStandard/UML#attribute> .

nc:BaseTimeSeries.timeSeriesKind
        rdf:type           rdf:Property ;
        rdfs:comment       "Kind of base time series." ;
        rdfs:domain        nc:BaseTimeSeries ;
        rdfs:label         "timeSeriesKind"@en ;
        rdfs:range         nc:BaseTimeSeriesKind ;
        cims:multiplicity  cims:M:0..1 ;
        cims:stereotype    "NC" ;
        cims:stereotype    <http://iec.ch/TC57/NonStandard/UML#attribute> .

nc:BaseTimeSeriesKind
        rdf:type                rdfs:Class ;
        rdfs:comment            "Kind of time series. " ;
        rdfs:label              "BaseTimeSeriesKind"@en ;
        cims:belongsToCategory  shs:Package_SteadyStateHypothesisScheduleProfile ;
        cims:stereotype         "NC" ;
        cims:stereotype         <http://iec.ch/TC57/NonStandard/UML#enumeration> .

nc:BaseTimeSeriesKind.actual
        rdf:type         nc:BaseTimeSeriesKind ;
        rdfs:comment     "Time series is actual data. The values represent measured or calculated values that represent the actual behaviour. " ;
        rdfs:label       "actual"@en ;
        cims:stereotype  "enum" .

nc:BaseTimeSeriesKind.forecast
        rdf:type         nc:BaseTimeSeriesKind ;
        rdfs:comment     "Time series is forecast data. The values represent the result of scientific predictions based on historical time stamped data." ;
        rdfs:label       "forecast"@en ;
        cims:stereotype  "enum" .

nc:BaseTimeSeriesKind.hindcast
        rdf:type         nc:BaseTimeSeriesKind ;
        rdfs:comment     "Time series is hindcast data. The value represent probable past (historic) condition given by calculation done using actual values. For instance, determine the among of wind based on the energy produced by wind. However, hindcast is typical the result of a simulated forecasts for historical periods." ;
        rdfs:label       "hindcast"@en ;
        cims:stereotype  "enum" .

nc:BaseTimeSeriesKind.schedule
        rdf:type         nc:BaseTimeSeriesKind ;
        rdfs:comment     "Time series is schedule data. The values represent the result of a committed and plan forecast data that has been through a quality control and could incur penalty when not followed." ;
        rdfs:label       "schedule"@en ;
        cims:stereotype  "enum" .

nc:BatteryUnit.BatteryUnitSchedule
        rdf:type              rdf:Property ;
        rdfs:comment          "Battery unit schedule associated with a battery unit." ;
        rdfs:domain           cim:BatteryUnit ;
        rdfs:label            "BatteryUnitSchedule"@en ;
        rdfs:range            nc:BatteryUnitSchedule ;
        cims:AssociationUsed  "No" ;
        cims:inverseRoleName  nc:BatteryUnitSchedule.BatteryUnit ;
        cims:multiplicity     cims:M:0..n ;
        cims:stereotype       "NC" .

nc:BatteryUnitSchedule
        rdf:type                rdfs:Class ;
        rdfs:comment            "Schedule for battery unit." ;
        rdfs:label              "BatteryUnitSchedule"@en ;
        rdfs:subClassOf         nc:BaseIrregularTimeSeries ;
        cims:belongsToCategory  shs:Package_SteadyStateHypothesisScheduleProfile ;
        cims:stereotype         "NC" ;
        cims:stereotype         <http://iec.ch/TC57/NonStandard/UML#concrete> .

nc:BatteryUnitSchedule.BatteryUnit
        rdf:type              rdf:Property ;
        rdfs:comment          "Battery unit which has battery unit schedules." ;
        rdfs:domain           nc:BatteryUnitSchedule ;
        rdfs:label            "BatteryUnit"@en ;
        rdfs:range            cim:BatteryUnit ;
        cims:AssociationUsed  "Yes" ;
        cims:inverseRoleName  nc:BatteryUnit.BatteryUnitSchedule ;
        cims:multiplicity     cims:M:0..1 ;
        cims:stereotype       "NC" .

nc:BatteryUnitSchedule.BatteryUnitTimePoint
        rdf:type              rdf:Property ;
        rdfs:comment          "The time point that relates to this battery unit schedule." ;
        rdfs:domain           nc:BatteryUnitSchedule ;
        rdfs:label            "BatteryUnitTimePoint"@en ;
        rdfs:range            nc:BatteryUnitTimePoint ;
        cims:AssociationUsed  "No" ;
        cims:inverseRoleName  nc:BatteryUnitTimePoint.BatteryUnitSchedule ;
        cims:multiplicity     cims:M:1..n ;
        cims:stereotype       "NC" ;
        cims:stereotype       <http://iec.ch/TC57/NonStandard/UML#ofAggregate> .

nc:BatteryUnitTimePoint
        rdf:type                rdfs:Class ;
        rdfs:comment            "Battery unit values for a given point in time." ;
        rdfs:label              "BatteryUnitTimePoint"@en ;
        cims:belongsToCategory  shs:Package_SteadyStateHypothesisScheduleProfile ;
        cims:stereotype         "NC" ;
        cims:stereotype         <http://iec.ch/TC57/NonStandard/UML#concrete> .

nc:BatteryUnitTimePoint.BatteryUnitSchedule
        rdf:type              rdf:Property ;
        rdfs:comment          "The battery unit schedule that has this time point." ;
        rdfs:domain           nc:BatteryUnitTimePoint ;
        rdfs:label            "BatteryUnitSchedule"@en ;
        rdfs:range            nc:BatteryUnitSchedule ;
        cims:AssociationUsed  "Yes" ;
        cims:inverseRoleName  nc:BatteryUnitSchedule.BatteryUnitTimePoint ;
        cims:multiplicity     cims:M:1 ;
        cims:stereotype       "NC" .

nc:BatteryUnitTimePoint.atTime
        rdf:type           rdf:Property ;
        rdfs:comment       "The time the data is valid for." ;
        rdfs:domain        nc:BatteryUnitTimePoint ;
        rdfs:label         "atTime"@en ;
        cims:dataType      cim:DateTime ;
        cims:multiplicity  cims:M:1..1 ;
        cims:stereotype    "NC" ;
        cims:stereotype    <http://iec.ch/TC57/NonStandard/UML#attribute> .

nc:BatteryUnitTimePoint.batteryState
        rdf:type           rdf:Property ;
        rdfs:comment       "The current state of the battery (charging, full, etc.)." ;
        rdfs:domain        nc:BatteryUnitTimePoint ;
        rdfs:label         "batteryState"@en ;
        rdfs:range         cim:BatteryStateKind ;
        cims:multiplicity  cims:M:1..1 ;
        cims:stereotype    "NC" ;
        cims:stereotype    <http://iec.ch/TC57/NonStandard/UML#attribute> .

nc:BatteryUnitTimePoint.storedE
        rdf:type           rdf:Property ;
        rdfs:comment       "Amount of energy currently stored. The attribute shall be a positive value or zero and lower than BatteryUnit.ratedE." ;
        rdfs:domain        nc:BatteryUnitTimePoint ;
        rdfs:label         "storedE"@en ;
        cims:dataType      cim:RealEnergy ;
        cims:multiplicity  cims:M:1..1 ;
        cims:stereotype    "NC" ;
        cims:stereotype    <http://iec.ch/TC57/NonStandard/UML#attribute> .

nc:ControlArea.ControlAreaRegularSchedule
        rdf:type              rdf:Property ;
        rdfs:comment          "ControlAreaRegularSchedule which belongs to a control area." ;
        rdfs:domain           cim:ControlArea ;
        rdfs:label            "ControlAreaRegularSchedule"@en ;
        rdfs:range            nc:ControlAreaRegularSchedule ;
        cims:AssociationUsed  "No" ;
        cims:inverseRoleName  nc:ControlAreaRegularSchedule.ControlArea ;
        cims:multiplicity     cims:M:0..n ;
        cims:stereotype       "NC" .

nc:ControlArea.ControlAreaSchedule
        rdf:type              rdf:Property ;
        rdfs:comment          "Control area schedule associated with a control area." ;
        rdfs:domain           cim:ControlArea ;
        rdfs:label            "ControlAreaSchedule"@en ;
        rdfs:range            nc:ControlAreaSchedule ;
        cims:AssociationUsed  "No" ;
        cims:inverseRoleName  nc:ControlAreaSchedule.ControlArea ;
        cims:multiplicity     cims:M:0..n ;
        cims:stereotype       "NC" .

nc:ControlAreaRegularSchedule
        rdf:type                rdfs:Class ;
        rdfs:comment            "Regular schedule for control area." ;
        rdfs:label              "ControlAreaRegularSchedule"@en ;
        rdfs:subClassOf         nc:BaseRegularIntervalSchedule ;
        cims:belongsToCategory  shs:Package_SteadyStateHypothesisScheduleProfile ;
        cims:stereotype         "NC" ;
        cims:stereotype         <http://iec.ch/TC57/NonStandard/UML#concrete> .

nc:ControlAreaRegularSchedule.ControlArea
        rdf:type              rdf:Property ;
        rdfs:comment          "ControlArea which has ControlAreaRegularSchedule." ;
        rdfs:domain           nc:ControlAreaRegularSchedule ;
        rdfs:label            "ControlArea"@en ;
        rdfs:range            cim:ControlArea ;
        cims:AssociationUsed  "Yes" ;
        cims:inverseRoleName  nc:ControlArea.ControlAreaRegularSchedule ;
        cims:multiplicity     cims:M:0..1 ;
        cims:stereotype       "NC" .

nc:ControlAreaRegularSchedule.netInterchange
        rdf:type           rdf:Property ;
        rdfs:comment       "The specified positive net interchange into the control area, i.e. positive sign means flow into the area." ;
        rdfs:domain        nc:ControlAreaRegularSchedule ;
        rdfs:label         "netInterchange"@en ;
        cims:dataType      cim:ActivePower ;
        cims:multiplicity  cims:M:1..1 ;
        cims:stereotype    "NC" ;
        cims:stereotype    <http://iec.ch/TC57/NonStandard/UML#attribute> .

nc:ControlAreaRegularSchedule.pTolerance
        rdf:type           rdf:Property ;
        rdfs:comment       "Active power net interchange tolerance. The attribute shall be a positive value or zero." ;
        rdfs:domain        nc:ControlAreaRegularSchedule ;
        rdfs:label         "pTolerance"@en ;
        cims:dataType      cim:ActivePower ;
        cims:multiplicity  cims:M:0..1 ;
        cims:stereotype    "NC" ;
        cims:stereotype    <http://iec.ch/TC57/NonStandard/UML#attribute> .

nc:ControlAreaSchedule
        rdf:type                rdfs:Class ;
        rdfs:comment            "Schedule for control area." ;
        rdfs:label              "ControlAreaSchedule"@en ;
        rdfs:subClassOf         nc:BaseIrregularTimeSeries ;
        cims:belongsToCategory  shs:Package_SteadyStateHypothesisScheduleProfile ;
        cims:stereotype         "NC" ;
        cims:stereotype         <http://iec.ch/TC57/NonStandard/UML#concrete> .

nc:ControlAreaSchedule.ControlArea
        rdf:type              rdf:Property ;
        rdfs:comment          "Control area which has control area schedules." ;
        rdfs:domain           nc:ControlAreaSchedule ;
        rdfs:label            "ControlArea"@en ;
        rdfs:range            cim:ControlArea ;
        cims:AssociationUsed  "Yes" ;
        cims:inverseRoleName  nc:ControlArea.ControlAreaSchedule ;
        cims:multiplicity     cims:M:0..1 ;
        cims:stereotype       "NC" .

nc:ControlAreaSchedule.ControlAreaTimePoint
        rdf:type              rdf:Property ;
        rdfs:comment          "The time point that relates to this control area schedule." ;
        rdfs:domain           nc:ControlAreaSchedule ;
        rdfs:label            "ControlAreaTimePoint"@en ;
        rdfs:range            nc:ControlAreaTimePoint ;
        cims:AssociationUsed  "No" ;
        cims:inverseRoleName  nc:ControlAreaTimePoint.ControlAreaSchedule ;
        cims:multiplicity     cims:M:1..n ;
        cims:stereotype       "NC" ;
        cims:stereotype       <http://iec.ch/TC57/NonStandard/UML#ofAggregate> .

nc:ControlAreaTimePoint
        rdf:type                rdfs:Class ;
        rdfs:comment            "Participation factor for a given point in time." ;
        rdfs:label              "ControlAreaTimePoint"@en ;
        cims:belongsToCategory  shs:Package_SteadyStateHypothesisScheduleProfile ;
        cims:stereotype         "NC" ;
        cims:stereotype         <http://iec.ch/TC57/NonStandard/UML#concrete> .

nc:ControlAreaTimePoint.ControlAreaSchedule
        rdf:type              rdf:Property ;
        rdfs:comment          "The control area schedule that has this time point." ;
        rdfs:domain           nc:ControlAreaTimePoint ;
        rdfs:label            "ControlAreaSchedule"@en ;
        rdfs:range            nc:ControlAreaSchedule ;
        cims:AssociationUsed  "Yes" ;
        cims:inverseRoleName  nc:ControlAreaSchedule.ControlAreaTimePoint ;
        cims:multiplicity     cims:M:1 ;
        cims:stereotype       "NC" .

nc:ControlAreaTimePoint.atTime
        rdf:type           rdf:Property ;
        rdfs:comment       "The time the data is valid for." ;
        rdfs:domain        nc:ControlAreaTimePoint ;
        rdfs:label         "atTime"@en ;
        cims:dataType      cim:DateTime ;
        cims:multiplicity  cims:M:1..1 ;
        cims:stereotype    "NC" ;
        cims:stereotype    <http://iec.ch/TC57/NonStandard/UML#attribute> .

nc:ControlAreaTimePoint.netInterchange
        rdf:type           rdf:Property ;
        rdfs:comment       "The specified positive net interchange into the control area, i.e. positive sign means flow into the area." ;
        rdfs:domain        nc:ControlAreaTimePoint ;
        rdfs:label         "netInterchange"@en ;
        cims:dataType      cim:ActivePower ;
        cims:multiplicity  cims:M:1..1 ;
        cims:stereotype    "NC" ;
        cims:stereotype    <http://iec.ch/TC57/NonStandard/UML#attribute> .

nc:ControlAreaTimePoint.pTolerance
        rdf:type           rdf:Property ;
        rdfs:comment       "Active power net interchange tolerance. The attribute shall be a positive value or zero." ;
        rdfs:domain        nc:ControlAreaTimePoint ;
        rdfs:label         "pTolerance"@en ;
        cims:dataType      cim:ActivePower ;
        cims:multiplicity  cims:M:0..1 ;
        cims:stereotype    "NC" ;
        cims:stereotype    <http://iec.ch/TC57/NonStandard/UML#attribute> .

nc:CsConverter.CsConverterSchedule
        rdf:type              rdf:Property ;
        rdfs:comment          "Cs converter schedule associated with a control area." , "CsConverterRegularSchedule which belongs to a CSConverter." ;
        rdfs:domain           cim:CsConverter ;
        rdfs:label            "CsConverterSchedule"@en ;
        rdfs:range            nc:CsConverterRegularSchedule , nc:CsConverterSchedule ;
        cims:AssociationUsed  "No" ;
        cims:inverseRoleName  nc:CsConverterRegularSchedule.CsConverter , nc:CsConverterSchedule.CsConverter ;
        cims:multiplicity     cims:M:0..n ;
        cims:stereotype       "NC" .

nc:CsConverterRegularSchedule
        rdf:type                rdfs:Class ;
        rdfs:comment            "Regular schedule for CS converter." ;
        rdfs:label              "CsConverterRegularSchedule"@en ;
        rdfs:subClassOf         nc:ACDCConverterRegularSchedule ;
        cims:belongsToCategory  shs:Package_SteadyStateHypothesisScheduleProfile ;
        cims:stereotype         "NC" ;
        cims:stereotype         <http://iec.ch/TC57/NonStandard/UML#concrete> .

nc:CsConverterRegularSchedule.CsConverter
        rdf:type              rdf:Property ;
        rdfs:comment          "CsConverter which has CsConverterRegularSchedule." ;
        rdfs:domain           nc:CsConverterRegularSchedule ;
        rdfs:label            "CsConverter"@en ;
        rdfs:range            cim:CsConverter ;
        cims:AssociationUsed  "Yes" ;
        cims:inverseRoleName  nc:CsConverter.CsConverterSchedule ;
        cims:multiplicity     cims:M:0..1 ;
        cims:stereotype       "NC" .

nc:CsConverterRegularSchedule.operatingMode
        rdf:type           rdf:Property ;
        rdfs:comment       "Indicates whether the DC pole is operating as an inverter or as a rectifier. It is converter’s control variable used in power flow." ;
        rdfs:domain        nc:CsConverterRegularSchedule ;
        rdfs:label         "operatingMode"@en ;
        rdfs:range         cim:CsOperatingModeKind ;
        cims:multiplicity  cims:M:1..1 ;
        cims:stereotype    "NC" ;
        cims:stereotype    <http://iec.ch/TC57/NonStandard/UML#attribute> .

nc:CsConverterRegularSchedule.pPccControl
        rdf:type           rdf:Property ;
        rdfs:comment       "Kind of active power control." ;
        rdfs:domain        nc:CsConverterRegularSchedule ;
        rdfs:label         "pPccControl"@en ;
        rdfs:range         cim:CsPpccControlKind ;
        cims:multiplicity  cims:M:1..1 ;
        cims:stereotype    "NC" ;
        cims:stereotype    <http://iec.ch/TC57/NonStandard/UML#attribute> .

nc:CsConverterRegularSchedule.targetAlpha
        rdf:type           rdf:Property ;
        rdfs:comment       "Target firing angle. It is converter’s control variable used in power flow. It is only applicable for rectifier if continuous tap changer control is used. Allowed values are within the range minAlpha&lt;=targetAlpha&lt;=maxAlpha. The attribute shall be a positive value." ;
        rdfs:domain        nc:CsConverterRegularSchedule ;
        rdfs:label         "targetAlpha"@en ;
        cims:dataType      cim:AngleDegrees ;
        cims:multiplicity  cims:M:0..1 ;
        cims:stereotype    "NC" ;
        cims:stereotype    <http://iec.ch/TC57/NonStandard/UML#attribute> .

nc:CsConverterRegularSchedule.targetGamma
        rdf:type           rdf:Property ;
        rdfs:comment       "Target extinction angle. It is converter’s control variable used in power flow. It is only applicable for inverter if continuous tap changer control is used. Allowed values are within the range minGamma&lt;=targetGamma&lt;=maxGamma. The attribute shall be a positive value." ;
        rdfs:domain        nc:CsConverterRegularSchedule ;
        rdfs:label         "targetGamma"@en ;
        cims:dataType      cim:AngleDegrees ;
        cims:multiplicity  cims:M:0..1 ;
        cims:stereotype    "NC" ;
        cims:stereotype    <http://iec.ch/TC57/NonStandard/UML#attribute> .

nc:CsConverterRegularSchedule.targetIdc
        rdf:type           rdf:Property ;
        rdfs:comment       "DC current target value. It is converter’s control variable used in power flow. The attribute shall be a positive value." ;
        rdfs:domain        nc:CsConverterRegularSchedule ;
        rdfs:label         "targetIdc"@en ;
        cims:dataType      cim:CurrentFlow ;
        cims:multiplicity  cims:M:0..1 ;
        cims:stereotype    "NC" ;
        cims:stereotype    <http://iec.ch/TC57/NonStandard/UML#attribute> .

nc:CsConverterSchedule
        rdf:type                rdfs:Class ;
        rdfs:comment            "Schedule for CS converter." ;
        rdfs:label              "CsConverterSchedule"@en ;
        rdfs:subClassOf         nc:BaseIrregularTimeSeries ;
        cims:belongsToCategory  shs:Package_SteadyStateHypothesisScheduleProfile ;
        cims:stereotype         "NC" ;
        cims:stereotype         <http://iec.ch/TC57/NonStandard/UML#concrete> .

nc:CsConverterSchedule.CsConverter
        rdf:type              rdf:Property ;
        rdfs:comment          "Cs converter which has Cs converter schedules." ;
        rdfs:domain           nc:CsConverterSchedule ;
        rdfs:label            "CsConverter"@en ;
        rdfs:range            cim:CsConverter ;
        cims:AssociationUsed  "Yes" ;
        cims:inverseRoleName  nc:CsConverter.CsConverterSchedule ;
        cims:multiplicity     cims:M:0..1 ;
        cims:stereotype       "NC" .

nc:CsConverterSchedule.CsConverterTimePoint
        rdf:type              rdf:Property ;
        rdfs:comment          "The time point that relates to this CS converter schedule." ;
        rdfs:domain           nc:CsConverterSchedule ;
        rdfs:label            "CsConverterTimePoint"@en ;
        rdfs:range            nc:CsConverterTimePoint ;
        cims:AssociationUsed  "No" ;
        cims:inverseRoleName  nc:CsConverterTimePoint.CsConverterSchedule ;
        cims:multiplicity     cims:M:1..n ;
        cims:stereotype       "NC" ;
        cims:stereotype       <http://iec.ch/TC57/NonStandard/UML#ofAggregate> .

nc:CsConverterTimePoint
        rdf:type                rdfs:Class ;
        rdfs:comment            "CSConverter values for a given point in time." ;
        rdfs:label              "CsConverterTimePoint"@en ;
        rdfs:subClassOf         nc:ACDCTimePoint ;
        cims:belongsToCategory  shs:Package_SteadyStateHypothesisScheduleProfile ;
        cims:stereotype         "NC" ;
        cims:stereotype         <http://iec.ch/TC57/NonStandard/UML#concrete> .

nc:CsConverterTimePoint.CsConverterSchedule
        rdf:type              rdf:Property ;
        rdfs:comment          "The CS converter schedule that has this time point." ;
        rdfs:domain           nc:CsConverterTimePoint ;
        rdfs:label            "CsConverterSchedule"@en ;
        rdfs:range            nc:CsConverterSchedule ;
        cims:AssociationUsed  "Yes" ;
        cims:inverseRoleName  nc:CsConverterSchedule.CsConverterTimePoint ;
        cims:multiplicity     cims:M:1 ;
        cims:stereotype       "NC" .

nc:CsConverterTimePoint.operatingMode
        rdf:type           rdf:Property ;
        rdfs:comment       "Indicates whether the DC pole is operating as an inverter or as a rectifier. It is converter’s control variable used in power flow." ;
        rdfs:domain        nc:CsConverterTimePoint ;
        rdfs:label         "operatingMode"@en ;
        rdfs:range         cim:CsOperatingModeKind ;
        cims:multiplicity  cims:M:1..1 ;
        cims:stereotype    "NC" ;
        cims:stereotype    <http://iec.ch/TC57/NonStandard/UML#attribute> .

nc:CsConverterTimePoint.pPccControl
        rdf:type           rdf:Property ;
        rdfs:comment       "Kind of active power control." ;
        rdfs:domain        nc:CsConverterTimePoint ;
        rdfs:label         "pPccControl"@en ;
        rdfs:range         cim:CsPpccControlKind ;
        cims:multiplicity  cims:M:1..1 ;
        cims:stereotype    "NC" ;
        cims:stereotype    <http://iec.ch/TC57/NonStandard/UML#attribute> .

nc:CsConverterTimePoint.targetAlpha
        rdf:type           rdf:Property ;
        rdfs:comment       "Target firing angle. It is converter’s control variable used in power flow. It is only applicable for rectifier if continuous tap changer control is used. Allowed values are within the range minAlpha&lt;=targetAlpha&lt;=maxAlpha. The attribute shall be a positive value." ;
        rdfs:domain        nc:CsConverterTimePoint ;
        rdfs:label         "targetAlpha"@en ;
        cims:dataType      cim:AngleDegrees ;
        cims:multiplicity  cims:M:0..1 ;
        cims:stereotype    "NC" ;
        cims:stereotype    <http://iec.ch/TC57/NonStandard/UML#attribute> .

nc:CsConverterTimePoint.targetGamma
        rdf:type           rdf:Property ;
        rdfs:comment       "Target extinction angle. It is converter’s control variable used in power flow. It is only applicable for inverter if continuous tap changer control is used. Allowed values are within the range minGamma&lt;=targetGamma&lt;=maxGamma. The attribute shall be a positive value." ;
        rdfs:domain        nc:CsConverterTimePoint ;
        rdfs:label         "targetGamma"@en ;
        cims:dataType      cim:AngleDegrees ;
        cims:multiplicity  cims:M:0..1 ;
        cims:stereotype    "NC" ;
        cims:stereotype    <http://iec.ch/TC57/NonStandard/UML#attribute> .

nc:CsConverterTimePoint.targetIdc
        rdf:type           rdf:Property ;
        rdfs:comment       "DC current target value. It is converter’s control variable used in power flow. The attribute shall be a positive value." ;
        rdfs:domain        nc:CsConverterTimePoint ;
        rdfs:label         "targetIdc"@en ;
        cims:dataType      cim:CurrentFlow ;
        cims:multiplicity  cims:M:0..1 ;
        cims:stereotype    "NC" ;
        cims:stereotype    <http://iec.ch/TC57/NonStandard/UML#attribute> .

nc:CurrentLimit.CurrentLimitSchedule
        rdf:type              rdf:Property ;
        rdfs:comment          "Current limit schedule associated with a current limit." ;
        rdfs:domain           cim:CurrentLimit ;
        rdfs:label            "CurrentLimitSchedule"@en ;
        rdfs:range            nc:CurrentLimitSchedule ;
        cims:AssociationUsed  "No" ;
        cims:inverseRoleName  nc:CurrentLimitSchedule.CurrentLimit ;
        cims:multiplicity     cims:M:0..n ;
        cims:stereotype       "NC" .

nc:CurrentLimitSchedule
        rdf:type                rdfs:Class ;
        rdfs:comment            "Schedule for current limit." ;
        rdfs:label              "CurrentLimitSchedule"@en ;
        rdfs:subClassOf         nc:BaseIrregularTimeSeries ;
        cims:belongsToCategory  shs:Package_SteadyStateHypothesisScheduleProfile ;
        cims:stereotype         "NC" ;
        cims:stereotype         <http://iec.ch/TC57/NonStandard/UML#concrete> .

nc:CurrentLimitSchedule.CurrentLimit
        rdf:type              rdf:Property ;
        rdfs:comment          "Current limit which has current limit schedules." ;
        rdfs:domain           nc:CurrentLimitSchedule ;
        rdfs:label            "CurrentLimit"@en ;
        rdfs:range            cim:CurrentLimit ;
        cims:AssociationUsed  "Yes" ;
        cims:inverseRoleName  nc:CurrentLimit.CurrentLimitSchedule ;
        cims:multiplicity     cims:M:0..1 ;
        cims:stereotype       "NC" .

nc:CurrentLimitSchedule.CurrentLimitTimePoint
        rdf:type              rdf:Property ;
        rdfs:comment          "The time point that relates to this current limit schedule." ;
        rdfs:domain           nc:CurrentLimitSchedule ;
        rdfs:label            "CurrentLimitTimePoint"@en ;
        rdfs:range            nc:CurrentLimitTimePoint ;
        cims:AssociationUsed  "No" ;
        cims:inverseRoleName  nc:CurrentLimitTimePoint.CurrentLimitSchedule ;
        cims:multiplicity     cims:M:1..n ;
        cims:stereotype       "NC" ;
        cims:stereotype       <http://iec.ch/TC57/NonStandard/UML#ofAggregate> .

nc:CurrentLimitTimePoint
        rdf:type                rdfs:Class ;
        rdfs:comment            "Current limit values for a given point in time." ;
        rdfs:label              "CurrentLimitTimePoint"@en ;
        cims:belongsToCategory  shs:Package_SteadyStateHypothesisScheduleProfile ;
        cims:stereotype         "NC" ;
        cims:stereotype         <http://iec.ch/TC57/NonStandard/UML#concrete> .

nc:CurrentLimitTimePoint.CurrentLimitSchedule
        rdf:type              rdf:Property ;
        rdfs:comment          "The current limit schedule that has this time point." ;
        rdfs:domain           nc:CurrentLimitTimePoint ;
        rdfs:label            "CurrentLimitSchedule"@en ;
        rdfs:range            nc:CurrentLimitSchedule ;
        cims:AssociationUsed  "Yes" ;
        cims:inverseRoleName  nc:CurrentLimitSchedule.CurrentLimitTimePoint ;
        cims:multiplicity     cims:M:1 ;
        cims:stereotype       "NC" .

nc:CurrentLimitTimePoint.atTime
        rdf:type           rdf:Property ;
        rdfs:comment       "The time the data is valid for." ;
        rdfs:domain        nc:CurrentLimitTimePoint ;
        rdfs:label         "atTime"@en ;
        cims:dataType      cim:DateTime ;
        cims:multiplicity  cims:M:1..1 ;
        cims:stereotype    "NC" ;
        cims:stereotype    <http://iec.ch/TC57/NonStandard/UML#attribute> .

nc:CurrentLimitTimePoint.value
        rdf:type           rdf:Property ;
        rdfs:comment       "Limit on current flow. The attribute shall be a positive value or zero." ;
        rdfs:domain        nc:CurrentLimitTimePoint ;
        rdfs:label         "value"@en ;
        cims:dataType      cim:CurrentFlow ;
        cims:multiplicity  cims:M:1..1 ;
        cims:stereotype    "NC" ;
        cims:stereotype    <http://iec.ch/TC57/NonStandard/UML#attribute> .

nc:DayOfWeekKind  rdf:type      rdfs:Class ;
        rdfs:comment            "The kind of day to be included in a regular schedule." ;
        rdfs:label              "DayOfWeekKind"@en ;
        cims:belongsToCategory  shs:Package_SteadyStateHypothesisScheduleProfile ;
        cims:stereotype         "NC" ;
        cims:stereotype         <http://iec.ch/TC57/NonStandard/UML#enumeration> .

nc:DayOfWeekKind.all  rdf:type  nc:DayOfWeekKind ;
        rdfs:comment     "All days of the week." ;
        rdfs:label       "all"@en ;
        cims:stereotype  "enum" .

nc:DayOfWeekKind.bridgeDay
        rdf:type         nc:DayOfWeekKind ;
        rdfs:comment     "A day that is a gap between two distinguished days e.g holiday and weekend that leads to an abnormal scheduling behavior. e.g. if Ascension day falls on a Thursday, then Friday would be a bridge day due to the schedule will not have a normal Friday consumption and production." ;
        rdfs:label       "bridgeDay"@en ;
        cims:stereotype  "enum" .

nc:DayOfWeekKind.friday
        rdf:type         nc:DayOfWeekKind ;
        rdfs:comment     "Friday as the day of the week." ;
        rdfs:label       "friday"@en ;
        cims:stereotype  "enum" .

nc:DayOfWeekKind.holiday
        rdf:type         nc:DayOfWeekKind ;
        rdfs:label       "holiday"@en ;
        cims:stereotype  "enum" .

nc:DayOfWeekKind.monday
        rdf:type         nc:DayOfWeekKind ;
        rdfs:comment     "Monday as the day of the week." ;
        rdfs:label       "monday"@en ;
        cims:stereotype  "enum" .

nc:DayOfWeekKind.saturday
        rdf:type         nc:DayOfWeekKind ;
        rdfs:comment     "Saturday as the day of the week." ;
        rdfs:label       "saturday"@en ;
        cims:stereotype  "enum" .

nc:DayOfWeekKind.sunday
        rdf:type         nc:DayOfWeekKind ;
        rdfs:comment     "Sunday as the day of the week." ;
        rdfs:label       "sunday"@en ;
        cims:stereotype  "enum" .

nc:DayOfWeekKind.thursday
        rdf:type         nc:DayOfWeekKind ;
        rdfs:comment     "Thursday as the day of the week." ;
        rdfs:label       "thursday"@en ;
        cims:stereotype  "enum" .

nc:DayOfWeekKind.tuesday
        rdf:type         nc:DayOfWeekKind ;
        rdfs:comment     "Tuesday as the day of the week." ;
        rdfs:label       "tuesday"@en ;
        cims:stereotype  "enum" .

nc:DayOfWeekKind.wednesday
        rdf:type         nc:DayOfWeekKind ;
        rdfs:comment     "Wednesday as the day of the week." ;
        rdfs:label       "wednesday"@en ;
        cims:stereotype  "enum" .

nc:DayOfWeekKind.weekday
        rdf:type         nc:DayOfWeekKind ;
        rdfs:comment     "A day of the week other than Sunday or Saturday." ;
        rdfs:label       "weekday"@en ;
        cims:stereotype  "enum" .

nc:DayOfWeekKind.weekend
        rdf:type         nc:DayOfWeekKind ;
        rdfs:comment     "A day of the week which is Sunday or Saturday." ;
        rdfs:label       "weekend"@en ;
        cims:stereotype  "enum" .

nc:EnergyConnection.EnergyConnectionSchedule
        rdf:type              rdf:Property ;
        rdfs:comment          "Energy connection schedule associated with a Vs converter." , "EnergyConnectionSchedule which belongs to an energy connection." ;
        rdfs:domain           cim:EnergyConnection ;
        rdfs:label            "EnergyConnectionSchedule"@en ;
        rdfs:range            nc:EnergyConnectionRegularSchedule , nc:EnergyConnectionSchedule ;
        cims:AssociationUsed  "No" ;
        cims:inverseRoleName  nc:EnergyConnectionSchedule.EnergyConnection , nc:EnergyConnectionRegularSchedule.EnergyConnection ;
        cims:multiplicity     cims:M:0..n ;
        cims:stereotype       "NC" .

nc:EnergyConnectionRegularSchedule
        rdf:type                rdfs:Class ;
        rdfs:comment            "Regular schedule for energy connection." ;
        rdfs:label              "EnergyConnectionRegularSchedule"@en ;
        rdfs:subClassOf         nc:BaseRegularIntervalSchedule ;
        cims:belongsToCategory  shs:Package_SteadyStateHypothesisScheduleProfile ;
        cims:stereotype         "NC" ;
        cims:stereotype         <http://iec.ch/TC57/NonStandard/UML#concrete> .

nc:EnergyConnectionRegularSchedule.EnergyConnection
        rdf:type              rdf:Property ;
        rdfs:comment          "EnergyConnection which has EnergyConnectionSchedule." ;
        rdfs:domain           nc:EnergyConnectionRegularSchedule ;
        rdfs:label            "EnergyConnection"@en ;
        rdfs:range            cim:EnergyConnection ;
        cims:AssociationUsed  "Yes" ;
        cims:inverseRoleName  nc:EnergyConnection.EnergyConnectionSchedule ;
        cims:multiplicity     cims:M:0..1 ;
        cims:stereotype       "NC" .

nc:EnergyConnectionRegularSchedule.p
        rdf:type           rdf:Property ;
        rdfs:comment       "Active power injection. Load sign convention is used, i.e. positive sign means flow out from a node.\nStarting value for a steady state solution." ;
        rdfs:domain        nc:EnergyConnectionRegularSchedule ;
        rdfs:label         "p"@en ;
        cims:dataType      cim:ActivePower ;
        cims:multiplicity  cims:M:1..1 ;
        cims:stereotype    "NC" ;
        cims:stereotype    <http://iec.ch/TC57/NonStandard/UML#attribute> .

nc:EnergyConnectionRegularSchedule.q
        rdf:type           rdf:Property ;
        rdfs:comment       "Reactive power injection. Load sign convention is used, i.e. positive sign means flow out from a node.\nStarting value for a steady state solution." ;
        rdfs:domain        nc:EnergyConnectionRegularSchedule ;
        rdfs:label         "q"@en ;
        cims:dataType      cim:ReactivePower ;
        cims:multiplicity  cims:M:1..1 ;
        cims:stereotype    "NC" ;
        cims:stereotype    <http://iec.ch/TC57/NonStandard/UML#attribute> .

nc:EnergyConnectionSchedule
        rdf:type                rdfs:Class ;
        rdfs:comment            "Schedule for energy connection." ;
        rdfs:label              "EnergyConnectionSchedule"@en ;
        rdfs:subClassOf         nc:BaseIrregularTimeSeries ;
        cims:belongsToCategory  shs:Package_SteadyStateHypothesisScheduleProfile ;
        cims:stereotype         "NC" ;
        cims:stereotype         <http://iec.ch/TC57/NonStandard/UML#concrete> .

nc:EnergyConnectionSchedule.EnergyConnection
        rdf:type              rdf:Property ;
        rdfs:comment          "Energy connection which has energy connection schedules." ;
        rdfs:domain           nc:EnergyConnectionSchedule ;
        rdfs:label            "EnergyConnection"@en ;
        rdfs:range            cim:EnergyConnection ;
        cims:AssociationUsed  "Yes" ;
        cims:inverseRoleName  nc:EnergyConnection.EnergyConnectionSchedule ;
        cims:multiplicity     cims:M:0..1 ;
        cims:stereotype       "NC" .

nc:EnergyConnectionSchedule.EnergyConnectionTimePoint
        rdf:type              rdf:Property ;
        rdfs:comment          "The time point that relates to this energy connection schedule." ;
        rdfs:domain           nc:EnergyConnectionSchedule ;
        rdfs:label            "EnergyConnectionTimePoint"@en ;
        rdfs:range            nc:EnergyConnectionTimePoint ;
        cims:AssociationUsed  "No" ;
        cims:inverseRoleName  nc:EnergyConnectionTimePoint.EnergyConnectionSchedule ;
        cims:multiplicity     cims:M:1..n ;
        cims:stereotype       "NC" ;
        cims:stereotype       <http://iec.ch/TC57/NonStandard/UML#ofAggregate> .

nc:EnergyConnectionTimePoint
        rdf:type                rdfs:Class ;
        rdfs:comment            "Energy connection values for a given point in time." ;
        rdfs:label              "EnergyConnectionTimePoint"@en ;
        cims:belongsToCategory  shs:Package_SteadyStateHypothesisScheduleProfile ;
        cims:stereotype         "NC" ;
        cims:stereotype         <http://iec.ch/TC57/NonStandard/UML#concrete> .

nc:EnergyConnectionTimePoint.EnergyConnectionSchedule
        rdf:type              rdf:Property ;
        rdfs:comment          "The energy connection schedule that has this time point." ;
        rdfs:domain           nc:EnergyConnectionTimePoint ;
        rdfs:label            "EnergyConnectionSchedule"@en ;
        rdfs:range            nc:EnergyConnectionSchedule ;
        cims:AssociationUsed  "Yes" ;
        cims:inverseRoleName  nc:EnergyConnectionSchedule.EnergyConnectionTimePoint ;
        cims:multiplicity     cims:M:1 ;
        cims:stereotype       "NC" .

nc:EnergyConnectionTimePoint.atTime
        rdf:type           rdf:Property ;
        rdfs:comment       "The time the data is valid for." ;
        rdfs:domain        nc:EnergyConnectionTimePoint ;
        rdfs:label         "atTime"@en ;
        cims:dataType      cim:DateTime ;
        cims:multiplicity  cims:M:1..1 ;
        cims:stereotype    "NC" ;
        cims:stereotype    <http://iec.ch/TC57/NonStandard/UML#attribute> .

nc:EnergyConnectionTimePoint.p
        rdf:type           rdf:Property ;
        rdfs:comment       "Active power injection. Load sign convention is used, i.e. positive sign means flow out from a node.\nStarting value for a steady state solution." ;
        rdfs:domain        nc:EnergyConnectionTimePoint ;
        rdfs:label         "p"@en ;
        cims:dataType      cim:ActivePower ;
        cims:multiplicity  cims:M:1..1 ;
        cims:stereotype    "NC" ;
        cims:stereotype    <http://iec.ch/TC57/NonStandard/UML#attribute> .

nc:EnergyConnectionTimePoint.q
        rdf:type           rdf:Property ;
        rdfs:comment       "Reactive power injection. Load sign convention is used, i.e. positive sign means flow out from a node.\nStarting value for a steady state solution." ;
        rdfs:domain        nc:EnergyConnectionTimePoint ;
        rdfs:label         "q"@en ;
        cims:dataType      cim:ReactivePower ;
        cims:multiplicity  cims:M:1..1 ;
        cims:stereotype    "NC" ;
        cims:stereotype    <http://iec.ch/TC57/NonStandard/UML#attribute> .
nc:EnergyDemandKind  rdf:type   rdfs:Class ;
        rdfs:comment            "Kind of energy demand." ;
        rdfs:label              "EnergyDemandKind"@en ;
        cims:belongsToCategory  shs:Package_SteadyStateHypothesisScheduleProfile ;
        cims:stereotype         "NC" ;
        cims:stereotype         <http://iec.ch/TC57/NonStandard/UML#enumeration> .

nc:EnergyDemandKind.consumption
        rdf:type         nc:EnergyDemandKind ;
        rdfs:label       "consumption"@en ;
        cims:stereotype  "enum" .

nc:EnergyDemandKind.export
        rdf:type         nc:EnergyDemandKind ;
        rdfs:label       "export"@en ;
        cims:stereotype  "enum" .

nc:EnergyDemandKind.import
        rdf:type         nc:EnergyDemandKind ;
        rdfs:label       "import"@en ;
        cims:stereotype  "enum" .

nc:EnergyDemandKind.production
        rdf:type         nc:EnergyDemandKind ;
        rdfs:label       "production"@en ;
        cims:stereotype  "enum" .

nc:EnergyDemandKind.storage
        rdf:type         nc:EnergyDemandKind ;
        rdfs:label       "storage"@en ;
        cims:stereotype  "enum" .

nc:Equipment.InServiceRegularSchedule
        rdf:type              rdf:Property ;
        rdfs:comment          "InServiceRegularSchedule which belongs to an equipment." ;
        rdfs:domain           cim:Equipment ;
        rdfs:label            "InServiceRegularSchedule"@en ;
        rdfs:range            nc:InServiceRegularSchedule ;
        cims:AssociationUsed  "No" ;
        cims:inverseRoleName  nc:InServiceRegularSchedule.Equipment ;
        cims:multiplicity     cims:M:0..n ;
        cims:stereotype       "NC" .

nc:Equipment.InServiceSchedule
        rdf:type              rdf:Property ;
        rdfs:comment          "In service schedule associated with an equipment." ;
        rdfs:domain           cim:Equipment ;
        rdfs:label            "InServiceSchedule"@en ;
        rdfs:range            nc:InServiceSchedule ;
        cims:AssociationUsed  "No" ;
        cims:inverseRoleName  nc:InServiceSchedule.Equipment ;
        cims:multiplicity     cims:M:0..n ;
        cims:stereotype       "NC" .

nc:EquivalentInjection.EquivalentInjectionRegularSchedule
        rdf:type              rdf:Property ;
        rdfs:comment          "EquivalentInjectionRegularSchedule which belongs to an equivalent injection." ;
        rdfs:domain           cim:EquivalentInjection ;
        rdfs:label            "EquivalentInjectionRegularSchedule"@en ;
        rdfs:range            nc:EquivalentInjectionRegularSchedule ;
        cims:AssociationUsed  "No" ;
        cims:inverseRoleName  nc:EquivalentInjectionRegularSchedule.EquivalentInjection ;
        cims:multiplicity     cims:M:0..n ;
        cims:stereotype       "NC" .

nc:EquivalentInjection.EquivalentInjectionSchedule
        rdf:type              rdf:Property ;
        rdfs:comment          "Equivalent injection schedule associated with an equivalent injection." ;
        rdfs:domain           cim:EquivalentInjection ;
        rdfs:label            "EquivalentInjectionSchedule"@en ;
        rdfs:range            nc:EquivalentInjectionSchedule ;
        cims:AssociationUsed  "No" ;
        cims:inverseRoleName  nc:EquivalentInjectionSchedule.EquivalentInjection ;
        cims:multiplicity     cims:M:0..n ;
        cims:stereotype       "NC" .

nc:EquivalentInjectionRegularSchedule
        rdf:type                rdfs:Class ;
        rdfs:comment            "Regular schedule for equivalent injection." ;
        rdfs:label              "EquivalentInjectionRegularSchedule"@en ;
        rdfs:subClassOf         nc:BaseRegularIntervalSchedule ;
        cims:belongsToCategory  shs:Package_SteadyStateHypothesisScheduleProfile ;
        cims:stereotype         "NC" ;
        cims:stereotype         <http://iec.ch/TC57/NonStandard/UML#concrete> .

nc:EquivalentInjectionRegularSchedule.EquivalentInjection
        rdf:type              rdf:Property ;
        rdfs:comment          "EquivalentInjection which has EquivalentInjectionRegularSchedule." ;
        rdfs:domain           nc:EquivalentInjectionRegularSchedule ;
        rdfs:label            "EquivalentInjection"@en ;
        rdfs:range            cim:EquivalentInjection ;
        cims:AssociationUsed  "Yes" ;
        cims:inverseRoleName  nc:EquivalentInjection.EquivalentInjectionRegularSchedule ;
        cims:multiplicity     cims:M:0..1 ;
        cims:stereotype       "NC" .

nc:EquivalentInjectionRegularSchedule.p
        rdf:type           rdf:Property ;
        rdfs:comment       "Equivalent active power injection. Load sign convention is used, i.e. positive sign means flow out from a node.\nStarting value for steady state solutions." ;
        rdfs:domain        nc:EquivalentInjectionRegularSchedule ;
        rdfs:label         "p"@en ;
        cims:dataType      cim:ActivePower ;
        cims:multiplicity  cims:M:1..1 ;
        cims:stereotype    "NC" ;
        cims:stereotype    <http://iec.ch/TC57/NonStandard/UML#attribute> .

nc:EquivalentInjectionRegularSchedule.q
        rdf:type           rdf:Property ;
        rdfs:comment       "Equivalent reactive power injection. Load sign convention is used, i.e. positive sign means flow out from a node.\nStarting value for steady state solutions." ;
        rdfs:domain        nc:EquivalentInjectionRegularSchedule ;
        rdfs:label         "q"@en ;
        cims:dataType      cim:ReactivePower ;
        cims:multiplicity  cims:M:1..1 ;
        cims:stereotype    "NC" ;
        cims:stereotype    <http://iec.ch/TC57/NonStandard/UML#attribute> .

nc:EquivalentInjectionRegularSchedule.regulationStatus
        rdf:type           rdf:Property ;
        rdfs:comment       "Specifies the regulation status of the EquivalentInjection.  True is regulating.  False is not regulating." ;
        rdfs:domain        nc:EquivalentInjectionRegularSchedule ;
        rdfs:label         "regulationStatus"@en ;
        cims:dataType      cim:Boolean ;
        cims:multiplicity  cims:M:0..1 ;
        cims:stereotype    "NC" ;
        cims:stereotype    <http://iec.ch/TC57/NonStandard/UML#attribute> .

nc:EquivalentInjectionRegularSchedule.regulationTarget
        rdf:type           rdf:Property ;
        rdfs:comment       "The target voltage for voltage regulation. The attribute shall be a positive value." ;
        rdfs:domain        nc:EquivalentInjectionRegularSchedule ;
        rdfs:label         "regulationTarget"@en ;
        cims:dataType      cim:Voltage ;
        cims:multiplicity  cims:M:0..1 ;
        cims:stereotype    "NC" ;
        cims:stereotype    <http://iec.ch/TC57/NonStandard/UML#attribute> .

nc:EquivalentInjectionSchedule
        rdf:type                rdfs:Class ;
        rdfs:comment            "Regular schedule for equivalent injection." ;
        rdfs:label              "EquivalentInjectionSchedule"@en ;
        rdfs:subClassOf         nc:BaseIrregularTimeSeries ;
        cims:belongsToCategory  shs:Package_SteadyStateHypothesisScheduleProfile ;
        cims:stereotype         "NC" ;
        cims:stereotype         <http://iec.ch/TC57/NonStandard/UML#concrete> .

nc:EquivalentInjectionSchedule.EquivalentInjection
        rdf:type              rdf:Property ;
        rdfs:comment          "Equivalent injection which has equivalent injection schedules." ;
        rdfs:domain           nc:EquivalentInjectionSchedule ;
        rdfs:label            "EquivalentInjection"@en ;
        rdfs:range            cim:EquivalentInjection ;
        cims:AssociationUsed  "Yes" ;
        cims:inverseRoleName  nc:EquivalentInjection.EquivalentInjectionSchedule ;
        cims:multiplicity     cims:M:0..1 ;
        cims:stereotype       "NC" .

nc:EquivalentInjectionSchedule.EquivalentInjectionTimePoint
        rdf:type              rdf:Property ;
        rdfs:comment          "The time point that relates to this equivalent injection schedule." ;
        rdfs:domain           nc:EquivalentInjectionSchedule ;
        rdfs:label            "EquivalentInjectionTimePoint"@en ;
        rdfs:range            nc:EquivalentInjectionTimePoint ;
        cims:AssociationUsed  "No" ;
        cims:inverseRoleName  nc:EquivalentInjectionTimePoint.EquivalentInjectionSchedule ;
        cims:multiplicity     cims:M:1..n ;
        cims:stereotype       "NC" ;
        cims:stereotype       <http://iec.ch/TC57/NonStandard/UML#ofAggregate> .

nc:EquivalentInjectionTimePoint
        rdf:type                rdfs:Class ;
        rdfs:comment            "Equivalent injection values for a given point in time." ;
        rdfs:label              "EquivalentInjectionTimePoint"@en ;
        cims:belongsToCategory  shs:Package_SteadyStateHypothesisScheduleProfile ;
        cims:stereotype         "NC" ;
        cims:stereotype         <http://iec.ch/TC57/NonStandard/UML#concrete> .

nc:EquivalentInjectionTimePoint.EquivalentInjectionSchedule
        rdf:type              rdf:Property ;
        rdfs:comment          "The EquivalentInjection schedule that has this time point." ;
        rdfs:domain           nc:EquivalentInjectionTimePoint ;
        rdfs:label            "EquivalentInjectionSchedule"@en ;
        rdfs:range            nc:EquivalentInjectionSchedule ;
        cims:AssociationUsed  "Yes" ;
        cims:inverseRoleName  nc:EquivalentInjectionSchedule.EquivalentInjectionTimePoint ;
        cims:multiplicity     cims:M:1 ;
        cims:stereotype       "NC" .

nc:EquivalentInjectionTimePoint.atTime
        rdf:type           rdf:Property ;
        rdfs:comment       "The time the data is valid for." ;
        rdfs:domain        nc:EquivalentInjectionTimePoint ;
        rdfs:label         "atTime"@en ;
        cims:dataType      cim:DateTime ;
        cims:multiplicity  cims:M:1..1 ;
        cims:stereotype    "NC" ;
        cims:stereotype    <http://iec.ch/TC57/NonStandard/UML#attribute> .

nc:EquivalentInjectionTimePoint.p
        rdf:type           rdf:Property ;
        rdfs:comment       "Equivalent active power injection. Load sign convention is used, i.e. positive sign means flow out from a node.\nStarting value for steady state solutions." ;
        rdfs:domain        nc:EquivalentInjectionTimePoint ;
        rdfs:label         "p"@en ;
        cims:dataType      cim:ActivePower ;
        cims:multiplicity  cims:M:1..1 ;
        cims:stereotype    "NC" ;
        cims:stereotype    <http://iec.ch/TC57/NonStandard/UML#attribute> .

nc:EquivalentInjectionTimePoint.q
        rdf:type           rdf:Property ;
        rdfs:comment       "Equivalent reactive power injection. Load sign convention is used, i.e. positive sign means flow out from a node.\nStarting value for steady state solutions." ;
        rdfs:domain        nc:EquivalentInjectionTimePoint ;
        rdfs:label         "q"@en ;
        cims:dataType      cim:ReactivePower ;
        cims:multiplicity  cims:M:1..1 ;
        cims:stereotype    "NC" ;
        cims:stereotype    <http://iec.ch/TC57/NonStandard/UML#attribute> .

nc:EquivalentInjectionTimePoint.regulationStatus
        rdf:type           rdf:Property ;
        rdfs:comment       "Specifies the regulation status of the EquivalentInjection.  True is regulating.  False is not regulating." ;
        rdfs:domain        nc:EquivalentInjectionTimePoint ;
        rdfs:label         "regulationStatus"@en ;
        cims:dataType      cim:Boolean ;
        cims:multiplicity  cims:M:0..1 ;
        cims:stereotype    "NC" ;
        cims:stereotype    <http://iec.ch/TC57/NonStandard/UML#attribute> .

nc:EquivalentInjectionTimePoint.regulationTarget
        rdf:type           rdf:Property ;
        rdfs:comment       "The target voltage for voltage regulation. The attribute shall be a positive value." ;
        rdfs:domain        nc:EquivalentInjectionTimePoint ;
        rdfs:label         "regulationTarget"@en ;
        cims:dataType      cim:Voltage ;
        cims:multiplicity  cims:M:0..1 ;
        cims:stereotype    "NC" ;
        cims:stereotype    <http://iec.ch/TC57/NonStandard/UML#attribute> .

nc:ExternalNetworkInjection.ExternalNetowrkInjectionSchedule
        rdf:type              rdf:Property ;
        rdfs:comment          "External Network Injection schedule associated with an External Network Injection." ;
        rdfs:domain           cim:ExternalNetworkInjection ;
        rdfs:label            "ExternalNetowrkInjectionSchedule"@en ;
        rdfs:range            nc:ExternalNetworkInjectionSchedule ;
        cims:AssociationUsed  "No" ;
        cims:inverseRoleName  nc:ExternalNetworkInjectionSchedule.ExternalNetworkInjection ;
        cims:multiplicity     cims:M:0..n ;
        cims:stereotype       "NC" .

nc:ExternalNetworkInjection.ExternalNetworkinjectionRegularSchedule
        rdf:type              rdf:Property ;
        rdfs:comment          "ExternalNetworkinjectionRegularSchedule which belongs to a external network injection." ;
        rdfs:domain           cim:ExternalNetworkInjection ;
        rdfs:label            "ExternalNetworkinjectionRegularSchedule"@en ;
        rdfs:range            nc:ExternalNetworkInjectionRegularSchedule ;
        cims:AssociationUsed  "No" ;
        cims:inverseRoleName  nc:ExternalNetworkInjectionRegularSchedule.ExternalNetworkinjection ;
        cims:multiplicity     cims:M:0..n ;
        cims:stereotype       "NC" .

nc:ExternalNetworkInjectionRegularSchedule
        rdf:type                rdfs:Class ;
        rdfs:comment            "Regular schedule for external network injection." ;
        rdfs:label              "ExternalNetworkInjectionRegularSchedule"@en ;
        rdfs:subClassOf         nc:BaseRegularIntervalSchedule ;
        cims:belongsToCategory  shs:Package_SteadyStateHypothesisScheduleProfile ;
        cims:stereotype         "NC" ;
        cims:stereotype         <http://iec.ch/TC57/NonStandard/UML#concrete> .

nc:ExternalNetworkInjectionRegularSchedule.ExternalNetworkinjection
        rdf:type              rdf:Property ;
        rdfs:comment          "External network injection which has ExternalNetworkinjectionRegularSchedule" ;
        rdfs:domain           nc:ExternalNetworkInjectionRegularSchedule ;
        rdfs:label            "ExternalNetworkinjection"@en ;
        rdfs:range            cim:ExternalNetworkInjection ;
        cims:AssociationUsed  "Yes" ;
        cims:inverseRoleName  nc:ExternalNetworkInjection.ExternalNetworkinjectionRegularSchedule ;
        cims:multiplicity     cims:M:0..1 ;
        cims:stereotype       "NC" .

nc:ExternalNetworkInjectionRegularSchedule.p
        rdf:type           rdf:Property ;
        rdfs:comment       "Active power injection. Load sign convention is used, i.e. positive sign means flow out from a node.\nStarting value for steady state solutions." ;
        rdfs:domain        nc:ExternalNetworkInjectionRegularSchedule ;
        rdfs:label         "p"@en ;
        cims:dataType      cim:ActivePower ;
        cims:multiplicity  cims:M:1..1 ;
        cims:stereotype    "NC" ;
        cims:stereotype    <http://iec.ch/TC57/NonStandard/UML#attribute> .

nc:ExternalNetworkInjectionRegularSchedule.q
        rdf:type           rdf:Property ;
        rdfs:comment       "Reactive power injection. Load sign convention is used, i.e. positive sign means flow out from a node.\nStarting value for steady state solutions." ;
        rdfs:domain        nc:ExternalNetworkInjectionRegularSchedule ;
        rdfs:label         "q"@en ;
        cims:dataType      cim:ReactivePower ;
        cims:multiplicity  cims:M:1..1 ;
        cims:stereotype    "NC" ;
        cims:stereotype    <http://iec.ch/TC57/NonStandard/UML#attribute> .

nc:ExternalNetworkInjectionRegularSchedule.referencePriority
        rdf:type           rdf:Property ;
        rdfs:comment       "Priority of unit for use as powerflow voltage phase angle reference bus selection. 0 = don t care (default) 1 = highest priority. 2 is less than 1 and so on." ;
        rdfs:domain        nc:ExternalNetworkInjectionRegularSchedule ;
        rdfs:label         "referencePriority"@en ;
        cims:dataType      cim:Integer ;
        cims:multiplicity  cims:M:1..1 ;
        cims:stereotype    "NC" ;
        cims:stereotype    <http://iec.ch/TC57/NonStandard/UML#attribute> .

nc:ExternalNetworkInjectionSchedule
        rdf:type                rdfs:Class ;
        rdfs:comment            "Schedule for external network injection." ;
        rdfs:label              "ExternalNetworkInjectionSchedule"@en ;
        rdfs:subClassOf         nc:BaseIrregularTimeSeries ;
        cims:belongsToCategory  shs:Package_SteadyStateHypothesisScheduleProfile ;
        cims:stereotype         "NC" ;
        cims:stereotype         <http://iec.ch/TC57/NonStandard/UML#concrete> .

nc:ExternalNetworkInjectionSchedule.ExternalNetworkInjection
        rdf:type              rdf:Property ;
        rdfs:comment          "External Network Injection which has External Network Injection schedules." ;
        rdfs:domain           nc:ExternalNetworkInjectionSchedule ;
        rdfs:label            "ExternalNetworkInjection"@en ;
        rdfs:range            cim:ExternalNetworkInjection ;
        cims:AssociationUsed  "Yes" ;
        cims:inverseRoleName  nc:ExternalNetworkInjection.ExternalNetowrkInjectionSchedule ;
        cims:multiplicity     cims:M:0..1 ;
        cims:stereotype       "NC" .

nc:ExternalNetworkInjectionSchedule.ExternalNetworkinjectionTimePoint
        rdf:type              rdf:Property ;
        rdfs:comment          "The time point that relates to this external network injection schedule." ;
        rdfs:domain           nc:ExternalNetworkInjectionSchedule ;
        rdfs:label            "ExternalNetworkinjectionTimePoint"@en ;
        rdfs:range            nc:ExternalNetworkInjectionTimePoint ;
        cims:AssociationUsed  "No" ;
        cims:inverseRoleName  nc:ExternalNetworkInjectionTimePoint.ExternalNetworkInjectionSchedule ;
        cims:multiplicity     cims:M:1..n ;
        cims:stereotype       "NC" ;
        cims:stereotype       <http://iec.ch/TC57/NonStandard/UML#ofAggregate> .

nc:ExternalNetworkInjectionTimePoint
        rdf:type                rdfs:Class ;
        rdfs:comment            "External network injection values for a given point in time." ;
        rdfs:label              "ExternalNetworkInjectionTimePoint"@en ;
        cims:belongsToCategory  shs:Package_SteadyStateHypothesisScheduleProfile ;
        cims:stereotype         "NC" ;
        cims:stereotype         <http://iec.ch/TC57/NonStandard/UML#concrete> .

nc:ExternalNetworkInjectionTimePoint.ExternalNetworkInjectionSchedule
        rdf:type              rdf:Property ;
        rdfs:comment          "The external network injection schedule that has this time point." ;
        rdfs:domain           nc:ExternalNetworkInjectionTimePoint ;
        rdfs:label            "ExternalNetworkInjectionSchedule"@en ;
        rdfs:range            nc:ExternalNetworkInjectionSchedule ;
        cims:AssociationUsed  "Yes" ;
        cims:inverseRoleName  nc:ExternalNetworkInjectionSchedule.ExternalNetworkinjectionTimePoint ;
        cims:multiplicity     cims:M:1 ;
        cims:stereotype       "NC" .

nc:ExternalNetworkInjectionTimePoint.atTime
        rdf:type           rdf:Property ;
        rdfs:comment       "The time the data is valid for." ;
        rdfs:domain        nc:ExternalNetworkInjectionTimePoint ;
        rdfs:label         "atTime"@en ;
        cims:dataType      cim:DateTime ;
        cims:multiplicity  cims:M:1..1 ;
        cims:stereotype    "NC" ;
        cims:stereotype    <http://iec.ch/TC57/NonStandard/UML#attribute> .

nc:ExternalNetworkInjectionTimePoint.p
        rdf:type           rdf:Property ;
        rdfs:comment       "Active power injection. Load sign convention is used, i.e. positive sign means flow out from a node.\nStarting value for steady state solutions." ;
        rdfs:domain        nc:ExternalNetworkInjectionTimePoint ;
        rdfs:label         "p"@en ;
        cims:dataType      cim:ActivePower ;
        cims:multiplicity  cims:M:1..1 ;
        cims:stereotype    "NC" ;
        cims:stereotype    <http://iec.ch/TC57/NonStandard/UML#attribute> .

nc:ExternalNetworkInjectionTimePoint.q
        rdf:type           rdf:Property ;
        rdfs:comment       "Reactive power injection. Load sign convention is used, i.e. positive sign means flow out from a node.\nStarting value for steady state solutions." ;
        rdfs:domain        nc:ExternalNetworkInjectionTimePoint ;
        rdfs:label         "q"@en ;
        cims:dataType      cim:ReactivePower ;
        cims:multiplicity  cims:M:1..1 ;
        cims:stereotype    "NC" ;
        cims:stereotype    <http://iec.ch/TC57/NonStandard/UML#attribute> .

nc:ExternalNetworkInjectionTimePoint.referencePriority
        rdf:type           rdf:Property ;
        rdfs:comment       "Priority of unit for use as powerflow voltage phase angle reference bus selection. 0 = don t care (default) 1 = highest priority. 2 is less than 1 and so on." ;
        rdfs:domain        nc:ExternalNetworkInjectionTimePoint ;
        rdfs:label         "referencePriority"@en ;
        cims:dataType      cim:Integer ;
        cims:multiplicity  cims:M:1..1 ;
        cims:stereotype    "NC" ;
        cims:stereotype    <http://iec.ch/TC57/NonStandard/UML#attribute> .

nc:GeneratingUnit.GeneratingUnitSchedule
        rdf:type              rdf:Property ;
        rdfs:comment          "Generating unit schedule associated with a generating unit." ;
        rdfs:domain           cim:GeneratingUnit ;
        rdfs:label            "GeneratingUnitSchedule"@en ;
        rdfs:range            nc:GeneratingUnitSchedule ;
        cims:AssociationUsed  "No" ;
        cims:inverseRoleName  nc:GeneratingUnitSchedule.GeneratingUnit ;
        cims:multiplicity     cims:M:0..n ;
        cims:stereotype       "NC" .

nc:GeneratingUnitSchedule
        rdf:type                rdfs:Class ;
        rdfs:comment            "Schedule for generating unit." ;
        rdfs:label              "GeneratingUnitSchedule"@en ;
        rdfs:subClassOf         nc:BaseIrregularTimeSeries ;
        cims:belongsToCategory  shs:Package_SteadyStateHypothesisScheduleProfile ;
        cims:stereotype         "NC" ;
        cims:stereotype         <http://iec.ch/TC57/NonStandard/UML#concrete> .

nc:GeneratingUnitSchedule.GeneratingUnit
        rdf:type              rdf:Property ;
        rdfs:comment          "Generating unit which has generating unit schedules." ;
        rdfs:domain           nc:GeneratingUnitSchedule ;
        rdfs:label            "GeneratingUnit"@en ;
        rdfs:range            cim:GeneratingUnit ;
        cims:AssociationUsed  "Yes" ;
        cims:inverseRoleName  nc:GeneratingUnit.GeneratingUnitSchedule ;
        cims:multiplicity     cims:M:0..1 ;
        cims:stereotype       "NC" .

nc:GeneratingUnitSchedule.GeneratingUnitTimePoint
        rdf:type              rdf:Property ;
        rdfs:comment          "The time point that relates to this generating unit schedule." ;
        rdfs:domain           nc:GeneratingUnitSchedule ;
        rdfs:label            "GeneratingUnitTimePoint"@en ;
        rdfs:range            nc:GeneratingUnitTimePoint ;
        cims:AssociationUsed  "No" ;
        cims:inverseRoleName  nc:GeneratingUnitTimePoint.GeneratingUnitSchedule ;
        cims:multiplicity     cims:M:1..n ;
        cims:stereotype       <http://iec.ch/TC57/NonStandard/UML#ofAggregate> .

nc:GeneratingUnitTimePoint
        rdf:type                rdfs:Class ;
        rdfs:comment            "Generating unit values for a given point in time." ;
        rdfs:label              "GeneratingUnitTimePoint"@en ;
        cims:belongsToCategory  shs:Package_SteadyStateHypothesisScheduleProfile ;
        cims:stereotype         "NC" ;
        cims:stereotype         <http://iec.ch/TC57/NonStandard/UML#concrete> .

nc:GeneratingUnitTimePoint.GeneratingUnitSchedule
        rdf:type              rdf:Property ;
        rdfs:comment          "The generating unit schedule that has this time point." ;
        rdfs:domain           nc:GeneratingUnitTimePoint ;
        rdfs:label            "GeneratingUnitSchedule"@en ;
        rdfs:range            nc:GeneratingUnitSchedule ;
        cims:AssociationUsed  "Yes" ;
        cims:inverseRoleName  nc:GeneratingUnitSchedule.GeneratingUnitTimePoint ;
        cims:multiplicity     cims:M:1 .

nc:GeneratingUnitTimePoint.atTime
        rdf:type           rdf:Property ;
        rdfs:comment       "The time the data is valid for." ;
        rdfs:domain        nc:GeneratingUnitTimePoint ;
        rdfs:label         "atTime"@en ;
        cims:dataType      cim:DateTime ;
        cims:multiplicity  cims:M:1..1 ;
        cims:stereotype    "NC" ;
        cims:stereotype    <http://iec.ch/TC57/NonStandard/UML#attribute> .

nc:GeneratingUnitTimePoint.normalPF
        rdf:type           rdf:Property ;
        rdfs:comment       "Generating unit economic participation factor.  The sum of the participation factors across generating units does not have to sum to one.  It is used for representing distributed slack participation factor. The attribute shall be a positive value or zero." ;
        rdfs:domain        nc:GeneratingUnitTimePoint ;
        rdfs:label         "normalPF"@en ;
        cims:dataType      cim:Float ;
        cims:multiplicity  cims:M:1..1 ;
        cims:stereotype    "NC" ;
        cims:stereotype    <http://iec.ch/TC57/NonStandard/UML#attribute> .

nc:HourPattern  rdf:type        rdfs:Class ;
        rdfs:comment            "A period of the day with a given pattern." ;
        rdfs:label              "HourPattern"@en ;
        rdfs:subClassOf         cim:IdentifiedObject ;
        cims:belongsToCategory  shs:Package_SteadyStateHypothesisScheduleProfile ;
        cims:stereotype         "NC" ;
        cims:stereotype         <http://iec.ch/TC57/NonStandard/UML#concrete> .

nc:HourPattern.BaseRegularIntervalSchedule
        rdf:type              rdf:Property ;
        rdfs:comment          "Base regulat interval schedule which belongs to an hour pattern." ;
        rdfs:domain           nc:HourPattern ;
        rdfs:label            "BaseRegularIntervalSchedule"@en ;
        rdfs:range            nc:BaseRegularIntervalSchedule ;
        cims:AssociationUsed  "No" ;
        cims:inverseRoleName  nc:BaseRegularIntervalSchedule.HourPattern ;
        cims:multiplicity     cims:M:0..n ;
        cims:stereotype       "NC" .

nc:HourPattern.HourPeriod
        rdf:type              rdf:Property ;
        rdfs:comment          "Hour period which belongs to an hour pattern." ;
        rdfs:domain           nc:HourPattern ;
        rdfs:label            "HourPeriod"@en ;
        rdfs:range            nc:HourPeriod ;
        cims:AssociationUsed  "No" ;
        cims:inverseRoleName  nc:HourPeriod.HourPattern ;
        cims:multiplicity     cims:M:1..n ;
        cims:stereotype       "NC" .

nc:HourPattern.energyDemandKind
        rdf:type           rdf:Property ;
        rdfs:domain        nc:HourPattern ;
        rdfs:label         "energyDemandKind"@en ;
        rdfs:range         nc:EnergyDemandKind ;
        cims:multiplicity  cims:M:0..1 ;
        cims:stereotype    "NC" ;
        cims:stereotype    <http://iec.ch/TC57/NonStandard/UML#attribute> .

nc:HourPattern.peakKind
        rdf:type           rdf:Property ;
        rdfs:comment       "Kind of peak for a given hour pattern." ;
        rdfs:domain        nc:HourPattern ;
        rdfs:label         "peakKind"@en ;
        rdfs:range         nc:PeakKind ;
        cims:multiplicity  cims:M:0..1 ;
        cims:stereotype    "NC" ;
        cims:stereotype    <http://iec.ch/TC57/NonStandard/UML#attribute> .

nc:HourPeriod  rdf:type         rdfs:Class ;
        rdfs:label              "HourPeriod"@en ;
        cims:belongsToCategory  shs:Package_SteadyStateHypothesisScheduleProfile ;
        cims:stereotype         "NC" ;
        cims:stereotype         <http://iec.ch/TC57/NonStandard/UML#concrete> .

nc:HourPeriod.HourPattern
        rdf:type              rdf:Property ;
        rdfs:comment          "HourPattern which has some hour periods." ;
        rdfs:domain           nc:HourPeriod ;
        rdfs:label            "HourPattern"@en ;
        rdfs:range            nc:HourPattern ;
        cims:AssociationUsed  "Yes" ;
        cims:inverseRoleName  nc:HourPattern.HourPeriod ;
        cims:multiplicity     cims:M:1 ;
        cims:stereotype       "NC" .

nc:HourPeriod.endTime
        rdf:type           rdf:Property ;
        rdfs:domain        nc:HourPeriod ;
        rdfs:label         "endTime"@en ;
        cims:dataType      cim:Time ;
        cims:multiplicity  cims:M:1..1 ;
        cims:stereotype    "NC" ;
        cims:stereotype    <http://iec.ch/TC57/NonStandard/UML#attribute> .

nc:HourPeriod.mRID  rdf:type  rdf:Property ;
        rdfs:comment       "Master resource identifier issued by a model authority. The mRID is unique within an exchange context. Global uniqueness is easily achieved by using a UUID, as specified in RFC 4122, for the mRID. The use of UUID is strongly recommended.\nFor CIMXML data files in RDF syntax conforming to IEC 61970-552, the mRID is mapped to rdf:ID or rdf:about attributes that identify CIM object elements." ;
        rdfs:domain        nc:HourPeriod ;
        rdfs:label         "mRID"@en ;
        cims:dataType      cim:String ;
        cims:multiplicity  cims:M:1..1 ;
        cims:stereotype    "NC" ;
        cims:stereotype    <http://iec.ch/TC57/NonStandard/UML#attribute> .

nc:HourPeriod.startTime
        rdf:type           rdf:Property ;
        rdfs:domain        nc:HourPeriod ;
        rdfs:label         "startTime"@en ;
        cims:dataType      cim:Time ;
        cims:multiplicity  cims:M:1..1 ;
        cims:stereotype    "NC" ;
        cims:stereotype    <http://iec.ch/TC57/NonStandard/UML#attribute> .

nc:InServiceRegularSchedule
        rdf:type                rdfs:Class ;
        rdfs:comment            "Regular schedule for elements having in service." ;
        rdfs:label              "InServiceRegularSchedule"@en ;
        rdfs:subClassOf         nc:BaseRegularIntervalSchedule ;
        cims:belongsToCategory  shs:Package_SteadyStateHypothesisScheduleProfile ;
        cims:stereotype         "NC" ;
        cims:stereotype         <http://iec.ch/TC57/NonStandard/UML#concrete> .

nc:InServiceRegularSchedule.Equipment
        rdf:type              rdf:Property ;
        rdfs:comment          "Equipment which has InServiceRegularSchedule." ;
        rdfs:domain           nc:InServiceRegularSchedule ;
        rdfs:label            "Equipment"@en ;
        rdfs:range            cim:Equipment ;
        cims:AssociationUsed  "Yes" ;
        cims:inverseRoleName  nc:Equipment.InServiceRegularSchedule ;
        cims:multiplicity     cims:M:0..1 ;
        cims:stereotype       "NC" .

nc:InServiceRegularSchedule.inService
        rdf:type           rdf:Property ;
        rdfs:comment       "Specifies the availability of the equipment. True means the equipment is available for topology processing, which determines if the equipment is energized or not. False means that the equipment is treated by network applications as if it is not in the model." ;
        rdfs:domain        nc:InServiceRegularSchedule ;
        rdfs:label         "inService"@en ;
        cims:dataType      cim:Boolean ;
        cims:multiplicity  cims:M:1..1 ;
        cims:stereotype    "NC" ;
        cims:stereotype    <http://iec.ch/TC57/NonStandard/UML#attribute> .

nc:InServiceSchedule  rdf:type  rdfs:Class ;
        rdfs:comment            "Schedule for elements having in service." ;
        rdfs:label              "InServiceSchedule"@en ;
        rdfs:subClassOf         nc:BaseIrregularTimeSeries ;
        cims:belongsToCategory  shs:Package_SteadyStateHypothesisScheduleProfile ;
        cims:stereotype         "NC" ;
        cims:stereotype         <http://iec.ch/TC57/NonStandard/UML#concrete> .

nc:InServiceSchedule.Equipment
        rdf:type              rdf:Property ;
        rdfs:comment          "Equipment which has equipment schedules." ;
        rdfs:domain           nc:InServiceSchedule ;
        rdfs:label            "Equipment"@en ;
        rdfs:range            cim:Equipment ;
        cims:AssociationUsed  "Yes" ;
        cims:inverseRoleName  nc:Equipment.InServiceSchedule ;
        cims:multiplicity     cims:M:0..1 ;
        cims:stereotype       "NC" .

nc:InServiceSchedule.InServiceTimePoint
        rdf:type              rdf:Property ;
        rdfs:comment          "The time point that relates to this in service schedule." ;
        rdfs:domain           nc:InServiceSchedule ;
        rdfs:label            "InServiceTimePoint"@en ;
        rdfs:range            nc:InServiceTimePoint ;
        cims:AssociationUsed  "No" ;
        cims:inverseRoleName  nc:InServiceTimePoint.InServiceSchedule ;
        cims:multiplicity     cims:M:1..n ;
        cims:stereotype       "NC" ;
        cims:stereotype       <http://iec.ch/TC57/NonStandard/UML#ofAggregate> .

nc:InServiceTimePoint
        rdf:type                rdfs:Class ;
        rdfs:comment            "In service values for a given point in time." ;
        rdfs:label              "InServiceTimePoint"@en ;
        cims:belongsToCategory  shs:Package_SteadyStateHypothesisScheduleProfile ;
        cims:stereotype         "NC" ;
        cims:stereotype         <http://iec.ch/TC57/NonStandard/UML#concrete> .

nc:InServiceTimePoint.InServiceSchedule
        rdf:type              rdf:Property ;
        rdfs:comment          "The in service schedule that has this time point." ;
        rdfs:domain           nc:InServiceTimePoint ;
        rdfs:label            "InServiceSchedule"@en ;
        rdfs:range            nc:InServiceSchedule ;
        cims:AssociationUsed  "Yes" ;
        cims:inverseRoleName  nc:InServiceSchedule.InServiceTimePoint ;
        cims:multiplicity     cims:M:1 ;
        cims:stereotype       "NC" .

nc:InServiceTimePoint.atTime
        rdf:type           rdf:Property ;
        rdfs:comment       "The time the data is valid for." ;
        rdfs:domain        nc:InServiceTimePoint ;
        rdfs:label         "atTime"@en ;
        cims:dataType      cim:DateTime ;
        cims:multiplicity  cims:M:1..1 ;
        cims:stereotype    "NC" ;
        cims:stereotype    <http://iec.ch/TC57/NonStandard/UML#attribute> .

nc:InServiceTimePoint.inService
        rdf:type           rdf:Property ;
        rdfs:comment       "Specifies the availability of the equipment. True means the equipment is available for topology processing, which determines if the equipment is energized or not. False means that the equipment is treated by network applications as if it is not in the model." ;
        rdfs:domain        nc:InServiceTimePoint ;
        rdfs:label         "inService"@en ;
        cims:dataType      cim:Boolean ;
        cims:multiplicity  cims:M:1..1 ;
        cims:stereotype    "NC" ;
        cims:stereotype    <http://iec.ch/TC57/NonStandard/UML#attribute> .

nc:PeakKind  rdf:type           rdfs:Class ;
        rdfs:label              "PeakKind"@en ;
        cims:belongsToCategory  shs:Package_SteadyStateHypothesisScheduleProfile ;
        cims:stereotype         "NC" ;
        cims:stereotype         <http://iec.ch/TC57/NonStandard/UML#enumeration> .

nc:PeakKind.offPeak  rdf:type  nc:PeakKind ;
        rdfs:comment     "Off-peak refer to periods of lower demand for a particular service or commodity." ;
        rdfs:label       "offPeak"@en ;
        cims:stereotype  "enum" .

nc:PeakKind.onPeak  rdf:type  nc:PeakKind ;
        rdfs:comment     "Off-peak refer to periods of higher demand for a particular service or commodity." ;
        rdfs:label       "onPeak"@en ;
        cims:stereotype  "enum" .

nc:RegulatingControl.RegulatingControlRegularSchedule
        rdf:type              rdf:Property ;
        rdfs:comment          "RegulatingControlRegularSchedule which belongs to a regulating control." ;
        rdfs:domain           cim:RegulatingControl ;
        rdfs:label            "RegulatingControlRegularSchedule"@en ;
        rdfs:range            nc:RegulatingControlRegularSchedule ;
        cims:AssociationUsed  "No" ;
        cims:inverseRoleName  nc:RegulatingControlRegularSchedule.RegulatingControl ;
        cims:multiplicity     cims:M:0..n ;
        cims:stereotype       "NC" .

nc:RegulatingControl.RegulatingControlSchedule
        rdf:type              rdf:Property ;
        rdfs:comment          "Regulating control schedule associated with a regulating control." ;
        rdfs:domain           cim:RegulatingControl ;
        rdfs:label            "RegulatingControlSchedule"@en ;
        rdfs:range            nc:RegulatingControlSchedule ;
        cims:AssociationUsed  "No" ;
        cims:inverseRoleName  nc:RegulatingControlSchedule.RegulatingControl ;
        cims:multiplicity     cims:M:0..n ;
        cims:stereotype       "NC" .

nc:RegulatingControlRegularSchedule
        rdf:type                rdfs:Class ;
        rdfs:comment            "Regular schedule for regulating control." ;
        rdfs:label              "RegulatingControlRegularSchedule"@en ;
        rdfs:subClassOf         nc:BaseRegularIntervalSchedule ;
        cims:belongsToCategory  shs:Package_SteadyStateHypothesisScheduleProfile ;
        cims:stereotype         "NC" ;
        cims:stereotype         <http://iec.ch/TC57/NonStandard/UML#concrete> .

nc:RegulatingControlRegularSchedule.RegulatingControl
        rdf:type              rdf:Property ;
        rdfs:comment          "Regulating control which has RegulatingControlRegularSchedule." ;
        rdfs:domain           nc:RegulatingControlRegularSchedule ;
        rdfs:label            "RegulatingControl"@en ;
        rdfs:range            cim:RegulatingControl ;
        cims:AssociationUsed  "Yes" ;
        cims:inverseRoleName  nc:RegulatingControl.RegulatingControlRegularSchedule ;
        cims:multiplicity     cims:M:0..1 ;
        cims:stereotype       "NC" .

nc:RegulatingControlRegularSchedule.maxAllowedTargetValue
        rdf:type           rdf:Property ;
        rdfs:comment       "Maximum allowed target value (RegulatingControl.targetValue)." ;
        rdfs:domain        nc:RegulatingControlRegularSchedule ;
        rdfs:label         "maxAllowedTargetValue"@en ;
        cims:dataType      cim:Float ;
        cims:multiplicity  cims:M:0..1 ;
        cims:stereotype    "NC" ;
        cims:stereotype    <http://iec.ch/TC57/NonStandard/UML#attribute> .

nc:RegulatingControlRegularSchedule.minAllowedTargetValue
        rdf:type           rdf:Property ;
        rdfs:comment       "Minimum allowed target value (RegulatingControl.targetValue)." ;
        rdfs:domain        nc:RegulatingControlRegularSchedule ;
        rdfs:label         "minAllowedTargetValue"@en ;
        cims:dataType      cim:Float ;
        cims:multiplicity  cims:M:0..1 ;
        cims:stereotype    "NC" ;
        cims:stereotype    <http://iec.ch/TC57/NonStandard/UML#attribute> .

nc:RegulatingControlRegularSchedule.targetValue
        rdf:type           rdf:Property ;
        rdfs:comment       "The target value specified for case input.   This value can be used for the target value without the use of schedules. The value has the units appropriate to the mode attribute." ;
        rdfs:domain        nc:RegulatingControlRegularSchedule ;
        rdfs:label         "targetValue"@en ;
        cims:dataType      cim:Float ;
        cims:multiplicity  cims:M:1..1 ;
        cims:stereotype    "NC" ;
        cims:stereotype    <http://iec.ch/TC57/NonStandard/UML#attribute> .

nc:RegulatingControlRegularSchedule.targetValueUnitMultiplier
        rdf:type           rdf:Property ;
        rdfs:comment       "Specify the multiplier for used for the targetValue." ;
        rdfs:domain        nc:RegulatingControlRegularSchedule ;
        rdfs:label         "targetValueUnitMultiplier"@en ;
        rdfs:range         cim:UnitMultiplier ;
        cims:multiplicity  cims:M:1..1 ;
        cims:stereotype    "NC" ;
        cims:stereotype    <http://iec.ch/TC57/NonStandard/UML#attribute> .

nc:RegulatingControlSchedule
        rdf:type                rdfs:Class ;
        rdfs:comment            "Schedule for regulating control." ;
        rdfs:label              "RegulatingControlSchedule"@en ;
        rdfs:subClassOf         nc:BaseIrregularTimeSeries ;
        cims:belongsToCategory  shs:Package_SteadyStateHypothesisScheduleProfile ;
        cims:stereotype         "NC" ;
        cims:stereotype         <http://iec.ch/TC57/NonStandard/UML#concrete> .

nc:RegulatingControlSchedule.RegulatingControl
        rdf:type              rdf:Property ;
        rdfs:comment          "Regulating control which has regulating control schedules." ;
        rdfs:domain           nc:RegulatingControlSchedule ;
        rdfs:label            "RegulatingControl"@en ;
        rdfs:range            cim:RegulatingControl ;
        cims:AssociationUsed  "Yes" ;
        cims:inverseRoleName  nc:RegulatingControl.RegulatingControlSchedule ;
        cims:multiplicity     cims:M:0..1 ;
        cims:stereotype       "NC" .

nc:RegulatingControlSchedule.RegulatingControlTimePoint
        rdf:type              rdf:Property ;
        rdfs:comment          "The time point that relates to this regulating control schedule." ;
        rdfs:domain           nc:RegulatingControlSchedule ;
        rdfs:label            "RegulatingControlTimePoint"@en ;
        rdfs:range            nc:RegulatingControlTimePoint ;
        cims:AssociationUsed  "No" ;
        cims:inverseRoleName  nc:RegulatingControlTimePoint.RegulatingControlSchedule ;
        cims:multiplicity     cims:M:1..n ;
        cims:stereotype       "NC" ;
        cims:stereotype       <http://iec.ch/TC57/NonStandard/UML#ofAggregate> .

nc:RegulatingControlTimePoint
        rdf:type                rdfs:Class ;
        rdfs:comment            "Regulating control values for a given point in time." ;
        rdfs:label              "RegulatingControlTimePoint"@en ;
        cims:belongsToCategory  shs:Package_SteadyStateHypothesisScheduleProfile ;
        cims:stereotype         "NC" ;
        cims:stereotype         <http://iec.ch/TC57/NonStandard/UML#concrete> .

nc:RegulatingControlTimePoint.RegulatingControlSchedule
        rdf:type              rdf:Property ;
        rdfs:comment          "The regulating control schedule that has this time point." ;
        rdfs:domain           nc:RegulatingControlTimePoint ;
        rdfs:label            "RegulatingControlSchedule"@en ;
        rdfs:range            nc:RegulatingControlSchedule ;
        cims:AssociationUsed  "Yes" ;
        cims:inverseRoleName  nc:RegulatingControlSchedule.RegulatingControlTimePoint ;
        cims:multiplicity     cims:M:1 ;
        cims:stereotype       "NC" .

nc:RegulatingControlTimePoint.TapChangerControlSchedule
        rdf:type              rdf:Property ;
        rdfs:comment          "The tap changer control schedule that has this time point." ;
        rdfs:domain           nc:RegulatingControlTimePoint ;
        rdfs:label            "TapChangerControlSchedule"@en ;
        rdfs:range            nc:TapChangerControlSchedule ;
        cims:AssociationUsed  "Yes" ;
        cims:inverseRoleName  nc:TapChangerControlSchedule.RegulatingControlTimePoint ;
        cims:multiplicity     cims:M:1 ;
        cims:stereotype       "NC" .

nc:RegulatingControlTimePoint.atTime
        rdf:type           rdf:Property ;
        rdfs:comment       "The time the data is valid for." ;
        rdfs:domain        nc:RegulatingControlTimePoint ;
        rdfs:label         "atTime"@en ;
        cims:dataType      cim:DateTime ;
        cims:multiplicity  cims:M:1..1 ;
        cims:stereotype    "NC" ;
        cims:stereotype    <http://iec.ch/TC57/NonStandard/UML#attribute> .

nc:RegulatingControlTimePoint.maxAllowedTargetValue
        rdf:type           rdf:Property ;
        rdfs:comment       "Maximum allowed target value (RegulatingControl.targetValue)." ;
        rdfs:domain        nc:RegulatingControlTimePoint ;
        rdfs:label         "maxAllowedTargetValue"@en ;
        cims:dataType      cim:Float ;
        cims:multiplicity  cims:M:0..1 ;
        cims:stereotype    "NC" ;
        cims:stereotype    <http://iec.ch/TC57/NonStandard/UML#attribute> .

nc:RegulatingControlTimePoint.minAllowedTargetValue
        rdf:type           rdf:Property ;
        rdfs:comment       "Minimum allowed target value (RegulatingControl.targetValue)." ;
        rdfs:domain        nc:RegulatingControlTimePoint ;
        rdfs:label         "minAllowedTargetValue"@en ;
        cims:dataType      cim:Float ;
        cims:multiplicity  cims:M:0..1 ;
        cims:stereotype    "NC" ;
        cims:stereotype    <http://iec.ch/TC57/NonStandard/UML#attribute> .

nc:RegulatingControlTimePoint.targetValue
        rdf:type           rdf:Property ;
        rdfs:comment       "The target value specified for case input.   This value can be used for the target value without the use of schedules. The value has the units appropriate to the mode attribute." ;
        rdfs:domain        nc:RegulatingControlTimePoint ;
        rdfs:label         "targetValue"@en ;
        cims:dataType      cim:Float ;
        cims:multiplicity  cims:M:1..1 ;
        cims:stereotype    "NC" ;
        cims:stereotype    <http://iec.ch/TC57/NonStandard/UML#attribute> .

nc:RegulatingControlTimePoint.targetValueUnitMultiplier
        rdf:type           rdf:Property ;
        rdfs:comment       "Specify the multiplier for used for the targetValue." ;
        rdfs:domain        nc:RegulatingControlTimePoint ;
        rdfs:label         "targetValueUnitMultiplier"@en ;
        rdfs:range         cim:UnitMultiplier ;
        cims:multiplicity  cims:M:1..1 ;
        cims:stereotype    "NC" ;
        cims:stereotype    <http://iec.ch/TC57/NonStandard/UML#attribute> .

nc:Season.BaseRegularIntervalSchedule
        rdf:type              rdf:Property ;
        rdfs:comment          "Base regular interval schedule which has seasons." ;
        rdfs:domain           cim:Season ;
        rdfs:label            "BaseRegularIntervalSchedule"@en ;
        rdfs:range            nc:BaseRegularIntervalSchedule ;
        cims:AssociationUsed  "No" ;
        cims:inverseRoleName  nc:BaseRegularIntervalSchedule.Season ;
        cims:multiplicity     cims:M:0..n ;
        cims:stereotype       "NC" .

nc:ShuntCompensator.ShuntCompensatorSchedule
        rdf:type              rdf:Property ;
        rdfs:comment          "Shunt compensator schedule associated with a shunt compensator." ;
        rdfs:domain           cim:ShuntCompensator ;
        rdfs:label            "ShuntCompensatorSchedule"@en ;
        rdfs:range            nc:ShuntCompensatorSchedule ;
        cims:AssociationUsed  "No" ;
        cims:inverseRoleName  nc:ShuntCompensatorSchedule.ShuntCompensator ;
        cims:multiplicity     cims:M:0..n ;
        cims:stereotype       "NC" .

nc:ShuntCompensatorSchedule
        rdf:type                rdfs:Class ;
        rdfs:comment            "Schedule for shunt compensator." ;
        rdfs:label              "ShuntCompensatorSchedule"@en ;
        rdfs:subClassOf         nc:BaseIrregularTimeSeries ;
        cims:belongsToCategory  shs:Package_SteadyStateHypothesisScheduleProfile ;
        cims:stereotype         "NC" ;
        cims:stereotype         <http://iec.ch/TC57/NonStandard/UML#concrete> .

nc:ShuntCompensatorSchedule.ShuntCompensator
        rdf:type              rdf:Property ;
        rdfs:comment          "Shunt compensator which has shunt compensator schedules." ;
        rdfs:domain           nc:ShuntCompensatorSchedule ;
        rdfs:label            "ShuntCompensator"@en ;
        rdfs:range            cim:ShuntCompensator ;
        cims:AssociationUsed  "Yes" ;
        cims:inverseRoleName  nc:ShuntCompensator.ShuntCompensatorSchedule ;
        cims:multiplicity     cims:M:0..1 ;
        cims:stereotype       "NC" .

nc:ShuntCompensatorSchedule.ShuntCompensatorTimePoint
        rdf:type              rdf:Property ;
        rdfs:comment          "The time point that relates to this shunt compensator schedule." ;
        rdfs:domain           nc:ShuntCompensatorSchedule ;
        rdfs:label            "ShuntCompensatorTimePoint"@en ;
        rdfs:range            nc:ShuntCompensatorTimePoint ;
        cims:AssociationUsed  "No" ;
        cims:inverseRoleName  nc:ShuntCompensatorTimePoint.ShuntCompensatorSchedule ;
        cims:multiplicity     cims:M:1..n ;
        cims:stereotype       "NC" ;
        cims:stereotype       <http://iec.ch/TC57/NonStandard/UML#ofAggregate> .

nc:ShuntCompensatorTimePoint
        rdf:type                rdfs:Class ;
        rdfs:comment            "Shunt compensator values for a given point in time." ;
        rdfs:label              "ShuntCompensatorTimePoint"@en ;
        cims:belongsToCategory  shs:Package_SteadyStateHypothesisScheduleProfile ;
        cims:stereotype         "NC" ;
        cims:stereotype         <http://iec.ch/TC57/NonStandard/UML#concrete> .

nc:ShuntCompensatorTimePoint.ShuntCompensatorSchedule
        rdf:type              rdf:Property ;
        rdfs:comment          "The shunt compensator schedule that has this time point." ;
        rdfs:domain           nc:ShuntCompensatorTimePoint ;
        rdfs:label            "ShuntCompensatorSchedule"@en ;
        rdfs:range            nc:ShuntCompensatorSchedule ;
        cims:AssociationUsed  "Yes" ;
        cims:inverseRoleName  nc:ShuntCompensatorSchedule.ShuntCompensatorTimePoint ;
        cims:multiplicity     cims:M:1 ;
        cims:stereotype       "NC" .

nc:ShuntCompensatorTimePoint.atTime
        rdf:type           rdf:Property ;
        rdfs:comment       "The time the data is valid for." ;
        rdfs:domain        nc:ShuntCompensatorTimePoint ;
        rdfs:label         "atTime"@en ;
        cims:dataType      cim:DateTime ;
        cims:multiplicity  cims:M:1..1 ;
        cims:stereotype    "NC" ;
        cims:stereotype    <http://iec.ch/TC57/NonStandard/UML#attribute> .

nc:ShuntCompensatorTimePoint.sections
        rdf:type           rdf:Property ;
        rdfs:comment       "Shunt compensator sections in use. Starting value for steady state solution. The attribute shall be a positive value or zero. Non integer values are allowed to support continuous variables. The reasons for continuous value are to support study cases where no discrete shunt compensators has yet been designed, a solutions where a narrow voltage band force the sections to oscillate or accommodate for a continuous solution as input. \nFor LinearShuntConpensator the value shall be between zero and ShuntCompensator.maximumSections. At value zero the shunt compensator conductance and admittance is zero. Linear interpolation of conductance and admittance between the previous and next integer section is applied in case of non-integer values.\nFor NonlinearShuntCompensator-s shall only be set to one of the NonlinearShuntCompenstorPoint.sectionNumber. There is no interpolation between NonlinearShuntCompenstorPoint-s." ;
        rdfs:domain        nc:ShuntCompensatorTimePoint ;
        rdfs:label         "sections"@en ;
        cims:dataType      cim:Float ;
        cims:multiplicity  cims:M:1..1 ;
        cims:stereotype    "NC" ;
        cims:stereotype    <http://iec.ch/TC57/NonStandard/UML#attribute> .

nc:StaticVarCompensator.StaticVarCompensatorSchedule
        rdf:type              rdf:Property ;
        rdfs:comment          "Static var compensator schedule associated with a static var compensator." ;
        rdfs:domain           cim:StaticVarCompensator ;
        rdfs:label            "StaticVarCompensatorSchedule"@en ;
        rdfs:range            nc:StaticVarCompensatorSchedule ;
        cims:AssociationUsed  "No" ;
        cims:inverseRoleName  nc:StaticVarCompensatorSchedule.StaticVarCompensator ;
        cims:multiplicity     cims:M:0..n ;
        cims:stereotype       "NC" .

nc:StaticVarCompensatorSchedule
        rdf:type                rdfs:Class ;
        rdfs:comment            "Schedule for static var compensator." ;
        rdfs:label              "StaticVarCompensatorSchedule"@en ;
        rdfs:subClassOf         nc:BaseIrregularTimeSeries ;
        cims:belongsToCategory  shs:Package_SteadyStateHypothesisScheduleProfile ;
        cims:stereotype         "NC" ;
        cims:stereotype         <http://iec.ch/TC57/NonStandard/UML#concrete> .

nc:StaticVarCompensatorSchedule.StaticVarCompensator
        rdf:type              rdf:Property ;
        rdfs:comment          "Static var compensator which has static var compensator schedules." ;
        rdfs:domain           nc:StaticVarCompensatorSchedule ;
        rdfs:label            "StaticVarCompensator"@en ;
        rdfs:range            cim:StaticVarCompensator ;
        cims:AssociationUsed  "Yes" ;
        cims:inverseRoleName  nc:StaticVarCompensator.StaticVarCompensatorSchedule ;
        cims:multiplicity     cims:M:0..1 ;
        cims:stereotype       "NC" .

nc:StaticVarCompensatorSchedule.StaticVarCompensatorTimePoint
        rdf:type              rdf:Property ;
        rdfs:comment          "The time point that relates to this static var compensator schedule." ;
        rdfs:domain           nc:StaticVarCompensatorSchedule ;
        rdfs:label            "StaticVarCompensatorTimePoint"@en ;
        rdfs:range            nc:StaticVarCompensatorTimePoint ;
        cims:AssociationUsed  "No" ;
        cims:inverseRoleName  nc:StaticVarCompensatorTimePoint.StaticVarCompensatorSchedule ;
        cims:multiplicity     cims:M:1..n ;
        cims:stereotype       "NC" ;
        cims:stereotype       <http://iec.ch/TC57/NonStandard/UML#ofAggregate> .

nc:StaticVarCompensatorTimePoint
        rdf:type                rdfs:Class ;
        rdfs:comment            "Static var compensator values for a given point in time." ;
        rdfs:label              "StaticVarCompensatorTimePoint"@en ;
        cims:belongsToCategory  shs:Package_SteadyStateHypothesisScheduleProfile ;
        cims:stereotype         "NC" ;
        cims:stereotype         <http://iec.ch/TC57/NonStandard/UML#concrete> .

nc:StaticVarCompensatorTimePoint.StaticVarCompensatorSchedule
        rdf:type              rdf:Property ;
        rdfs:comment          "The StaticVarCompensator schedule that has this time point." ;
        rdfs:domain           nc:StaticVarCompensatorTimePoint ;
        rdfs:label            "StaticVarCompensatorSchedule"@en ;
        rdfs:range            nc:StaticVarCompensatorSchedule ;
        cims:AssociationUsed  "Yes" ;
        cims:inverseRoleName  nc:StaticVarCompensatorSchedule.StaticVarCompensatorTimePoint ;
        cims:multiplicity     cims:M:1 ;
        cims:stereotype       "NC" .

nc:StaticVarCompensatorTimePoint.atTime
        rdf:type           rdf:Property ;
        rdfs:comment       "The time the data is valid for." ;
        rdfs:domain        nc:StaticVarCompensatorTimePoint ;
        rdfs:label         "atTime"@en ;
        cims:dataType      cim:DateTime ;
        cims:multiplicity  cims:M:0..1 ;
        cims:stereotype    "NC" ;
        cims:stereotype    <http://iec.ch/TC57/NonStandard/UML#attribute> .

nc:StaticVarCompensatorTimePoint.q
        rdf:type           rdf:Property ;
        rdfs:comment       "Reactive power injection. Load sign convention is used, i.e. positive sign means flow out from a node.\nStarting value for a steady state solution." ;
        rdfs:domain        nc:StaticVarCompensatorTimePoint ;
        rdfs:label         "q"@en ;
        cims:dataType      cim:ReactivePower ;
        cims:multiplicity  cims:M:1..1 ;
        cims:stereotype    "NC" ;
        cims:stereotype    <http://iec.ch/TC57/NonStandard/UML#attribute> .

nc:Switch.SwitchRegularSchedule
        rdf:type              rdf:Property ;
        rdfs:comment          "SwitchRegularSchedule which belongs to a switch." ;
        rdfs:domain           cim:Switch ;
        rdfs:label            "SwitchRegularSchedule"@en ;
        rdfs:range            nc:SwitchRegularSchedule ;
        cims:AssociationUsed  "No" ;
        cims:inverseRoleName  nc:SwitchRegularSchedule.Switch ;
        cims:multiplicity     cims:M:0..n ;
        cims:stereotype       "NC" .

nc:Switch.SwitchSchedule
        rdf:type              rdf:Property ;
        rdfs:comment          "Switch schedule associated with a switch." ;
        rdfs:domain           cim:Switch ;
        rdfs:label            "SwitchSchedule"@en ;
        rdfs:range            nc:SwitchSchedule ;
        cims:AssociationUsed  "No" ;
        cims:inverseRoleName  nc:SwitchSchedule.Switch ;
        cims:multiplicity     cims:M:0..n ;
        cims:stereotype       "NC" .

nc:SwitchRegularSchedule
        rdf:type                rdfs:Class ;
        rdfs:comment            "Regular schedule for switch." ;
        rdfs:label              "SwitchRegularSchedule"@en ;
        rdfs:subClassOf         nc:BaseRegularIntervalSchedule ;
        cims:belongsToCategory  shs:Package_SteadyStateHypothesisScheduleProfile ;
        cims:stereotype         "NC" ;
        cims:stereotype         <http://iec.ch/TC57/NonStandard/UML#concrete> .

nc:SwitchRegularSchedule.Switch
        rdf:type              rdf:Property ;
        rdfs:comment          "Switch which has SwitchRegularSchedule." ;
        rdfs:domain           nc:SwitchRegularSchedule ;
        rdfs:label            "Switch"@en ;
        rdfs:range            cim:Switch ;
        cims:AssociationUsed  "Yes" ;
        cims:inverseRoleName  nc:Switch.SwitchRegularSchedule ;
        cims:multiplicity     cims:M:0..1 ;
        cims:stereotype       "NC" .

nc:SwitchRegularSchedule.locked
        rdf:type           rdf:Property ;
        rdfs:comment       "If true, the switch is locked. The resulting switch state is a combination of locked and Switch.open attributes as follows:\n<ul>\n\t<li>locked=true and Switch.open=true. The resulting state is open and locked;</li>\n\t<li>locked=false and Switch.open=true. The resulting state is open;</li>\n\t<li>locked=false and Switch.open=false. The resulting state is closed.</li>\n</ul>" ;
        rdfs:domain        nc:SwitchRegularSchedule ;
        rdfs:label         "locked"@en ;
        cims:dataType      cim:Boolean ;
        cims:multiplicity  cims:M:1..1 ;
        cims:stereotype    "NC" ;
        cims:stereotype    <http://iec.ch/TC57/NonStandard/UML#attribute> .

nc:SwitchRegularSchedule.open
        rdf:type           rdf:Property ;
        rdfs:comment       "The attribute tells if the switch is considered open when used as input to topology processing." ;
        rdfs:domain        nc:SwitchRegularSchedule ;
        rdfs:label         "open"@en ;
        cims:dataType      cim:Boolean ;
        cims:multiplicity  cims:M:1..1 ;
        cims:stereotype    "NC" ;
        cims:stereotype    <http://iec.ch/TC57/NonStandard/UML#attribute> .

nc:SwitchSchedule  rdf:type     rdfs:Class ;
        rdfs:comment            "Schedule for switch." ;
        rdfs:label              "SwitchSchedule"@en ;
        rdfs:subClassOf         nc:BaseIrregularTimeSeries ;
        cims:belongsToCategory  shs:Package_SteadyStateHypothesisScheduleProfile ;
        cims:stereotype         "NC" ;
        cims:stereotype         <http://iec.ch/TC57/NonStandard/UML#concrete> .

nc:SwitchSchedule.Switch
        rdf:type              rdf:Property ;
        rdfs:comment          "Switch which has switch schedules." ;
        rdfs:domain           nc:SwitchSchedule ;
        rdfs:label            "Switch"@en ;
        rdfs:range            cim:Switch ;
        cims:AssociationUsed  "Yes" ;
        cims:inverseRoleName  nc:Switch.SwitchSchedule ;
        cims:multiplicity     cims:M:0..1 ;
        cims:stereotype       "NC" .

nc:SwitchSchedule.SwitchTimePoint
        rdf:type              rdf:Property ;
        rdfs:comment          "The time point that relates to this switch schedule." ;
        rdfs:domain           nc:SwitchSchedule ;
        rdfs:label            "SwitchTimePoint"@en ;
        rdfs:range            nc:SwitchTimePoint ;
        cims:AssociationUsed  "No" ;
        cims:inverseRoleName  nc:SwitchTimePoint.SwitchSchedule ;
        cims:multiplicity     cims:M:1..n ;
        cims:stereotype       <http://iec.ch/TC57/NonStandard/UML#ofAggregate> .

nc:SwitchTimePoint  rdf:type    rdfs:Class ;
        rdfs:comment            "Switch values for a given point in time." ;
        rdfs:label              "SwitchTimePoint"@en ;
        cims:belongsToCategory  shs:Package_SteadyStateHypothesisScheduleProfile ;
        cims:stereotype         "NC" ;
        cims:stereotype         <http://iec.ch/TC57/NonStandard/UML#concrete> .

nc:SwitchTimePoint.SwitchSchedule
        rdf:type              rdf:Property ;
        rdfs:comment          "The switch schedule that has this time point." ;
        rdfs:domain           nc:SwitchTimePoint ;
        rdfs:label            "SwitchSchedule"@en ;
        rdfs:range            nc:SwitchSchedule ;
        cims:AssociationUsed  "Yes" ;
        cims:inverseRoleName  nc:SwitchSchedule.SwitchTimePoint ;
        cims:multiplicity     cims:M:1 .

nc:SwitchTimePoint.atTime
        rdf:type           rdf:Property ;
        rdfs:comment       "The time the data is valid for." ;
        rdfs:domain        nc:SwitchTimePoint ;
        rdfs:label         "atTime"@en ;
        cims:dataType      cim:DateTime ;
        cims:multiplicity  cims:M:1..1 ;
        cims:stereotype    "NC" ;
        cims:stereotype    <http://iec.ch/TC57/NonStandard/UML#attribute> .

nc:SwitchTimePoint.locked
        rdf:type           rdf:Property ;
        rdfs:comment       "If true, the switch is locked. The resulting switch state is a combination of locked and Switch.open attributes as follows:\n<ul>\n\t<li>locked=true and Switch.open=true. The resulting state is open and locked;</li>\n\t<li>locked=false and Switch.open=true. The resulting state is open;</li>\n\t<li>locked=false and Switch.open=false. The resulting state is closed.</li>\n</ul>" ;
        rdfs:domain        nc:SwitchTimePoint ;
        rdfs:label         "locked"@en ;
        cims:dataType      cim:Boolean ;
        cims:multiplicity  cims:M:1..1 ;
        cims:stereotype    "NC" ;
        cims:stereotype    <http://iec.ch/TC57/NonStandard/UML#attribute> .

nc:SwitchTimePoint.open
        rdf:type           rdf:Property ;
        rdfs:comment       "The attribute tells if the switch is considered open when used as input to topology processing." ;
        rdfs:domain        nc:SwitchTimePoint ;
        rdfs:label         "open"@en ;
        cims:dataType      cim:Boolean ;
        cims:multiplicity  cims:M:1..1 ;
        cims:stereotype    "NC" ;
        cims:stereotype    <http://iec.ch/TC57/NonStandard/UML#attribute> .

nc:SynchronousMachine.SynchronousMachineRegularSchedule
        rdf:type              rdf:Property ;
        rdfs:comment          "SynchronousMachineRegularSchedule which belongs to a synchronous machine." ;
        rdfs:domain           cim:SynchronousMachine ;
        rdfs:label            "SynchronousMachineRegularSchedule"@en ;
        rdfs:range            nc:SynchronousMachineRegularSchedule ;
        cims:AssociationUsed  "No" ;
        cims:inverseRoleName  nc:SynchronousMachineRegularSchedule.SynchronousMachine ;
        cims:multiplicity     cims:M:0..n ;
        cims:stereotype       "NC" .

nc:SynchronousMachine.SynchronousMachineSchedule
        rdf:type              rdf:Property ;
        rdfs:comment          "Synchronous machine schedule associated with a synchronous machine." ;
        rdfs:domain           cim:SynchronousMachine ;
        rdfs:label            "SynchronousMachineSchedule"@en ;
        rdfs:range            nc:SynchronousMachineSchedule ;
        cims:AssociationUsed  "No" ;
        cims:inverseRoleName  nc:SynchronousMachineSchedule.SynchronousMachine ;
        cims:multiplicity     cims:M:0..n ;
        cims:stereotype       "NC" .

nc:SynchronousMachineRegularSchedule
        rdf:type                rdfs:Class ;
        rdfs:comment            "Regular schedule for synchronous machine." ;
        rdfs:label              "SynchronousMachineRegularSchedule"@en ;
        rdfs:subClassOf         nc:BaseRegularIntervalSchedule ;
        cims:belongsToCategory  shs:Package_SteadyStateHypothesisScheduleProfile ;
        cims:stereotype         "NC" ;
        cims:stereotype         <http://iec.ch/TC57/NonStandard/UML#concrete> .

nc:SynchronousMachineRegularSchedule.SynchronousMachine
        rdf:type              rdf:Property ;
        rdfs:comment          "SynchronousMachine which has SynchronousMachineRegularSchedule." ;
        rdfs:domain           nc:SynchronousMachineRegularSchedule ;
        rdfs:label            "SynchronousMachine"@en ;
        rdfs:range            cim:SynchronousMachine ;
        cims:AssociationUsed  "Yes" ;
        cims:inverseRoleName  nc:SynchronousMachine.SynchronousMachineRegularSchedule ;
        cims:multiplicity     cims:M:0..1 ;
        cims:stereotype       "NC" .

nc:SynchronousMachineRegularSchedule.operatingMode
        rdf:type           rdf:Property ;
        rdfs:comment       "Current mode of operation." ;
        rdfs:domain        nc:SynchronousMachineRegularSchedule ;
        rdfs:label         "operatingMode"@en ;
        rdfs:range         cim:SynchronousMachineOperatingMode ;
        cims:multiplicity  cims:M:1..1 ;
        cims:stereotype    "NC" ;
        cims:stereotype    <http://iec.ch/TC57/NonStandard/UML#attribute> .

nc:SynchronousMachineRegularSchedule.referencePriority
        rdf:type           rdf:Property ;
        rdfs:comment       "Priority of unit for use as powerflow voltage phase angle reference bus selection. 0 = don t care (default) 1 = highest priority. 2 is less than 1 and so on." ;
        rdfs:domain        nc:SynchronousMachineRegularSchedule ;
        rdfs:label         "referencePriority"@en ;
        cims:dataType      cim:Integer ;
        cims:multiplicity  cims:M:1..1 ;
        cims:stereotype    "NC" ;
        cims:stereotype    <http://iec.ch/TC57/NonStandard/UML#attribute> .

nc:SynchronousMachineSchedule
        rdf:type                rdfs:Class ;
        rdfs:comment            "Schedule for synchronous machine." ;
        rdfs:label              "SynchronousMachineSchedule"@en ;
        rdfs:subClassOf         nc:BaseIrregularTimeSeries ;
        cims:belongsToCategory  shs:Package_SteadyStateHypothesisScheduleProfile ;
        cims:stereotype         "NC" ;
        cims:stereotype         <http://iec.ch/TC57/NonStandard/UML#concrete> .

nc:SynchronousMachineSchedule.SynchronousMachine
        rdf:type              rdf:Property ;
        rdfs:comment          "Synchronous machine which has synchronous machine schedules." ;
        rdfs:domain           nc:SynchronousMachineSchedule ;
        rdfs:label            "SynchronousMachine"@en ;
        rdfs:range            cim:SynchronousMachine ;
        cims:AssociationUsed  "Yes" ;
        cims:inverseRoleName  nc:SynchronousMachine.SynchronousMachineSchedule ;
        cims:multiplicity     cims:M:0..1 ;
        cims:stereotype       "NC" .

nc:SynchronousMachineSchedule.SynchronousMachineTimePoint
        rdf:type              rdf:Property ;
        rdfs:comment          "The time point that relates to this synchronous machine schedule." ;
        rdfs:domain           nc:SynchronousMachineSchedule ;
        rdfs:label            "SynchronousMachineTimePoint"@en ;
        rdfs:range            nc:SynchronousMachineTimePoint ;
        cims:AssociationUsed  "No" ;
        cims:inverseRoleName  nc:SynchronousMachineTimePoint.SynchronousMachineSchedule ;
        cims:multiplicity     cims:M:1..n ;
        cims:stereotype       "NC" ;
        cims:stereotype       <http://iec.ch/TC57/NonStandard/UML#ofAggregate> .

nc:SynchronousMachineTimePoint
        rdf:type                rdfs:Class ;
        rdfs:comment            "Synchronous machine values for a given point in time." ;
        rdfs:label              "SynchronousMachineTimePoint"@en ;
        cims:belongsToCategory  shs:Package_SteadyStateHypothesisScheduleProfile ;
        cims:stereotype         "NC" ;
        cims:stereotype         <http://iec.ch/TC57/NonStandard/UML#concrete> .

nc:SynchronousMachineTimePoint.SynchronousMachineSchedule
        rdf:type              rdf:Property ;
        rdfs:comment          "The synchronous machine schedule that has this time point." ;
        rdfs:domain           nc:SynchronousMachineTimePoint ;
        rdfs:label            "SynchronousMachineSchedule"@en ;
        rdfs:range            nc:SynchronousMachineSchedule ;
        cims:AssociationUsed  "Yes" ;
        cims:inverseRoleName  nc:SynchronousMachineSchedule.SynchronousMachineTimePoint ;
        cims:multiplicity     cims:M:1 ;
        cims:stereotype       "NC" .

nc:SynchronousMachineTimePoint.atTime
        rdf:type           rdf:Property ;
        rdfs:comment       "The time the data is valid for." ;
        rdfs:domain        nc:SynchronousMachineTimePoint ;
        rdfs:label         "atTime"@en ;
        cims:dataType      cim:DateTime ;
        cims:multiplicity  cims:M:1..1 ;
        cims:stereotype    "NC" ;
        cims:stereotype    <http://iec.ch/TC57/NonStandard/UML#attribute> .

nc:SynchronousMachineTimePoint.operatingMode
        rdf:type           rdf:Property ;
        rdfs:comment       "Current mode of operation." ;
        rdfs:domain        nc:SynchronousMachineTimePoint ;
        rdfs:label         "operatingMode"@en ;
        rdfs:range         cim:SynchronousMachineOperatingMode ;
        cims:multiplicity  cims:M:1..1 ;
        cims:stereotype    "NC" ;
        cims:stereotype    <http://iec.ch/TC57/NonStandard/UML#attribute> .

nc:SynchronousMachineTimePoint.referencePriority
        rdf:type           rdf:Property ;
        rdfs:comment       "Priority of unit for use as powerflow voltage phase angle reference bus selection. 0 = don t care (default) 1 = highest priority. 2 is less than 1 and so on." ;
        rdfs:domain        nc:SynchronousMachineTimePoint ;
        rdfs:label         "referencePriority"@en ;
        cims:dataType      cim:Integer ;
        cims:multiplicity  cims:M:1..1 ;
        cims:stereotype    "NC" ;
        cims:stereotype    <http://iec.ch/TC57/NonStandard/UML#attribute> .

nc:TapChanger.TapRegularSchedule
        rdf:type              rdf:Property ;
        rdfs:comment          "TapRegularSchedule which belongs to a tap change." ;
        rdfs:domain           cim:TapChanger ;
        rdfs:label            "TapRegularSchedule"@en ;
        rdfs:range            nc:TapRegularSchedule ;
        cims:AssociationUsed  "No" ;
        cims:inverseRoleName  nc:TapRegularSchedule.TapChanger ;
        cims:multiplicity     cims:M:0..n ;
        cims:stereotype       "NC" .

nc:TapChanger.TapSchedule
        rdf:type              rdf:Property ;
        rdfs:comment          "Tap schedule associated with a tap changer." ;
        rdfs:domain           cim:TapChanger ;
        rdfs:label            "TapSchedule"@en ;
        rdfs:range            nc:TapSchedule ;
        cims:AssociationUsed  "No" ;
        cims:inverseRoleName  nc:TapSchedule.TapChanger ;
        cims:multiplicity     cims:M:0..n ;
        cims:stereotype       "NC" .

nc:TapChangerControl.TapChangerControlRegularSchedule
        rdf:type              rdf:Property ;
        rdfs:comment          "TapChangerControlRegularSchedule which belongs to a tap changer control." ;
        rdfs:domain           cim:TapChangerControl ;
        rdfs:label            "TapChangerControlRegularSchedule"@en ;
        rdfs:range            nc:TapChangerControlRegularSchedule ;
        cims:AssociationUsed  "No" ;
        cims:inverseRoleName  nc:TapChangerControlRegularSchedule.TapChangerControl ;
        cims:multiplicity     cims:M:0..n ;
        cims:stereotype       "NC" .

nc:TapChangerControl.TapChangerControlSchedule
        rdf:type              rdf:Property ;
        rdfs:domain           cim:TapChangerControl ;
        rdfs:label            "TapChangerControlSchedule"@en ;
        rdfs:range            nc:TapChangerControlSchedule ;
        cims:AssociationUsed  "No" ;
        cims:inverseRoleName  nc:TapChangerControlSchedule.TapChangerControl ;
        cims:multiplicity     cims:M:0..n ;
        cims:stereotype       "NC" .

nc:TapChangerControlRegularSchedule
        rdf:type                rdfs:Class ;
        rdfs:comment            "Regular schedule for tap changer control." ;
        rdfs:label              "TapChangerControlRegularSchedule"@en ;
        rdfs:subClassOf         nc:RegulatingControlRegularSchedule ;
        cims:belongsToCategory  shs:Package_SteadyStateHypothesisScheduleProfile ;
        cims:stereotype         "NC" ;
        cims:stereotype         <http://iec.ch/TC57/NonStandard/UML#concrete> .

nc:TapChangerControlRegularSchedule.TapChangerControl
        rdf:type              rdf:Property ;
        rdfs:comment          "Tap changer control which has TapChangerControlRegularSchedule." ;
        rdfs:domain           nc:TapChangerControlRegularSchedule ;
        rdfs:label            "TapChangerControl"@en ;
        rdfs:range            cim:TapChangerControl ;
        cims:AssociationUsed  "Yes" ;
        cims:inverseRoleName  nc:TapChangerControl.TapChangerControlRegularSchedule ;
        cims:multiplicity     cims:M:0..1 ;
        cims:stereotype       "NC" .

nc:TapChangerControlSchedule
        rdf:type                rdfs:Class ;
        rdfs:comment            "Schedule for tap changer control." ;
        rdfs:label              "TapChangerControlSchedule"@en ;
        rdfs:subClassOf         nc:BaseIrregularTimeSeries ;
        cims:belongsToCategory  shs:Package_SteadyStateHypothesisScheduleProfile ;
        cims:stereotype         "NC" ;
        cims:stereotype         <http://iec.ch/TC57/NonStandard/UML#concrete> .

nc:TapChangerControlSchedule.RegulatingControlTimePoint
        rdf:type              rdf:Property ;
        rdfs:comment          "The time point that relates to this stap changer control schedule." ;
        rdfs:domain           nc:TapChangerControlSchedule ;
        rdfs:label            "RegulatingControlTimePoint"@en ;
        rdfs:range            nc:RegulatingControlTimePoint ;
        cims:AssociationUsed  "No" ;
        cims:inverseRoleName  nc:RegulatingControlTimePoint.TapChangerControlSchedule ;
        cims:multiplicity     cims:M:1..n ;
        cims:stereotype       "NC" ;
        cims:stereotype       <http://iec.ch/TC57/NonStandard/UML#ofAggregate> .

nc:TapChangerControlSchedule.TapChangerControl
        rdf:type              rdf:Property ;
        rdfs:domain           nc:TapChangerControlSchedule ;
        rdfs:label            "TapChangerControl"@en ;
        rdfs:range            cim:TapChangerControl ;
        cims:AssociationUsed  "Yes" ;
        cims:inverseRoleName  nc:TapChangerControl.TapChangerControlSchedule ;
        cims:multiplicity     cims:M:0..1 ;
        cims:stereotype       "NC" .

nc:TapRegularSchedule
        rdf:type                rdfs:Class ;
        rdfs:comment            "Regular schedule for tap." ;
        rdfs:label              "TapRegularSchedule"@en ;
        rdfs:subClassOf         nc:BaseRegularIntervalSchedule ;
        cims:belongsToCategory  shs:Package_SteadyStateHypothesisScheduleProfile ;
        cims:stereotype         "NC" ;
        cims:stereotype         <http://iec.ch/TC57/NonStandard/UML#concrete> .

nc:TapRegularSchedule.TapChanger
        rdf:type              rdf:Property ;
        rdfs:comment          "Tap changer which has TapRegularSchedule." ;
        rdfs:domain           nc:TapRegularSchedule ;
        rdfs:label            "TapChanger"@en ;
        rdfs:range            cim:TapChanger ;
        cims:AssociationUsed  "Yes" ;
        cims:inverseRoleName  nc:TapChanger.TapRegularSchedule ;
        cims:multiplicity     cims:M:0..1 ;
        cims:stereotype       "NC" .

nc:TapRegularSchedule.controlEnabled
        rdf:type           rdf:Property ;
        rdfs:comment       "Specifies the regulation status of the equipment.  True is regulating, false is not regulating." ;
        rdfs:domain        nc:TapRegularSchedule ;
        rdfs:label         "controlEnabled"@en ;
        cims:dataType      cim:Boolean ;
        cims:multiplicity  cims:M:1..1 ;
        cims:stereotype    "NC" ;
        cims:stereotype    <http://iec.ch/TC57/NonStandard/UML#attribute> .

nc:TapRegularSchedule.step
        rdf:type           rdf:Property ;
        rdfs:comment       "Tap changer position.\nStarting step for a steady state solution. Non integer values are allowed to support continuous tap variables. The reasons for continuous value are to support study cases where no discrete tap changer has yet been designed, a solution where a narrow voltage band forces the tap step to oscillate or to accommodate for a continuous solution as input.\nThe attribute shall be equal to or greater than lowStep and equal to or less than highStep." ;
        rdfs:domain        nc:TapRegularSchedule ;
        rdfs:label         "step"@en ;
        cims:dataType      cim:Float ;
        cims:multiplicity  cims:M:1..1 ;
        cims:stereotype    "NC" ;
        cims:stereotype    <http://iec.ch/TC57/NonStandard/UML#attribute> .

nc:TapSchedule  rdf:type        rdfs:Class ;
        rdfs:comment            "Schedule for tap." ;
        rdfs:label              "TapSchedule"@en ;
        rdfs:subClassOf         nc:BaseIrregularTimeSeries ;
        cims:belongsToCategory  shs:Package_SteadyStateHypothesisScheduleProfile ;
        cims:stereotype         "NC" ;
        cims:stereotype         <http://iec.ch/TC57/NonStandard/UML#concrete> .

nc:TapSchedule.TapChanger
        rdf:type              rdf:Property ;
        rdfs:comment          "Tap changer which has tap schedules." ;
        rdfs:domain           nc:TapSchedule ;
        rdfs:label            "TapChanger"@en ;
        rdfs:range            cim:TapChanger ;
        cims:AssociationUsed  "Yes" ;
        cims:inverseRoleName  nc:TapChanger.TapSchedule ;
        cims:multiplicity     cims:M:0..1 ;
        cims:stereotype       "NC" .

nc:TapSchedule.TapScheduleTimePoint
        rdf:type              rdf:Property ;
        rdfs:comment          "The time point that relates to this tap schedule." ;
        rdfs:domain           nc:TapSchedule ;
        rdfs:label            "TapScheduleTimePoint"@en ;
        rdfs:range            nc:TapScheduleTimePoint ;
        cims:AssociationUsed  "No" ;
        cims:inverseRoleName  nc:TapScheduleTimePoint.TapSchedule ;
        cims:multiplicity     cims:M:1..n ;
        cims:stereotype       "NC" ;
        cims:stereotype       <http://iec.ch/TC57/NonStandard/UML#ofAggregate> .

nc:TapScheduleTimePoint
        rdf:type                rdfs:Class ;
        rdfs:comment            "Tap schedule values for a given point in time." ;
        rdfs:label              "TapScheduleTimePoint"@en ;
        cims:belongsToCategory  shs:Package_SteadyStateHypothesisScheduleProfile ;
        cims:stereotype         "NC" ;
        cims:stereotype         <http://iec.ch/TC57/NonStandard/UML#concrete> .

nc:TapScheduleTimePoint.TapSchedule
        rdf:type              rdf:Property ;
        rdfs:comment          "The tap schedule that has this time point." ;
        rdfs:domain           nc:TapScheduleTimePoint ;
        rdfs:label            "TapSchedule"@en ;
        rdfs:range            nc:TapSchedule ;
        cims:AssociationUsed  "Yes" ;
        cims:inverseRoleName  nc:TapSchedule.TapScheduleTimePoint ;
        cims:multiplicity     cims:M:1 ;
        cims:stereotype       "NC" .

nc:TapScheduleTimePoint.atTime
        rdf:type           rdf:Property ;
        rdfs:comment       "The time the data is valid for." ;
        rdfs:domain        nc:TapScheduleTimePoint ;
        rdfs:label         "atTime"@en ;
        cims:dataType      cim:DateTime ;
        cims:multiplicity  cims:M:1..1 ;
        cims:stereotype    "NC" ;
        cims:stereotype    <http://iec.ch/TC57/NonStandard/UML#attribute> .

nc:TapScheduleTimePoint.controlEnabled
        rdf:type           rdf:Property ;
        rdfs:comment       "Specifies the regulation status of the equipment.  True is regulating, false is not regulating." ;
        rdfs:domain        nc:TapScheduleTimePoint ;
        rdfs:label         "controlEnabled"@en ;
        cims:dataType      cim:Boolean ;
        cims:multiplicity  cims:M:1..1 ;
        cims:stereotype    "NC" ;
        cims:stereotype    <http://iec.ch/TC57/NonStandard/UML#attribute> .

nc:TapScheduleTimePoint.step
        rdf:type           rdf:Property ;
        rdfs:comment       "Tap changer position.\nStarting step for a steady state solution. Non integer values are allowed to support continuous tap variables. The reasons for continuous value are to support study cases where no discrete tap changer has yet been designed, a solution where a narrow voltage band forces the tap step to oscillate or to accommodate for a continuous solution as input.\nThe attribute shall be equal to or greater than lowStep and equal to or less than highStep." ;
        rdfs:domain        nc:TapScheduleTimePoint ;
        rdfs:label         "step"@en ;
        cims:dataType      cim:Float ;
        cims:multiplicity  cims:M:1..1 ;
        cims:stereotype    "NC" ;
        cims:stereotype    <http://iec.ch/TC57/NonStandard/UML#attribute> .

nc:TimeSeriesInterpolationKind
        rdf:type                rdfs:Class ;
        rdfs:comment            "Kinds of interpolation of values between two time point. " ;
        rdfs:label              "TimeSeriesInterpolationKind"@en ;
        cims:belongsToCategory  shs:Package_SteadyStateHypothesisScheduleProfile ;
        cims:stereotype         "NC" ;
        cims:stereotype         <http://iec.ch/TC57/NonStandard/UML#enumeration> .

nc:TimeSeriesInterpolationKind.linear
        rdf:type         nc:TimeSeriesInterpolationKind ;
        rdfs:comment     "Linear interpolation is applied for values between two time points." ;
        rdfs:label       "linear"@en ;
        cims:stereotype  "enum" .

nc:TimeSeriesInterpolationKind.next
        rdf:type         nc:TimeSeriesInterpolationKind ;
        rdfs:comment     "The value between two time points is set to next value." ;
        rdfs:label       "next"@en ;
        cims:stereotype  "enum" .

nc:TimeSeriesInterpolationKind.none
        rdf:type         nc:TimeSeriesInterpolationKind ;
        rdfs:comment     "No interpolation is applied." ;
        rdfs:label       "none"@en ;
        cims:stereotype  "enum" .

nc:TimeSeriesInterpolationKind.previous
        rdf:type         nc:TimeSeriesInterpolationKind ;
        rdfs:comment     "The value between two time points is set to previous value." ;
        rdfs:label       "previous"@en ;
        cims:stereotype  "enum" .

nc:TimeSeriesInterpolationKind.zero
        rdf:type         nc:TimeSeriesInterpolationKind ;
        rdfs:comment     "The value between two time points is set to zero." ;
        rdfs:label       "zero"@en ;
        cims:stereotype  "enum" .

nc:VoltageLimit.VoltageLimitSchedule
        rdf:type              rdf:Property ;
        rdfs:comment          "Voltage limit schedule associated with a voltage limit." ;
        rdfs:domain           cim:VoltageLimit ;
        rdfs:label            "VoltageLimitSchedule"@en ;
        rdfs:range            nc:VoltageLimitSchedule ;
        cims:AssociationUsed  "No" ;
        cims:inverseRoleName  nc:VoltageLimitSchedule.VoltageLimit ;
        cims:multiplicity     cims:M:0..n ;
        cims:stereotype       "NC" .

nc:VoltageLimitSchedule
        rdf:type                rdfs:Class ;
        rdfs:comment            "Schedule for voltage limit." ;
        rdfs:label              "VoltageLimitSchedule"@en ;
        rdfs:subClassOf         nc:BaseIrregularTimeSeries ;
        cims:belongsToCategory  shs:Package_SteadyStateHypothesisScheduleProfile ;
        cims:stereotype         "NC" ;
        cims:stereotype         <http://iec.ch/TC57/NonStandard/UML#concrete> .

nc:VoltageLimitSchedule.VoltageLimit
        rdf:type              rdf:Property ;
        rdfs:comment          "Voltage limit which has voltage limit schedules." ;
        rdfs:domain           nc:VoltageLimitSchedule ;
        rdfs:label            "VoltageLimit"@en ;
        rdfs:range            cim:VoltageLimit ;
        cims:AssociationUsed  "Yes" ;
        cims:inverseRoleName  nc:VoltageLimit.VoltageLimitSchedule ;
        cims:multiplicity     cims:M:0..1 ;
        cims:stereotype       "NC" .

nc:VoltageLimitSchedule.VoltageLimitTimePoint
        rdf:type              rdf:Property ;
        rdfs:comment          "The time point that relates to this voltage limit schedule." ;
        rdfs:domain           nc:VoltageLimitSchedule ;
        rdfs:label            "VoltageLimitTimePoint"@en ;
        rdfs:range            nc:VoltageLimitTimePoint ;
        cims:AssociationUsed  "No" ;
        cims:inverseRoleName  nc:VoltageLimitTimePoint.VoltageLimitSchedule ;
        cims:multiplicity     cims:M:1..n ;
        cims:stereotype       "NC" ;
        cims:stereotype       <http://iec.ch/TC57/NonStandard/UML#ofAggregate> .

nc:VoltageLimitTimePoint
        rdf:type                rdfs:Class ;
        rdfs:comment            "Voltage limit values for a given point in time." ;
        rdfs:label              "VoltageLimitTimePoint"@en ;
        cims:belongsToCategory  shs:Package_SteadyStateHypothesisScheduleProfile ;
        cims:stereotype         "NC" ;
        cims:stereotype         <http://iec.ch/TC57/NonStandard/UML#concrete> .

nc:VoltageLimitTimePoint.VoltageLimitSchedule
        rdf:type              rdf:Property ;
        rdfs:comment          "The voltage limit schedule that has this time point." ;
        rdfs:domain           nc:VoltageLimitTimePoint ;
        rdfs:label            "VoltageLimitSchedule"@en ;
        rdfs:range            nc:VoltageLimitSchedule ;
        cims:AssociationUsed  "Yes" ;
        cims:inverseRoleName  nc:VoltageLimitSchedule.VoltageLimitTimePoint ;
        cims:multiplicity     cims:M:1 ;
        cims:stereotype       "NC" .

nc:VoltageLimitTimePoint.atTime
        rdf:type           rdf:Property ;
        rdfs:comment       "The time the data is valid for." ;
        rdfs:domain        nc:VoltageLimitTimePoint ;
        rdfs:label         "atTime"@en ;
        cims:dataType      cim:DateTime ;
        cims:multiplicity  cims:M:1..1 ;
        cims:stereotype    "NC" ;
        cims:stereotype    <http://iec.ch/TC57/NonStandard/UML#attribute> .

nc:VoltageLimitTimePoint.value
        rdf:type           rdf:Property ;
        rdfs:comment       "Limit on voltage. High or low limit nature of the limit depends upon the properties of the operational limit type. The attribute shall be a positive value or zero." ;
        rdfs:domain        nc:VoltageLimitTimePoint ;
        rdfs:label         "value"@en ;
        cims:dataType      cim:Voltage ;
        cims:multiplicity  cims:M:1..1 ;
        cims:stereotype    "NC" ;
        cims:stereotype    <http://iec.ch/TC57/NonStandard/UML#attribute> .

nc:VsConverter.VsConverterRegularSchedule
        rdf:type              rdf:Property ;
        rdfs:comment          "VsConverterRegularSchedule which belongs to a VSConverter." ;
        rdfs:domain           cim:VsConverter ;
        rdfs:label            "VsConverterRegularSchedule"@en ;
        rdfs:range            nc:VsConverterRegularSchedule ;
        cims:AssociationUsed  "No" ;
        cims:inverseRoleName  nc:VsConverterRegularSchedule.VsConverter ;
        cims:multiplicity     cims:M:0..n ;
        cims:stereotype       "NC" .

nc:VsConverter.VsConverterSchedule
        rdf:type              rdf:Property ;
        rdfs:comment          "Vs converter schedule associated with a Vs converter." ;
        rdfs:domain           cim:VsConverter ;
        rdfs:label            "VsConverterSchedule"@en ;
        rdfs:range            nc:VsConverterSchedule ;
        cims:AssociationUsed  "No" ;
        cims:inverseRoleName  nc:VsConverterSchedule.VsConverter ;
        cims:multiplicity     cims:M:0..n ;
        cims:stereotype       "NC" .

nc:VsConverterRegularSchedule
        rdf:type                rdfs:Class ;
        rdfs:comment            "Regular schedule for VS converter." ;
        rdfs:label              "VsConverterRegularSchedule"@en ;
        rdfs:subClassOf         nc:ACDCConverterRegularSchedule ;
        cims:belongsToCategory  shs:Package_SteadyStateHypothesisScheduleProfile ;
        cims:stereotype         "NC" ;
        cims:stereotype         <http://iec.ch/TC57/NonStandard/UML#concrete> .

nc:VsConverterRegularSchedule.VsConverter
        rdf:type              rdf:Property ;
        rdfs:comment          "VsConverter which has VsConverterRegularSchedule." ;
        rdfs:domain           nc:VsConverterRegularSchedule ;
        rdfs:label            "VsConverter"@en ;
        rdfs:range            cim:VsConverter ;
        cims:AssociationUsed  "Yes" ;
        cims:inverseRoleName  nc:VsConverter.VsConverterRegularSchedule ;
        cims:multiplicity     cims:M:0..1 ;
        cims:stereotype       "NC" .

nc:VsConverterRegularSchedule.droop
        rdf:type           rdf:Property ;
        rdfs:comment       "Droop constant. The pu value is obtained as D [kV/MW] x Sb / Ubdc. The attribute shall be a positive value." ;
        rdfs:domain        nc:VsConverterRegularSchedule ;
        rdfs:label         "droop"@en ;
        cims:dataType      cim:PU ;
        cims:multiplicity  cims:M:0..1 ;
        cims:stereotype    <http://iec.ch/TC57/NonStandard/UML#attribute> .

nc:VsConverterRegularSchedule.droopCompensation
        rdf:type           rdf:Property ;
        rdfs:comment       "Compensation constant. Used to compensate for voltage drop when controlling voltage at a distant bus. The attribute shall be a positive value." ;
        rdfs:domain        nc:VsConverterRegularSchedule ;
        rdfs:label         "droopCompensation"@en ;
        cims:dataType      cim:Resistance ;
        cims:multiplicity  cims:M:0..1 ;
        cims:stereotype    <http://iec.ch/TC57/NonStandard/UML#attribute> .

nc:VsConverterRegularSchedule.pPccControl
        rdf:type           rdf:Property ;
        rdfs:comment       "Kind of control of real power and/or DC voltage." ;
        rdfs:domain        nc:VsConverterRegularSchedule ;
        rdfs:label         "pPccControl"@en ;
        rdfs:range         cim:VsPpccControlKind ;
        cims:multiplicity  cims:M:1..1 ;
        cims:stereotype    <http://iec.ch/TC57/NonStandard/UML#attribute> .

nc:VsConverterRegularSchedule.qPccControl
        rdf:type           rdf:Property ;
        rdfs:comment       "Kind of reactive power control." ;
        rdfs:domain        nc:VsConverterRegularSchedule ;
        rdfs:label         "qPccControl"@en ;
        rdfs:range         cim:VsQpccControlKind ;
        cims:multiplicity  cims:M:1..1 ;
        cims:stereotype    <http://iec.ch/TC57/NonStandard/UML#attribute> .

nc:VsConverterRegularSchedule.qShare
        rdf:type           rdf:Property ;
        rdfs:comment       "Reactive power sharing factor among parallel converters on Uac control. The attribute shall be a positive value or zero." ;
        rdfs:domain        nc:VsConverterRegularSchedule ;
        rdfs:label         "qShare"@en ;
        cims:dataType      cim:PerCent ;
        cims:multiplicity  cims:M:0..1 ;
        cims:stereotype    <http://iec.ch/TC57/NonStandard/UML#attribute> .

nc:VsConverterRegularSchedule.targetPWMfactor
        rdf:type           rdf:Property ;
        rdfs:comment       "Magnitude of pulse-modulation factor. The attribute shall be a positive value." ;
        rdfs:domain        nc:VsConverterRegularSchedule ;
        rdfs:label         "targetPWMfactor"@en ;
        cims:dataType      cim:Float ;
        cims:multiplicity  cims:M:0..1 ;
        cims:stereotype    <http://iec.ch/TC57/NonStandard/UML#attribute> .

nc:VsConverterRegularSchedule.targetPhasePcc
        rdf:type           rdf:Property ;
        rdfs:comment       "Phase target at AC side, at point of common coupling. The attribute shall be a positive value." ;
        rdfs:domain        nc:VsConverterRegularSchedule ;
        rdfs:label         "targetPhasePcc"@en ;
        cims:dataType      cim:AngleDegrees ;
        cims:multiplicity  cims:M:0..1 ;
        cims:stereotype    <http://iec.ch/TC57/NonStandard/UML#attribute> .

nc:VsConverterRegularSchedule.targetPowerFactorPcc
        rdf:type           rdf:Property ;
        rdfs:comment       "Power factor target at the AC side, at point of common coupling. The attribute shall be a positive value." ;
        rdfs:domain        nc:VsConverterRegularSchedule ;
        rdfs:label         "targetPowerFactorPcc"@en ;
        cims:dataType      cim:Float ;
        cims:multiplicity  cims:M:0..1 ;
        cims:stereotype    <http://iec.ch/TC57/NonStandard/UML#attribute> .

nc:VsConverterRegularSchedule.targetQpcc
        rdf:type           rdf:Property ;
        rdfs:comment       "Reactive power injection target in AC grid, at point of common coupling.  Load sign convention is used, i.e. positive sign means flow out from a node." ;
        rdfs:domain        nc:VsConverterRegularSchedule ;
        rdfs:label         "targetQpcc"@en ;
        cims:dataType      cim:ReactivePower ;
        cims:multiplicity  cims:M:0..1 ;
        cims:stereotype    <http://iec.ch/TC57/NonStandard/UML#attribute> .

nc:VsConverterRegularSchedule.targetUpcc
        rdf:type           rdf:Property ;
        rdfs:comment       "Voltage target in AC grid, at point of common coupling. The attribute shall be a positive value." ;
        rdfs:domain        nc:VsConverterRegularSchedule ;
        rdfs:label         "targetUpcc"@en ;
        cims:dataType      cim:Voltage ;
        cims:multiplicity  cims:M:0..1 ;
        cims:stereotype    <http://iec.ch/TC57/NonStandard/UML#attribute> .

nc:VsConverterSchedule
        rdf:type                rdfs:Class ;
        rdfs:comment            "Schedule for VS converter." ;
        rdfs:label              "VsConverterSchedule"@en ;
        rdfs:subClassOf         nc:BaseIrregularTimeSeries ;
        cims:belongsToCategory  shs:Package_SteadyStateHypothesisScheduleProfile ;
        cims:stereotype         "NC" ;
        cims:stereotype         <http://iec.ch/TC57/NonStandard/UML#concrete> .

nc:VsConverterSchedule.VsConverter
        rdf:type              rdf:Property ;
        rdfs:comment          "Vs converter which has Vs converter schedules." ;
        rdfs:domain           nc:VsConverterSchedule ;
        rdfs:label            "VsConverter"@en ;
        rdfs:range            cim:VsConverter ;
        cims:AssociationUsed  "Yes" ;
        cims:inverseRoleName  nc:VsConverter.VsConverterSchedule ;
        cims:multiplicity     cims:M:0..1 ;
        cims:stereotype       "NC" .

nc:VsConverterSchedule.VsConverterTimePoint
        rdf:type              rdf:Property ;
        rdfs:comment          "The time point that relates to this VS converter schedule." ;
        rdfs:domain           nc:VsConverterSchedule ;
        rdfs:label            "VsConverterTimePoint"@en ;
        rdfs:range            nc:VsConverterTimePoint ;
        cims:AssociationUsed  "No" ;
        cims:inverseRoleName  nc:VsConverterTimePoint.VsConverterSchedule ;
        cims:multiplicity     cims:M:1..n ;
        cims:stereotype       "NC" ;
        cims:stereotype       <http://iec.ch/TC57/NonStandard/UML#ofAggregate> .

nc:VsConverterTimePoint
        rdf:type                rdfs:Class ;
        rdfs:comment            "VS converter values for a given point in time." ;
        rdfs:label              "VsConverterTimePoint"@en ;
        rdfs:subClassOf         nc:ACDCTimePoint ;
        cims:belongsToCategory  shs:Package_SteadyStateHypothesisScheduleProfile ;
        cims:stereotype         "NC" ;
        cims:stereotype         <http://iec.ch/TC57/NonStandard/UML#concrete> .

nc:VsConverterTimePoint.VsConverterSchedule
        rdf:type              rdf:Property ;
        rdfs:comment          "The VS converter schedule that has this time point." ;
        rdfs:domain           nc:VsConverterTimePoint ;
        rdfs:label            "VsConverterSchedule"@en ;
        rdfs:range            nc:VsConverterSchedule ;
        cims:AssociationUsed  "Yes" ;
        cims:inverseRoleName  nc:VsConverterSchedule.VsConverterTimePoint ;
        cims:multiplicity     cims:M:1 ;
        cims:stereotype       "NC" .

nc:VsConverterTimePoint.droop
        rdf:type           rdf:Property ;
        rdfs:comment       "Droop constant. The pu value is obtained as D [kV/MW] x Sb / Ubdc. The attribute shall be a positive value." ;
        rdfs:domain        nc:VsConverterTimePoint ;
        rdfs:label         "droop"@en ;
        cims:dataType      cim:PU ;
        cims:multiplicity  cims:M:0..1 ;
        cims:stereotype    "NC" ;
        cims:stereotype    <http://iec.ch/TC57/NonStandard/UML#attribute> .

nc:VsConverterTimePoint.droopCompensation
        rdf:type           rdf:Property ;
        rdfs:comment       "Compensation constant. Used to compensate for voltage drop when controlling voltage at a distant bus. The attribute shall be a positive value." ;
        rdfs:domain        nc:VsConverterTimePoint ;
        rdfs:label         "droopCompensation"@en ;
        cims:dataType      cim:Resistance ;
        cims:multiplicity  cims:M:0..1 ;
        cims:stereotype    "NC" ;
        cims:stereotype    <http://iec.ch/TC57/NonStandard/UML#attribute> .

nc:VsConverterTimePoint.pPccControl
        rdf:type           rdf:Property ;
        rdfs:comment       "Kind of control of real power and/or DC voltage." ;
        rdfs:domain        nc:VsConverterTimePoint ;
        rdfs:label         "pPccControl"@en ;
        rdfs:range         cim:VsPpccControlKind ;
        cims:multiplicity  cims:M:1..1 ;
        cims:stereotype    "NC" ;
        cims:stereotype    <http://iec.ch/TC57/NonStandard/UML#attribute> .

nc:VsConverterTimePoint.qPccControl
        rdf:type           rdf:Property ;
        rdfs:comment       "Kind of reactive power control." ;
        rdfs:domain        nc:VsConverterTimePoint ;
        rdfs:label         "qPccControl"@en ;
        rdfs:range         cim:VsQpccControlKind ;
        cims:multiplicity  cims:M:1..1 ;
        cims:stereotype    "NC" ;
        cims:stereotype    <http://iec.ch/TC57/NonStandard/UML#attribute> .

nc:VsConverterTimePoint.qShare
        rdf:type           rdf:Property ;
        rdfs:comment       "Reactive power sharing factor among parallel converters on Uac control. The attribute shall be a positive value or zero." ;
        rdfs:domain        nc:VsConverterTimePoint ;
        rdfs:label         "qShare"@en ;
        cims:dataType      cim:PerCent ;
        cims:multiplicity  cims:M:0..1 ;
        cims:stereotype    "NC" ;
        cims:stereotype    <http://iec.ch/TC57/NonStandard/UML#attribute> .

nc:VsConverterTimePoint.targetPWMfactor
        rdf:type           rdf:Property ;
        rdfs:comment       "Magnitude of pulse-modulation factor. The attribute shall be a positive value." ;
        rdfs:domain        nc:VsConverterTimePoint ;
        rdfs:label         "targetPWMfactor"@en ;
        cims:dataType      cim:Float ;
        cims:multiplicity  cims:M:0..1 ;
        cims:stereotype    "NC" ;
        cims:stereotype    <http://iec.ch/TC57/NonStandard/UML#attribute> .

nc:VsConverterTimePoint.targetPhasePcc
        rdf:type           rdf:Property ;
        rdfs:comment       "Phase target at AC side, at point of common coupling. The attribute shall be a positive value." ;
        rdfs:domain        nc:VsConverterTimePoint ;
        rdfs:label         "targetPhasePcc"@en ;
        cims:dataType      cim:AngleDegrees ;
        cims:multiplicity  cims:M:0..1 ;
        cims:stereotype    "NC" ;
        cims:stereotype    <http://iec.ch/TC57/NonStandard/UML#attribute> .

nc:VsConverterTimePoint.targetPowerFactorPcc
        rdf:type           rdf:Property ;
        rdfs:comment       "Power factor target at the AC side, at point of common coupling. The attribute shall be a positive value." ;
        rdfs:domain        nc:VsConverterTimePoint ;
        rdfs:label         "targetPowerFactorPcc"@en ;
        cims:dataType      cim:Float ;
        cims:multiplicity  cims:M:0..1 ;
        cims:stereotype    "NC" ;
        cims:stereotype    <http://iec.ch/TC57/NonStandard/UML#attribute> .

nc:VsConverterTimePoint.targetQpcc
        rdf:type           rdf:Property ;
        rdfs:comment       "Reactive power injection target in AC grid, at point of common coupling.  Load sign convention is used, i.e. positive sign means flow out from a node." ;
        rdfs:domain        nc:VsConverterTimePoint ;
        rdfs:label         "targetQpcc"@en ;
        cims:dataType      cim:ReactivePower ;
        cims:multiplicity  cims:M:0..1 ;
        cims:stereotype    "NC" ;
        cims:stereotype    <http://iec.ch/TC57/NonStandard/UML#attribute> .

nc:VsConverterTimePoint.targetUpcc
        rdf:type           rdf:Property ;
        rdfs:comment       "Voltage target in AC grid, at point of common coupling. The attribute shall be a positive value." ;
        rdfs:domain        nc:VsConverterTimePoint ;
        rdfs:label         "targetUpcc"@en ;
        cims:dataType      cim:Voltage ;
        cims:multiplicity  cims:M:0..1 ;
        cims:stereotype    "NC" ;
        cims:stereotype    <http://iec.ch/TC57/NonStandard/UML#attribute> .

profcim:IRI  rdf:type           rdfs:Class ;
        rdfs:comment            "An IRI (Internationalized Resource Identifier) within an RDF graph is a Unicode string that conforms to the syntax defined in RFC 3987.\nThe primitive is serialized as rdf:resource in RDFXML.\nIRIs in the RDF abstract syntax must be absolute, and may contain a fragment identifier.\nIRI equality: Two IRIs are equal if and only if they are equivalent under Simple String Comparison according to section 5.1 of [RFC3987]. Further normalization must not be performed when comparing IRIs for equality.\nIRIs are a generalization of URIs [RFC3986] that permits a wider range of Unicode characters. Every absolute URI and URL is an IRI, but not every IRI is an URI. When IRIs are used in operations that are only defined for URIs, they must first be converted according to the mapping defined in section 3.1 of [RFC3987]. A notable example is retrieval over the HTTP protocol. The mapping involves UTF-8 encoding of non-ASCII characters, %-encoding of octets not allowed in URIs, and Punycode-encoding of domain names." ;
        rdfs:label              "IRI"@en ;
        cims:belongsToCategory  shs:Package_DocSteadyStateHypothesisScheduleProfile ;
        cims:stereotype         "profcim" , "Primitive" .

profcim:StringFixedLanguage
        rdf:type                rdfs:Class ;
        rdfs:comment            "A string consisting of a sequence of characters. The character encoding is UTF-8. The string length is unspecified and unlimited.\nThe primitive is serialized as literal without language support." ;
        rdfs:label              "StringFixedLanguage"@en ;
        cims:belongsToCategory  shs:Package_DocSteadyStateHypothesisScheduleProfile ;
        cims:stereotype         "profcim" , "Primitive" .

profcim:StringIRI  rdf:type     rdfs:Class ;
        rdfs:comment            "An IRI (Internationalized Resource Identifier) within an RDF graph is a Unicode string that conforms to the syntax defined in RFC 3987.\nThe primitive is serialized as literal without language support.\nIRIs in the RDF abstract syntax must be absolute, and may contain a fragment identifier.\nIRI equality: Two IRIs are equal if and only if they are equivalent under Simple String Comparison according to section 5.1 of [RFC3987]. Further normalization must not be performed when comparing IRIs for equality.\nIRIs are a generalization of URIs [RFC3986] that permits a wider range of Unicode characters. Every absolute URI and URL is an IRI, but not every IRI is an URI. When IRIs are used in operations that are only defined for URIs, they must first be converted according to the mapping defined in section 3.1 of [RFC3987]. A notable example is retrieval over the HTTP protocol. The mapping involves UTF-8 encoding of non-ASCII characters, %-encoding of octets not allowed in URIs, and Punycode-encoding of domain names." ;
        rdfs:label              "StringIRI"@en ;
        cims:belongsToCategory  shs:Package_DocSteadyStateHypothesisScheduleProfile ;
        cims:stereotype         "profcim" , "Primitive" .

profcim:URL  rdf:type           rdfs:Class ;
        rdfs:comment            "A Uniform Resource Locator (URL), colloquially termed a web address, is a reference to a web resource that specifies its location on a computer network and a mechanism for retrieving it. A URL is a specific type of Uniform Resource Identifier (URI), although many people use the two terms interchangeably.URLs occur most commonly to reference web pages (http), but are also used for file transfer (ftp), email (mailto), database access (JDBC), and many other applications." ;
        rdfs:label              "URL"@en ;
        cims:belongsToCategory  shs:Package_DocSteadyStateHypothesisScheduleProfile ;
        cims:stereotype         "profcim" , "Primitive" .

shs:Ontology  rdf:type        owl:Ontology ;
        dcterms:conformsTo    "file://iec61970cim17v40_iec61968cim13v13a_iec62325cim03v17a.eap" , "urn:iso:std:iec:61970-501:draft:ed-2" , "file://CIM100_CGMES31v01_501-20v02_NC23v62_MM10v01.eap" , "urn:iso:std:iec:61970-401:draft:ed-1" , "urn:iso:std:iec:61970-600-2:ed-1" , "urn:iso:std:iec:61970-301:ed-7:amd1" ;
        dcterms:creator       "ENTSO-E CIM WG NC project"@en ;
        dcterms:description   "This vocabulary is describing the steady state hypothesis schedule."@en ;
        dcterms:identifier    "urn:uuid:0d815deb-9968-4c6f-85d7-503d49e0b81f" ;
        dcterms:language      "en-GB" ;
        dcterms:license       "https://www.apache.org/licenses/LICENSE-2.0"@en ;
        dcterms:modified      "2024-04-08"^^<http://www.w3.org/2001/XMLSchema#date> ;
        dcterms:publisher     "ENTSO-E"@en ;
        dcterms:rightsHolder  "ENTSO-E"@en ;
        dcterms:title         "Steady State Hypothesis Schedule Vocabulary"@en ;
        owl:versionIRI        <https://ap.cim4.eu/SteadyStateHypothesisSchedule/1.0> ;
        owl:versionInfo       "1.0.0"@en ;
        dcat:keyword          "SHS" ;
        dcat:theme            "vocabulary"@en .

shs:Package_DocSteadyStateHypothesisScheduleProfile
        rdf:type      cims:ClassCategory ;
        rdfs:comment  "This package contains datatypes used only in the RDFS header." ;
        rdfs:label    "DocSteadyStateHypothesisScheduleProfile"@en .

shs:Package_SteadyStateHypothesisScheduleProfile
        rdf:type      cims:ClassCategory ;
        rdfs:comment  "This package contains steady state hypothesis schedule profile." ;
        rdfs:label    "SteadyStateHypothesisScheduleProfile"@en .

